@prefix : <https://www.archimitra.org/ontologies/archimate/> .
@prefix sh: <http://www.w3.org/ns/shacl#> .
@prefix owl: <http://www.w3.org/2002/07/owl#> .
@prefix rdf: <http://www.w3.org/1999/02/22-rdf-syntax-ns#> .
@prefix xml: <http://www.w3.org/XML/1998/namespace> .
@prefix xsd: <http://www.w3.org/2001/XMLSchema#> .
@prefix gist: <https://ontologies.semanticarts.com/gist/> .
@prefix rdfs: <http://www.w3.org/2000/01/rdf-schema#> .
@prefix skos: <http://www.w3.org/2004/02/skos/core#> .
@base <https://www.archimitra.org/ontologies/archimate/> .

<https://ontologies.semanticarts.com/o/gistCore> rdf:type owl:Ontology ;
                                                  owl:versionIRI <https://ontologies.semanticarts.com/o/gistCore11.1.0> ;
                                                  skos:definition "Archimitra architect model will try to create an upper ontology for architecture models" ;
                                                  sh:declare gist:_PrefixDeclaration_gist ;
                                                  gist:license "https://creativecommons.org/licenses/by-sa/3.0/" .

#################################################################
#    Annotation properties
#################################################################

###  http://www.w3.org/2004/02/skos/core#definition
skos:definition rdf:type owl:AnnotationProperty .


###  http://www.w3.org/2004/02/skos/core#example
skos:example rdf:type owl:AnnotationProperty .


###  http://www.w3.org/2004/02/skos/core#prefLabel
skos:prefLabel rdf:type owl:AnnotationProperty .


###  http://www.w3.org/2004/02/skos/core#scopeNote
skos:scopeNote rdf:type owl:AnnotationProperty .


###  http://www.w3.org/ns/shacl#declare
sh:declare rdf:type owl:AnnotationProperty .


###  http://www.w3.org/ns/shacl#namespace
sh:namespace rdf:type owl:AnnotationProperty .


###  http://www.w3.org/ns/shacl#prefix
sh:prefix rdf:type owl:AnnotationProperty .


###  https://ontologies.semanticarts.com/gist/domainIncludes
gist:domainIncludes rdf:type owl:AnnotationProperty ;
                    rdfs:isDefinedBy <https://ontologies.semanticarts.com/o/gistCore> ;
                    skos:definition "Relates a property to a class that is (one of) the type(s) the property is expected to be used on." ;
                    skos:example "The domain for the property gist:hasMember includes gist:Collection." ;
                    skos:prefLabel "domain includes" ;
                    skos:scopeNote "This property is used to guide the ontology user; like all annotation properties, it does not play a role in inference." ,
                                   "This property means the same thing as the Schema.org version, which is an rdf:Property and not compliant with OWL-DL." ;
                    rdfs:subPropertyOf skos:scopeNote .


###  https://ontologies.semanticarts.com/gist/license
gist:license rdf:type owl:AnnotationProperty ;
             rdfs:isDefinedBy <https://ontologies.semanticarts.com/o/gistCore> ;
             skos:definition "An annotation for providing the licensing on this or derivative ontologies" ;
             skos:prefLabel "license" .


###  https://ontologies.semanticarts.com/gist/rangeIncludes
gist:rangeIncludes rdf:type owl:AnnotationProperty ;
                   rdfs:isDefinedBy <https://ontologies.semanticarts.com/o/gistCore> ;
                   skos:definition "Relates a property to a class that constitutes (one of) the expected type(s) for values of the property." ;
                   skos:example "The range for the property gist:isCategorizedBy includes gist:Category." ;
                   skos:prefLabel "range includes" ;
                   skos:scopeNote "This property is used to guide the ontology user; like all annotation properties, it does not play a role in inference." ,
                                  "This property means the same thing as the Schema.org version, which is an rdf:Property and not compliant with OWL-DL." ;
                   rdfs:subPropertyOf skos:scopeNote .


#################################################################
#    Object Properties
#################################################################

###  https://ontologies.semanticarts.com/gist/accepts
gist:accepts rdf:type owl:ObjectProperty ;
             rdfs:isDefinedBy <https://ontologies.semanticarts.com/o/gistCore> ;
             skos:definition "The types of input messages that will be allowed." ;
             skos:prefLabel "accepts" .


###  https://ontologies.semanticarts.com/gist/affects
gist:affects rdf:type owl:ObjectProperty ;
             owl:inverseOf gist:isAffectedBy ;
             rdfs:isDefinedBy <https://ontologies.semanticarts.com/o/gistCore> ;
             skos:definition "The subject has, had, or will have an effect on the object." ;
             skos:prefLabel "affects" .


###  https://ontologies.semanticarts.com/gist/allows
gist:allows rdf:type owl:ObjectProperty ;
            rdfs:domain gist:Intention ;
            rdfs:range gist:Behavior ;
            rdfs:isDefinedBy <https://ontologies.semanticarts.com/o/gistCore> ;
            skos:definition "The intention (say a grant) allows a particular kind of activity (for instance egress)" ;
            skos:prefLabel "allows" .


###  https://ontologies.semanticarts.com/gist/comesFromAgent
gist:comesFromAgent rdf:type owl:ObjectProperty ;
                    rdfs:subPropertyOf gist:hasParticipant ;
                    rdfs:range [ rdf:type owl:Class ;
                                 owl:unionOf ( gist:Organization
                                               gist:Person
                                             )
                               ] ;
                    rdfs:isDefinedBy <https://ontologies.semanticarts.com/o/gistCore> ;
                    skos:definition "The party that is the source of something (e.g. a message, shipment, etc.)" ;
                    skos:prefLabel "comes from agent" ;
                    skos:scopeNote "This is not the inverse of gist:goesToAgent. A message can be to someone. If we made it the inverse the person would be \"from\" the message" .


###  https://ontologies.semanticarts.com/gist/comesFromPlace
gist:comesFromPlace rdf:type owl:ObjectProperty ;
                    rdfs:range [ rdf:type owl:Class ;
                                 owl:unionOf ( gist:Address
                                               gist:Place
                                             )
                               ] ;
                    rdfs:isDefinedBy <https://ontologies.semanticarts.com/o/gistCore> ;
                    skos:definition "Origin" ;
                    skos:prefLabel "comes from place" .


###  https://ontologies.semanticarts.com/gist/conformsTo
gist:conformsTo rdf:type owl:ObjectProperty ;
                rdfs:isDefinedBy <https://ontologies.semanticarts.com/o/gistCore> ;
                skos:definition "The subject conforms to the Object, e.g. meet an obligation, meet terms of an offer, adhere to a specification" ;
                skos:prefLabel "conforms to" ;
                gist:rangeIncludes gist:Intention .


###  https://ontologies.semanticarts.com/gist/containsGeographically
gist:containsGeographically rdf:type owl:ObjectProperty ;
                            owl:inverseOf gist:isGeographicallyContainedIn ;
                            rdf:type owl:TransitiveProperty ;
                            rdfs:domain gist:Place ;
                            rdfs:range gist:Place ;
                            rdfs:isDefinedBy <https://ontologies.semanticarts.com/o/gistCore> ;
                            skos:definition "Relate one place to another place that is contained within the first." ;
                            skos:prefLabel "contains geographically" .


###  https://ontologies.semanticarts.com/gist/contributesTo
gist:contributesTo rdf:type owl:ObjectProperty ;
                   rdfs:isDefinedBy <https://ontologies.semanticarts.com/o/gistCore> ;
                   skos:definition "The parts of a system contribute to the goal/ function of the whole system" ;
                   skos:prefLabel "contributes to" .


###  https://ontologies.semanticarts.com/gist/directs
gist:directs rdf:type owl:ObjectProperty ;
             rdfs:isDefinedBy <https://ontologies.semanticarts.com/o/gistCore> ;
             skos:definition "The set of actuators that a controller can affect" ;
             skos:prefLabel "directs" .


###  https://ontologies.semanticarts.com/gist/follows
gist:follows rdf:type owl:ObjectProperty ;
             owl:inverseOf gist:precedes ;
             rdf:type owl:TransitiveProperty ;
             rdfs:isDefinedBy <https://ontologies.semanticarts.com/o/gistCore> ;
             skos:definition "A generic ordering relation indicating that the subject comes after the object." ;
             skos:prefLabel "follows" ;
             skos:scopeNote "The greater-than symbol is often used to represent this relation." ,
                            "This is the transitive version of gist:followsDirectly." ,
                            "Typically this predicate would be used asymmetricallly and irreflexively, but the ontology does not formalize this." .


###  https://ontologies.semanticarts.com/gist/followsDirectly
gist:followsDirectly rdf:type owl:ObjectProperty ;
                     rdfs:subPropertyOf gist:follows ;
                     owl:inverseOf gist:precedesDirectly ;
                     rdfs:isDefinedBy <https://ontologies.semanticarts.com/o/gistCore> ;
                     skos:definition "A generic ordering relation indicating that the subject comes immediately after the object." ;
                     skos:prefLabel "follows directly" ;
                     skos:scopeNote "If two items in an ordered collection share the same position, they both directly follow the preceding element." ,
                                    "It is safest to use this property only when the directness has a semantic correspondence with the world. Only break a direct link by inserting an intermediate item when that change corresponds to a change in the world." ,
                                    "Typically this predicate would be used asymmetricallly and irreflexively, but the ontology does not formalize this." .


###  https://ontologies.semanticarts.com/gist/goesToAgent
gist:goesToAgent rdf:type owl:ObjectProperty ;
                 rdfs:subPropertyOf gist:hasParticipant ;
                 rdfs:range [ rdf:type owl:Class ;
                              owl:unionOf ( gist:Organization
                                            gist:Person
                                          )
                            ] ;
                 rdfs:isDefinedBy <https://ontologies.semanticarts.com/o/gistCore> ;
                 skos:definition "The party that is the recipient of something (e.g. a message, shipment, etc.)" ;
                 skos:prefLabel "goes to agent" ;
                 skos:scopeNote "This is not the inverse of gist:comesFromAgent. A message can be from someone. If we made it the inverse the person would be \"to\" the message" .


###  https://ontologies.semanticarts.com/gist/goesToPlace
gist:goesToPlace rdf:type owl:ObjectProperty ;
                 rdfs:range [ rdf:type owl:Class ;
                              owl:unionOf ( gist:Address
                                            gist:Place
                                          )
                            ] ;
                 rdfs:isDefinedBy <https://ontologies.semanticarts.com/o/gistCore> ;
                 skos:definition "Destination" ;
                 skos:prefLabel "goes to place" .


###  https://ontologies.semanticarts.com/gist/governs
gist:governs rdf:type owl:ObjectProperty ;
             owl:inverseOf gist:isGovernedBy ;
             rdfs:domain [ rdf:type owl:Class ;
                           owl:unionOf ( gist:Intention
                                         gist:Organization
                                         gist:Person
                                         gist:Template
                                       )
                         ] ;
             rdfs:range [ rdf:type owl:Class ;
                          owl:unionOf ( gist:Category
                                        gist:Content
                                        gist:GeoRegion
                                        gist:IntellectualProperty
                                        gist:Intention
                                        gist:Organization
                                        gist:Person
                                        gist:PhysicalIdentifiableItem
                                        gist:PhysicalSubstance
                                      )
                        ] ;
             rdfs:isDefinedBy <https://ontologies.semanticarts.com/o/gistCore> ;
             skos:definition "The subject controls or inhibits the object in some way" ;
             skos:prefLabel "governs" .


###  https://ontologies.semanticarts.com/gist/hasAddress
gist:hasAddress rdf:type owl:ObjectProperty ;
                rdfs:range gist:Address ;
                rdfs:isDefinedBy <https://ontologies.semanticarts.com/o/gistCore> ;
                skos:definition "Relates the subject to its physical or virtual address." ;
                skos:example "The street address of a building; the email address of a person." ;
                skos:prefLabel "has address" .


###  https://ontologies.semanticarts.com/gist/hasAltitude
gist:hasAltitude rdf:type owl:ObjectProperty ;
                 rdfs:domain gist:GeoPoint ;
                 rdfs:range gist:Extent ;
                 rdfs:isDefinedBy <https://ontologies.semanticarts.com/o/gistCore> ;
                 skos:definition "Distance above sea level" ;
                 skos:prefLabel "has altitude" .


###  https://ontologies.semanticarts.com/gist/hasBaseUnit
gist:hasBaseUnit rdf:type owl:ObjectProperty ;
                 rdfs:subPropertyOf gist:hasStandardUnit ;
                 rdfs:domain gist:UnitOfMeasure ;
                 rdfs:range gist:BaseUnit ;
                 rdfs:isDefinedBy <https://ontologies.semanticarts.com/o/gistCore> ;
                 skos:definition "Relates a UnitOfMeasure to its BaseUnit.  This indicates what kind of Unit something is." ;
                 skos:example "Saying that a furlong hasBaseUnit  meter says it is a DistanceUnit." ;
                 skos:prefLabel "has base unit" .


###  https://ontologies.semanticarts.com/gist/hasBiologicalParent
gist:hasBiologicalParent rdf:type owl:ObjectProperty ;
                         rdfs:domain gist:LivingThing ;
                         rdfs:range gist:LivingThing ;
                         rdfs:isDefinedBy <https://ontologies.semanticarts.com/o/gistCore> ;
                         skos:definition "Relates a living thing to its biological parent." ;
                         skos:prefLabel "has biological parent" .


###  https://ontologies.semanticarts.com/gist/hasCommunicationAddress
gist:hasCommunicationAddress rdf:type owl:ObjectProperty ;
                             rdfs:subPropertyOf gist:hasAddress ;
                             rdfs:domain [ rdf:type owl:Class ;
                                           owl:unionOf ( gist:Organization
                                                         gist:Person
                                                       )
                                         ] ;
                             rdfs:range gist:Address ;
                             rdfs:isDefinedBy <https://ontologies.semanticarts.com/o/gistCore> ;
                             skos:definition "Relates a Person or Organization to where they can receive messages, including postal addresses, fax numbers, phone numbers, email, web site, etc." ;
                             skos:prefLabel "has communication address" .


###  https://ontologies.semanticarts.com/gist/hasDenominator
gist:hasDenominator rdf:type owl:ObjectProperty ;
                    rdfs:isDefinedBy <https://ontologies.semanticarts.com/o/gistCore> ;
                    skos:definition "Relates a RatioUnit such as meters/second to the denominator Unit (e.g. second)." ;
                    skos:prefLabel "has denominator" .


###  https://ontologies.semanticarts.com/gist/hasDirectPart
gist:hasDirectPart rdf:type owl:ObjectProperty ;
                   rdfs:subPropertyOf gist:hasPart ;
                   owl:inverseOf gist:isDirectPartOf ;
                   rdfs:isDefinedBy <https://ontologies.semanticarts.com/o/gistCore> ;
                   skos:definition "The relationship between a whole and a part where the part has independent existence." ;
                   skos:prefLabel "has direct part" ;
                   skos:scopeNote "It is safest to use this property when there is semantic directness inherent in the relationship, rather than choosing appropriate granularity. For example, a spark plug is a direct part of an engine block; there cannot be any intermediate parts.  Beware of making a hasDirectPart assertion and then inserting an intermediate part; this will result in making an asserted triple false even though there was no change in the world." ,
                                  "No cascading delete." ,
                                  "Use this property to directly associate a part with the whole. gist:hasPart is the transitive version." .


###  https://ontologies.semanticarts.com/gist/hasDirectSubCategory
gist:hasDirectSubCategory rdf:type owl:ObjectProperty ;
                          rdfs:subPropertyOf gist:hasSubCategory ;
                          rdfs:isDefinedBy <https://ontologies.semanticarts.com/o/gistCore> ;
                          skos:definition "The subject category is a supercategory of the object category. This property defines the direct links in a category hierarchy; no intermediate categories can exist between the direct links." ;
                          skos:prefLabel "has direct subcategory" ;
                          skos:scopeNote "Unlike its superproperty gist:hasSubCategory, this property is not transitive. It is essentially the same as the non-transitive skos:narrower, using gist:Category rather than skos:Concept." .


###  https://ontologies.semanticarts.com/gist/hasDirectSubTask
gist:hasDirectSubTask rdf:type owl:ObjectProperty ;
                      rdfs:subPropertyOf gist:hasSubTask ;
                      owl:inverseOf gist:isDirectSubTaskOf ;
                      rdfs:domain gist:TaskExecution ;
                      rdfs:range gist:TaskExecution ;
                      rdfs:isDefinedBy <https://ontologies.semanticarts.com/o/gistCore> ;
                      skos:definition "Immediate child task" ;
                      skos:prefLabel "has direct sub task" .


###  https://ontologies.semanticarts.com/gist/hasDirectSuperCategory
gist:hasDirectSuperCategory rdf:type owl:ObjectProperty ;
                            rdfs:subPropertyOf gist:hasSuperCategory ;
                            rdfs:isDefinedBy <https://ontologies.semanticarts.com/o/gistCore> ;
                            skos:definition "The subject category is a subcategory of the object category. This property defines the direct links in a category hierarchy; no intermediate categories can exist between the direct links." ;
                            skos:prefLabel "has direct supercategory" ;
                            skos:scopeNote "Unlike its superproperty gist:hasSuperCategory, this property is not transitive. It is essentially the same as the non-transitive skos:broader, using gist:Category rather than skos:Concept." .


###  https://ontologies.semanticarts.com/gist/hasFirstMember
gist:hasFirstMember rdf:type owl:ObjectProperty ;
                    rdfs:subPropertyOf gist:hasMember ;
                    rdf:type owl:InverseFunctionalProperty ;
                    rdfs:domain gist:OrderedCollection ;
                    rdfs:range gist:OrderedMember ;
                    rdfs:isDefinedBy <https://ontologies.semanticarts.com/o/gistCore> ;
                    skos:definition "Relates an ordered collection to its first member." ;
                    skos:prefLabel "has first member" ;
                    skos:scopeNote "Given the Open World Assumption, the absence of a predecessor does not entail that an ordered member is the first member of an ordered collection. This property is used to explicitly indicate the first member. Since ordered collections may not be strictly ordered, there can be more than one first member." .


###  https://ontologies.semanticarts.com/gist/hasGiver
gist:hasGiver rdf:type owl:ObjectProperty ;
              rdfs:subPropertyOf gist:hasParticipant ;
              owl:propertyDisjointWith gist:hasRecipient ;
              rdfs:isDefinedBy <https://ontologies.semanticarts.com/o/gistCore> ;
              skos:definition "The active party, the one with the obligation or the one initiating the transfer" ;
              skos:prefLabel "has giver" .


###  https://ontologies.semanticarts.com/gist/hasGoal
gist:hasGoal rdf:type owl:ObjectProperty ;
             rdfs:isDefinedBy <https://ontologies.semanticarts.com/o/gistCore> ;
             skos:definition "The reason for doing something" ;
             skos:prefLabel "has goal" .


###  https://ontologies.semanticarts.com/gist/hasIncumbent
gist:hasIncumbent rdf:type owl:ObjectProperty ;
                  rdfs:isDefinedBy <https://ontologies.semanticarts.com/o/gistCore> ;
                  skos:definition "What equipment or person is currently in this node.  Note to create a temporal view make a TemporalRelation for this property" ;
                  skos:prefLabel "has incumbent" .


###  https://ontologies.semanticarts.com/gist/hasMagnitude
gist:hasMagnitude rdf:type owl:ObjectProperty ;
                  rdfs:range gist:Magnitude ;
                  rdfs:isDefinedBy <https://ontologies.semanticarts.com/o/gistCore> ;
                  skos:definition "To have a comparable numeric value. Each magnitude has a unit." ;
                  skos:prefLabel "has magnitude" .


###  https://ontologies.semanticarts.com/gist/hasMember
gist:hasMember rdf:type owl:ObjectProperty ;
               owl:inverseOf gist:isMemberOf ;
               rdfs:isDefinedBy <https://ontologies.semanticarts.com/o/gistCore> ;
               skos:definition "Relates a Collection to its member individuals." ;
               skos:prefLabel "has member" ;
               gist:domainIncludes gist:Collection .


###  https://ontologies.semanticarts.com/gist/hasMultiplicand
gist:hasMultiplicand rdf:type owl:ObjectProperty ;
                     rdfs:isDefinedBy <https://ontologies.semanticarts.com/o/gistCore> ;
                     skos:definition "Relates a ProductUnit such as square mile to the second of two units multiplied together (e.g. mile)." ;
                     skos:prefLabel "has multiplicand" .


###  https://ontologies.semanticarts.com/gist/hasMultiplier
gist:hasMultiplier rdf:type owl:ObjectProperty ;
                   rdfs:isDefinedBy <https://ontologies.semanticarts.com/o/gistCore> ;
                   skos:definition "Relates a ProductUnit such as square mile to the first of two units multiplied together (e.g. mile)" ;
                   skos:prefLabel "has multiplier" .


###  https://ontologies.semanticarts.com/gist/hasNavigationalChild
gist:hasNavigationalChild rdf:type owl:ObjectProperty ;
                          owl:inverseOf gist:hasNavigationalParent ;
                          rdfs:isDefinedBy <https://ontologies.semanticarts.com/o/gistCore> ;
                          skos:definition "Relates a parent category to a child category in an informal (e.g., faceted) hierarchy." ;
                          skos:example "Refrigerator handles are not refrigerators, but it may be useful to represent their relationship hierarchically for a faceted UI filter." ;
                          skos:prefLabel "has navigational child" .


###  https://ontologies.semanticarts.com/gist/hasNavigationalParent
gist:hasNavigationalParent rdf:type owl:ObjectProperty ;
                           rdfs:isDefinedBy <https://ontologies.semanticarts.com/o/gistCore> ;
                           skos:definition "Relates a child category to a parent category in an informal (e.g., faceted) hierarchy." ;
                           skos:example "Refrigerator handles are not refrigerators, but it may be useful to represent their relationship hierarchically for a faceted UI filter." ;
                           skos:prefLabel "has navigational parent" .


###  https://ontologies.semanticarts.com/gist/hasNumerator
gist:hasNumerator rdf:type owl:ObjectProperty ;
                  rdfs:isDefinedBy <https://ontologies.semanticarts.com/o/gistCore> ;
                  skos:definition "Relates a RatioUnit such as meter(s)/second to the numerator Unit (e.g. meter)." ;
                  skos:prefLabel "has numerator" .


###  https://ontologies.semanticarts.com/gist/hasOffsetToUniversal
gist:hasOffsetToUniversal rdf:type owl:ObjectProperty ;
                          rdfs:domain gist:TimeZone ;
                          rdfs:range gist:Duration ;
                          rdfs:isDefinedBy <https://ontologies.semanticarts.com/o/gistCore> ;
                          skos:definition "How many hours the time zone is off GMT" ;
                          skos:prefLabel "has offset to universal" .


###  https://ontologies.semanticarts.com/gist/hasPart
gist:hasPart rdf:type owl:ObjectProperty ;
             owl:inverseOf gist:isPartOf ;
             rdf:type owl:TransitiveProperty ;
             rdfs:isDefinedBy <https://ontologies.semanticarts.com/o/gistCore> ;
             skos:definition "The transitive version of gist:hasDirectPart" ;
             skos:prefLabel "has part" .


###  https://ontologies.semanticarts.com/gist/hasParticipant
gist:hasParticipant rdf:type owl:ObjectProperty ;
                    rdfs:isDefinedBy <https://ontologies.semanticarts.com/o/gistCore> ;
                    skos:definition "Relates something (e.g. an agreement) to things that play a role, or take part or are otherwise involved in some way." ;
                    skos:example "An event of transferring money has a participating account that receives the money." ;
                    skos:prefLabel "has participant" ;
                    skos:scopeNote "The thing with participants will often be an agreement, event or obligation." ,
                                   "This is intended as an abstract property. Only its subproperties will be directly used." .


###  https://ontologies.semanticarts.com/gist/hasParty
gist:hasParty rdf:type owl:ObjectProperty ;
              rdfs:subPropertyOf gist:hasParticipant ;
              rdfs:range [ rdf:type owl:Class ;
                           owl:unionOf ( gist:Organization
                                         gist:Person
                                       )
                         ] ;
              rdfs:isDefinedBy <https://ontologies.semanticarts.com/o/gistCore> ;
              skos:definition "The people or organizations participating in an event, agreement or obligation" ;
              skos:example "For loan agreements, one might create hasLender and hasBorrower as subproperties of hasParty." ;
              skos:prefLabel "has party" .


###  https://ontologies.semanticarts.com/gist/hasPhysicalLocation
gist:hasPhysicalLocation rdf:type owl:ObjectProperty ,
                                  owl:TransitiveProperty ;
                         rdfs:range gist:Place ;
                         rdfs:isDefinedBy <https://ontologies.semanticarts.com/o/gistCore> ;
                         skos:definition "Where something is located" ;
                         skos:prefLabel "has physical location" .


###  https://ontologies.semanticarts.com/gist/hasPrecision
gist:hasPrecision rdf:type owl:ObjectProperty ;
                  rdfs:range gist:Magnitude ;
                  rdfs:isDefinedBy <https://ontologies.semanticarts.com/o/gistCore> ;
                  skos:definition "Links a Magnitude to the degree of accuracy of the numeric value.   This allows for fuzzy numbers.  All magnitudes have a precision.  Usually we don't record them.  When we do this, it will be a value whose extent covers 2 standard deviations around the stated magnitude" ;
                  skos:example "Temperature precise to tenth of a degree C; length precise to the nearest centimeter." ;
                  skos:prefLabel "has precision" .


###  https://ontologies.semanticarts.com/gist/hasRecipient
gist:hasRecipient rdf:type owl:ObjectProperty ;
                  rdfs:subPropertyOf gist:hasParticipant ;
                  rdfs:isDefinedBy <https://ontologies.semanticarts.com/o/gistCore> ;
                  skos:definition "The recipient" ;
                  skos:prefLabel "has recipient" .


###  https://ontologies.semanticarts.com/gist/hasStandardUnit
gist:hasStandardUnit rdf:type owl:ObjectProperty ;
                     rdfs:domain gist:UnitOfMeasure ;
                     rdfs:range gist:CoherentUnit ;
                     rdfs:isDefinedBy <https://ontologies.semanticarts.com/o/gistCore> ;
                     skos:definition "For a complex unit refers to a unit that has all the component parts in SI" ;
                     skos:prefLabel "has standard unit" .


###  https://ontologies.semanticarts.com/gist/hasSubCategory
gist:hasSubCategory rdf:type owl:ObjectProperty ;
                    owl:inverseOf gist:hasSuperCategory ;
                    rdfs:isDefinedBy <https://ontologies.semanticarts.com/o/gistCore> ;
                    skos:definition "The subject category is inclusive of, or broader than, the object category. Everything categorized by the subcategory can be inferred to be categorized by the supercategory." ;
                    skos:prefLabel "has subcategory" ;
                    skos:scopeNote "This is essentially the same as skos:narrowerTransitive, using gist:Category instead of skos:Concept." .


###  https://ontologies.semanticarts.com/gist/hasSubTask
gist:hasSubTask rdf:type owl:ObjectProperty ;
                owl:inverseOf gist:isSubTaskOf ;
                rdf:type owl:TransitiveProperty ;
                rdfs:domain gist:TaskExecution ;
                rdfs:range gist:TaskExecution ;
                rdfs:isDefinedBy <https://ontologies.semanticarts.com/o/gistCore> ;
                skos:definition "A task that is part of a larger task. The time frame of the subtasks may overlap but may not extend beyond the time frame of the parent task. A subtask may be part of more than one parent task." ;
                skos:prefLabel "has subtask" .


###  https://ontologies.semanticarts.com/gist/hasSuperCategory
gist:hasSuperCategory rdf:type owl:ObjectProperty ,
                               owl:TransitiveProperty ;
                      rdfs:isDefinedBy <https://ontologies.semanticarts.com/o/gistCore> ;
                      skos:definition "The subject category is included by, or narrower than, the object category. Everything categorized by the subcategory can be inferred to be categorized by the supercategory." ;
                      skos:prefLabel "has supercategory" ;
                      skos:scopeNote "This is essentially the same as skos:broaderTransitive, using gist:Category instead of skos:Concept." .


###  https://ontologies.semanticarts.com/gist/hasUniqueNavigationalParent
gist:hasUniqueNavigationalParent rdf:type owl:ObjectProperty ;
                                 rdfs:subPropertyOf gist:hasNavigationalParent ;
                                 rdf:type owl:FunctionalProperty ;
                                 rdfs:isDefinedBy <https://ontologies.semanticarts.com/o/gistCore> ;
                                 skos:definition "Relates a subject category to a unique parent category in an informal (e.g., faceted) hierarchy." ;
                                 skos:prefLabel "has unique navigational parent" .


###  https://ontologies.semanticarts.com/gist/hasUniqueSuperCategory
gist:hasUniqueSuperCategory rdf:type owl:ObjectProperty ;
                            rdfs:subPropertyOf gist:hasSuperCategory ;
                            rdf:type owl:FunctionalProperty ;
                            rdfs:isDefinedBy <https://ontologies.semanticarts.com/o/gistCore> ;
                            skos:definition "Used for taxos that must have single parents" ;
                            skos:prefLabel "has unique supercategory" .


###  https://ontologies.semanticarts.com/gist/hasUnitOfMeasure
gist:hasUnitOfMeasure rdf:type owl:ObjectProperty ;
                      rdfs:domain gist:Magnitude ;
                      rdfs:range gist:UnitOfMeasure ;
                      rdfs:isDefinedBy <https://ontologies.semanticarts.com/o/gistCore> ;
                      skos:definition "Which unit of measure you are using. All measures are expressed in some unit of measure, even if we don't know what it is initially." ;
                      skos:prefLabel "has unit of measure" .


###  https://ontologies.semanticarts.com/gist/hasViableRange
gist:hasViableRange rdf:type owl:ObjectProperty ;
                    rdfs:isDefinedBy <https://ontologies.semanticarts.com/o/gistCore> ;
                    skos:definition "The area over which the sensor can sense (might be a small geospatial area or a specific wire in a circuit)" ;
                    skos:prefLabel "has viable range" .


###  https://ontologies.semanticarts.com/gist/identifies
gist:identifies rdf:type owl:ObjectProperty ;
                owl:inverseOf gist:isIdentifiedBy ;
                rdf:type owl:FunctionalProperty ;
                rdfs:isDefinedBy <https://ontologies.semanticarts.com/o/gistCore> ;
                skos:definition "The thing the identifier refers to." ;
                skos:prefLabel "identifies" .


###  https://ontologies.semanticarts.com/gist/isAbout
gist:isAbout rdf:type owl:ObjectProperty ;
             owl:inverseOf gist:isDescribedIn ;
             rdfs:domain gist:Content ;
             rdfs:isDefinedBy <https://ontologies.semanticarts.com/o/gistCore> ;
             skos:definition "Subject matter of a document." ;
             skos:prefLabel "is about" .


###  https://ontologies.semanticarts.com/gist/isAffectedBy
gist:isAffectedBy rdf:type owl:ObjectProperty ;
                  rdfs:isDefinedBy <https://ontologies.semanticarts.com/o/gistCore> ;
                  skos:definition "Where the effect came from" ;
                  skos:prefLabel "is affected by" .


###  https://ontologies.semanticarts.com/gist/isAllocatedBy
gist:isAllocatedBy rdf:type owl:ObjectProperty ;
                   rdfs:range [ rdf:type owl:Class ;
                                owl:unionOf ( gist:IntellectualProperty
                                              gist:Organization
                                              gist:Person
                                            )
                              ] ;
                   rdfs:isDefinedBy <https://ontologies.semanticarts.com/o/gistCore> ;
                   skos:definition "Connection between an ID and the thing that minted the ID.  It may be a person or organization, or could be an algorithm (next available or random number generator)" ;
                   skos:prefLabel "is allocated by" .


###  https://ontologies.semanticarts.com/gist/isAspectOf
gist:isAspectOf rdf:type owl:ObjectProperty ;
                rdfs:isDefinedBy <https://ontologies.semanticarts.com/o/gistCore> ;
                skos:definition "What this aspect is referring to" ;
                skos:prefLabel "is aspect of" .


###  https://ontologies.semanticarts.com/gist/isBasedOn
gist:isBasedOn rdf:type owl:ObjectProperty ;
               owl:inverseOf gist:isBasisFor ;
               rdfs:isDefinedBy <https://ontologies.semanticarts.com/o/gistCore> ;
               skos:definition "The Object is a foundation for, a starting point for, gave rise to or justifies the Subject" ;
               skos:example "A document is based on a document template. A metric computing the average income of a population is based on the metric for individual income." ;
               skos:prefLabel "is based on" .


###  https://ontologies.semanticarts.com/gist/isBasisFor
gist:isBasisFor rdf:type owl:ObjectProperty ;
                rdfs:isDefinedBy <https://ontologies.semanticarts.com/o/gistCore> ;
                skos:definition "The Subject is a foundation for, a starting point for, gave rise to or justifies the Object" ;
                skos:example "The reason, law, rule, etc. behind an action or decision. The desire to create a community around the data-centric revolution/movement was the basis for initiating the Data-Centric Architecture Summit in 2018. The unabridged dictionary was the basis for the abridged dictionary." ;
                skos:prefLabel "is basis for" .


###  https://ontologies.semanticarts.com/gist/isCategorizedBy
gist:isCategorizedBy rdf:type owl:ObjectProperty ;
                     rdfs:isDefinedBy <https://ontologies.semanticarts.com/o/gistCore> ;
                     skos:definition "Points to a taxonomy item or other less formally defined class." ;
                     skos:prefLabel "is categorized by" ;
                     gist:rangeIncludes gist:Category .


###  https://ontologies.semanticarts.com/gist/isCharacterizedAs
gist:isCharacterizedAs rdf:type owl:ObjectProperty ;
                       rdfs:domain gist:Event ;
                       rdfs:range gist:Behavior ;
                       rdfs:isDefinedBy <https://ontologies.semanticarts.com/o/gistCore> ;
                       skos:definition "A way to categorize a behavior." ;
                       skos:prefLabel "is characterized as" .


###  https://ontologies.semanticarts.com/gist/isConnectedTo
gist:isConnectedTo rdf:type owl:ObjectProperty ,
                            owl:SymmetricProperty ;
                   rdfs:isDefinedBy <https://ontologies.semanticarts.com/o/gistCore> ;
                   skos:definition "A non-owning, non-causal, non-subordinate (i.e., peer-to-peer) relationship." ;
                   skos:prefLabel "is connected to" .


###  https://ontologies.semanticarts.com/gist/isDescribedIn
gist:isDescribedIn rdf:type owl:ObjectProperty ;
                   rdfs:isDefinedBy <https://ontologies.semanticarts.com/o/gistCore> ;
                   skos:definition "Document the subject matter appeared in" ;
                   skos:prefLabel "is described in" .


###  https://ontologies.semanticarts.com/gist/isDirectPartOf
gist:isDirectPartOf rdf:type owl:ObjectProperty ;
                    rdfs:isDefinedBy <https://ontologies.semanticarts.com/o/gistCore> ;
                    skos:definition "The relationship between a part and a whole where the part has independent existence." ;
                    skos:prefLabel "is direct part of" ;
                    skos:scopeNote "It is safest to use this property when there is semantic directness inherent in the relationship, rather than choosing appropriate granularity. For example, a spark plug is a direct part of an engine block; there cannot be any intermediate parts.  Beware of making a directPartOf assertion and then inserting an intermediate part; this will result in making an asserted triple false even though there was no change in the world." ,
                                   "Use this property to directly associate a part with the whole. partOf is the transitive version." .


###  https://ontologies.semanticarts.com/gist/isDirectSubTaskOf
gist:isDirectSubTaskOf rdf:type owl:ObjectProperty ;
                       rdfs:isDefinedBy <https://ontologies.semanticarts.com/o/gistCore> ;
                       skos:definition "Immediate parent task" ;
                       skos:prefLabel "is direct subtask of" .


###  https://ontologies.semanticarts.com/gist/isExpressedIn
gist:isExpressedIn rdf:type owl:ObjectProperty ;
                   rdfs:isDefinedBy <https://ontologies.semanticarts.com/o/gistCore> ;
                   skos:definition "The language something was expressed in" ;
                   skos:prefLabel "is expressed in" .


###  https://ontologies.semanticarts.com/gist/isGeographicallyContainedIn
gist:isGeographicallyContainedIn rdf:type owl:ObjectProperty ;
                                 rdfs:isDefinedBy <https://ontologies.semanticarts.com/o/gistCore> ;
                                 skos:definition "Relates one place to another place that contains the first." ;
                                 skos:prefLabel "is geographically contained in" .


###  https://ontologies.semanticarts.com/gist/isGeographicallyOccupiedBy
gist:isGeographicallyOccupiedBy rdf:type owl:ObjectProperty ;
                                owl:inverseOf gist:occupiesGeographically ;
                                rdfs:isDefinedBy <https://ontologies.semanticarts.com/o/gistCore> ;
                                skos:definition "What is in the location" ;
                                skos:prefLabel "is geographically occupied by" .


###  https://ontologies.semanticarts.com/gist/isGeographicallyPermanentlyOccupiedBy
gist:isGeographicallyPermanentlyOccupiedBy rdf:type owl:ObjectProperty ;
                                           owl:inverseOf gist:occupiesGeographicallyPermanently ;
                                           rdfs:isDefinedBy <https://ontologies.semanticarts.com/o/gistCore> ;
                                           skos:definition "What is in the fixed location" ;
                                           skos:prefLabel "is geographically permanently occupied by" .


###  https://ontologies.semanticarts.com/gist/isGovernedBy
gist:isGovernedBy rdf:type owl:ObjectProperty ;
                  rdfs:isDefinedBy <https://ontologies.semanticarts.com/o/gistCore> ;
                  skos:definition "A reference from the thing being governed to the governor" ;
                  skos:prefLabel "is governed by" .


###  https://ontologies.semanticarts.com/gist/isIdentifiedBy
gist:isIdentifiedBy rdf:type owl:ObjectProperty ,
                             owl:InverseFunctionalProperty ;
                    rdfs:range gist:ID ;
                    rdfs:isDefinedBy <https://ontologies.semanticarts.com/o/gistCore> ;
                    skos:definition "This is like a URI: a thing can have more than one ID, but each of the IDs must refer to a unique thing." ;
                    skos:prefLabel "is identified by" .


###  https://ontologies.semanticarts.com/gist/isMadeUpOf
gist:isMadeUpOf rdf:type owl:ObjectProperty ;
                rdfs:range gist:PhysicalSubstance ;
                rdfs:isDefinedBy <https://ontologies.semanticarts.com/o/gistCore> ;
                skos:definition "Relates something to a substance that it is made up of." ;
                skos:example "The vase is made up of clay. Water is made up of hydrogen and oxygen." ;
                skos:prefLabel "is made up of" .


###  https://ontologies.semanticarts.com/gist/isMemberOf
gist:isMemberOf rdf:type owl:ObjectProperty ;
                rdfs:isDefinedBy <https://ontologies.semanticarts.com/o/gistCore> ;
                skos:definition "What group the member is in" ;
                skos:prefLabel "is member of" .


###  https://ontologies.semanticarts.com/gist/isPartOf
gist:isPartOf rdf:type owl:ObjectProperty ,
                       owl:TransitiveProperty ;
              rdfs:isDefinedBy <https://ontologies.semanticarts.com/o/gistCore> ;
              skos:definition "The transitive version of gist:isDirectPartOf" ;
              skos:prefLabel "is part of" .


###  https://ontologies.semanticarts.com/gist/isRecognizedBy
gist:isRecognizedBy rdf:type owl:ObjectProperty ;
                    owl:inverseOf gist:recognizes ;
                    rdfs:range [ rdf:type owl:Class ;
                                 owl:unionOf ( gist:Organization
                                               gist:Person
                                             )
                               ] ;
                    rdfs:isDefinedBy <https://ontologies.semanticarts.com/o/gistCore> ;
                    skos:definition "The entity that formally acknowledges the existence of, as the State recognizes the existence of a particular company" ;
                    skos:prefLabel "is recognized by" .


###  https://ontologies.semanticarts.com/gist/isRecognizedDirectlyBy
gist:isRecognizedDirectlyBy rdf:type owl:ObjectProperty ;
                            rdfs:subPropertyOf gist:isRecognizedBy ;
                            rdfs:isDefinedBy <https://ontologies.semanticarts.com/o/gistCore> ;
                            skos:definition "The party doing the recognition" ;
                            skos:prefLabel "is recognized directly by" .


###  https://ontologies.semanticarts.com/gist/isRenderedOn
gist:isRenderedOn rdf:type owl:ObjectProperty ;
                  rdfs:isDefinedBy <https://ontologies.semanticarts.com/o/gistCore> ;
                  skos:definition "What media something was rendered On" ;
                  skos:prefLabel "is rendered on" .


###  https://ontologies.semanticarts.com/gist/isSubTaskOf
gist:isSubTaskOf rdf:type owl:ObjectProperty ,
                          owl:TransitiveProperty ;
                 rdfs:isDefinedBy <https://ontologies.semanticarts.com/o/gistCore> ;
                 skos:definition "All the upper tasks this task belongs to" ;
                 skos:prefLabel "is subtask of" .


###  https://ontologies.semanticarts.com/gist/isTriggeredBy
gist:isTriggeredBy rdf:type owl:ObjectProperty ;
                   rdfs:isDefinedBy <https://ontologies.semanticarts.com/o/gistCore> ;
                   skos:definition "General causal relation.  For obligations a property that describes what would happen to trigger the contingent obligation.  In most cases, before the Contingent becomes an Obligation, the triggered by event is a planned event (that is it hasn't happened yet -- if it had happened the contingency would no longer be contingent.  In most cases it will be  a ContingentEvent .  Other uses include controls, processes etc" ;
                   skos:prefLabel "is triggered by" .


###  https://ontologies.semanticarts.com/gist/isUnderJurisdictionOf
gist:isUnderJurisdictionOf rdf:type owl:ObjectProperty ;
                           rdfs:isDefinedBy <https://ontologies.semanticarts.com/o/gistCore> ;
                           skos:definition "Relates a law, contract, etc., to the system of law or government which has the power, right, or authority to interpret and apply it." ;
                           skos:prefLabel "is under jurisdiction of" .


###  https://ontologies.semanticarts.com/gist/links
gist:links rdf:type owl:ObjectProperty ;
           rdfs:isDefinedBy <https://ontologies.semanticarts.com/o/gistCore> ;
           skos:definition "Relates a NetworkLink to a NetworkNode that it connects to another node. Used when the connections are undirected, or the direction is not known." ;
           skos:prefLabel "links" .


###  https://ontologies.semanticarts.com/gist/linksFrom
gist:linksFrom rdf:type owl:ObjectProperty ;
               rdfs:subPropertyOf gist:links ;
               rdfs:isDefinedBy <https://ontologies.semanticarts.com/o/gistCore> ;
               skos:definition "Relates a NetworkLink to its origin NetworkNode. Unlike the superproperty, this represents a directed connection." ;
               skos:prefLabel "links from" .


###  https://ontologies.semanticarts.com/gist/linksTo
gist:linksTo rdf:type owl:ObjectProperty ;
             rdfs:subPropertyOf gist:links ;
             rdfs:isDefinedBy <https://ontologies.semanticarts.com/o/gistCore> ;
             skos:definition "Relates a NetworkLink to its destination NetworkNode. Unlike the superproperty, this represents a directed connection." ;
             skos:prefLabel "links to" .


###  https://ontologies.semanticarts.com/gist/occupiesGeographically
gist:occupiesGeographically rdf:type owl:ObjectProperty ;
                            rdfs:domain [ rdf:type owl:Class ;
                                          owl:unionOf ( gist:PhysicalIdentifiableItem
                                                        gist:PhysicalSubstance
                                                      )
                                        ] ;
                            rdfs:range gist:Place ;
                            rdfs:isDefinedBy <https://ontologies.semanticarts.com/o/gistCore> ;
                            skos:definition "A thing occupies are region" ;
                            skos:prefLabel "occupies geographically" .


###  https://ontologies.semanticarts.com/gist/occupiesGeographicallyPermanently
gist:occupiesGeographicallyPermanently rdf:type owl:ObjectProperty ;
                                       rdfs:subPropertyOf gist:occupiesGeographically ;
                                       rdfs:isDefinedBy <https://ontologies.semanticarts.com/o/gistCore> ;
                                       skos:definition "To be in a fixed position on the earth" ;
                                       skos:prefLabel "occupies geographically permanently" .


###  https://ontologies.semanticarts.com/gist/occursIn
gist:occursIn rdf:type owl:ObjectProperty ;
              rdfs:isDefinedBy <https://ontologies.semanticarts.com/o/gistCore> ;
              skos:definition "The geospatial place where something happened or will happen" ;
              skos:prefLabel "occurs in" .


###  https://ontologies.semanticarts.com/gist/owns
gist:owns rdf:type owl:ObjectProperty ;
          rdfs:domain [ rdf:type owl:Class ;
                        owl:unionOf ( gist:Organization
                                      gist:Person
                                    )
                      ] ;
          rdfs:isDefinedBy <https://ontologies.semanticarts.com/o/gistCore> ;
          skos:definition "Possessing and controlling.  Ultimate form of ownership is the right to destroy.  Long list of potential Range classes" ;
          skos:prefLabel "owns" .


###  https://ontologies.semanticarts.com/gist/precedes
gist:precedes rdf:type owl:ObjectProperty ,
                       owl:TransitiveProperty ;
              rdfs:isDefinedBy <https://ontologies.semanticarts.com/o/gistCore> ;
              skos:definition "A generic ordering relation indicating that the subject comes before the object." ;
              skos:prefLabel "precedes" ;
              skos:scopeNote "The less-than symbol is often used to represent this relation." ,
                             "This is the transitive version of gist:precedesDirectly." ,
                             "Typically this predicate would be used asymmetricallly and irreflexively, but the ontology does not formalize this." .


###  https://ontologies.semanticarts.com/gist/precedesDirectly
gist:precedesDirectly rdf:type owl:ObjectProperty ;
                      rdfs:subPropertyOf gist:precedes ;
                      rdfs:isDefinedBy <https://ontologies.semanticarts.com/o/gistCore> ;
                      skos:definition "A generic ordering relation indicating that the subject comes immediately before the object." ;
                      skos:prefLabel "precedes directly" ;
                      skos:scopeNote "If two items in an ordered collection share the same position, they both directly precede the following element." ,
                                     "It is safest to use this property only when the directness has a semantic correspondence with the world. Only break a direct link by inserting an intermediate item when that change corresponds to a change in the world." ,
                                     "Typically this predicate would be used asymmetricallly and irreflexively, but the ontology does not formalize this." .


###  https://ontologies.semanticarts.com/gist/prevents
gist:prevents rdf:type owl:ObjectProperty ;
              rdfs:domain gist:Intention ;
              rdfs:range gist:Behavior ;
              rdfs:isDefinedBy <https://ontologies.semanticarts.com/o/gistCore> ;
              skos:definition "The intention (say a law) is intended to prevent this kind of behavior (say jay-walking)" ;
              skos:prefLabel "prevents" .


###  https://ontologies.semanticarts.com/gist/produces
gist:produces rdf:type owl:ObjectProperty ;
              rdfs:isDefinedBy <https://ontologies.semanticarts.com/o/gistCore> ;
              skos:definition "The subject creates the object." ;
              skos:example "A task produces a deliverable." ;
              skos:prefLabel "produces" .


###  https://ontologies.semanticarts.com/gist/providesOrderFor
gist:providesOrderFor rdf:type owl:ObjectProperty ,
                               owl:FunctionalProperty ;
                      rdfs:domain gist:OrderedMember ;
                      rdfs:isDefinedBy <https://ontologies.semanticarts.com/o/gistCore> ;
                      skos:definition "Links a member of an ordered collection to the real-world item it represents in that collection." ;
                      skos:prefLabel "provides order for" .


###  https://ontologies.semanticarts.com/gist/recognizes
gist:recognizes rdf:type owl:ObjectProperty ;
                rdfs:isDefinedBy <https://ontologies.semanticarts.com/o/gistCore> ;
                skos:definition "Recognizes" ;
                skos:prefLabel "recognizes" .


###  https://ontologies.semanticarts.com/gist/requires
gist:requires rdf:type owl:ObjectProperty ;
              rdfs:isDefinedBy <https://ontologies.semanticarts.com/o/gistCore> ;
              skos:definition "The subject needs the object or makes it necessary, mandatory, or compulsory." ;
              skos:example "Humans require air; solar power requires sunshine." ;
              skos:prefLabel "requires" ;
              skos:scopeNote """This predicate is defined generally enough to encompass a few different meanings of the English word 'requires': 
		
		1. To need something or to make something necessary.
		2. To order or demand something, or to order someone to do something, especially because of a rule or law.
		3. To make it officially necessary for someone to do something.
	
	Implementations requiring a more specific meaning should define subproperties.""" .


###  https://ontologies.semanticarts.com/gist/respondsTo
gist:respondsTo rdf:type owl:ObjectProperty ;
                rdfs:isDefinedBy <https://ontologies.semanticarts.com/o/gistCore> ;
                skos:definition "The set of sensors that a controller is attached to" ;
                skos:prefLabel "responds to" .


###  https://ontologies.semanticarts.com/gist/usesTimeZoneStandard
gist:usesTimeZoneStandard rdf:type owl:ObjectProperty ;
                          rdfs:range gist:TimeZoneStandard ;
                          rdfs:isDefinedBy <https://ontologies.semanticarts.com/o/gistCore> ;
                          skos:definition "The time zone, including daylight savings time adjustment, of an event or other object that can have a date and time." ;
                          skos:example "EST (Eastern Standard Time), PST (Pacific Daylight Time)." ;
                          skos:prefLabel "uses time zone standard" .


###  https://ontology.architmitra.org/archimodel/accessedBy
<https://ontology.architmitra.org/archimodel/accessedBy> rdf:type owl:ObjectProperty ;
                                                         owl:inverseOf <https://ontology.architmitra.org/archimodel/accesses> ;
                                                         skos:definition "The access relationship represents the ability of behavior and active structure elements to observe or act upon passive structure elements." ;
                                                         skos:prefLabel "accessed by" .


###  https://ontology.architmitra.org/archimodel/accesses
<https://ontology.architmitra.org/archimodel/accesses> rdf:type owl:ObjectProperty ;
                                                       skos:definition "The access relationship represents the ability of behavior and active structure elements to observe or act upon passive structure elements." ;
                                                       skos:prefLabel "accesses" .


###  https://ontology.architmitra.org/archimodel/addresses
<https://ontology.architmitra.org/archimodel/addresses> rdf:type owl:ObjectProperty ;
                                                        skos:prefLabel "addresses" .


###  https://ontology.architmitra.org/archimodel/aggregatedIn
<https://ontology.architmitra.org/archimodel/aggregatedIn> rdf:type owl:ObjectProperty ;
                                                           owl:inverseOf <https://ontology.architmitra.org/archimodel/aggregates> ;
                                                           skos:prefLabel "aggregated in" .


###  https://ontology.architmitra.org/archimodel/aggregates
<https://ontology.architmitra.org/archimodel/aggregates> rdf:type owl:ObjectProperty ,
                                                                  owl:TransitiveProperty ;
                                                         skos:definition "The aggregation relationship represents that an element combines one or more other concepts." ;
                                                         skos:prefLabel "aggregates" .


###  https://ontology.architmitra.org/archimodel/assignedTo
<https://ontology.architmitra.org/archimodel/assignedTo> rdf:type owl:ObjectProperty ;
                                                         owl:inverseOf <https://ontology.architmitra.org/archimodel/hasAssigned> ;
                                                         rdf:type owl:TransitiveProperty ;
                                                         skos:prefLabel "assigned to" .


###  https://ontology.architmitra.org/archimodel/associatedFrom
<https://ontology.architmitra.org/archimodel/associatedFrom> rdf:type owl:ObjectProperty ;
                                                             owl:inverseOf <https://ontology.architmitra.org/archimodel/associatedTo> ;
                                                             skos:prefLabel "associated from" .


###  https://ontology.architmitra.org/archimodel/associatedTo
<https://ontology.architmitra.org/archimodel/associatedTo> rdf:type owl:ObjectProperty ;
                                                           skos:definition "An association relationship represents an unspecified relationship, or one that is not represented by another ArchiMate relationship." ;
                                                           skos:prefLabel "associated to" .


###  https://ontology.architmitra.org/archimodel/associatedWith
<https://ontology.architmitra.org/archimodel/associatedWith> rdf:type owl:ObjectProperty ;
                                                             skos:prefLabel "associated with" .


###  https://ontology.architmitra.org/archimodel/composedIn
<https://ontology.architmitra.org/archimodel/composedIn> rdf:type owl:ObjectProperty ;
                                                         owl:inverseOf <https://ontology.architmitra.org/archimodel/composedOf> ;
                                                         skos:prefLabel "composed in" .


###  https://ontology.architmitra.org/archimodel/composedOf
<https://ontology.architmitra.org/archimodel/composedOf> rdf:type owl:ObjectProperty ,
                                                                  owl:TransitiveProperty ;
                                                         skos:definition "Represents that an element consists of one or more other concepts. A composition relationship is always allowed between two instances of the same element type." ;
                                                         skos:prefLabel "composed of" .


###  https://ontology.architmitra.org/archimodel/dependsOn
<https://ontology.architmitra.org/archimodel/dependsOn> rdf:type owl:ObjectProperty ;
                                                        skos:prefLabel "depends on" .


###  https://ontology.architmitra.org/archimodel/exhibits
<https://ontology.architmitra.org/archimodel/exhibits> rdf:type owl:ObjectProperty ;
                                                       skos:prefLabel "exhibits" .


###  https://ontology.architmitra.org/archimodel/exposes
<https://ontology.architmitra.org/archimodel/exposes> rdf:type owl:ObjectProperty ;
                                                      skos:prefLabel "exposes" .


###  https://ontology.architmitra.org/archimodel/expresses
<https://ontology.architmitra.org/archimodel/expresses> rdf:type owl:ObjectProperty ;
                                                        skos:prefLabel "expresses" .


###  https://ontology.architmitra.org/archimodel/flowsFrom
<https://ontology.architmitra.org/archimodel/flowsFrom> rdf:type owl:ObjectProperty ;
                                                        owl:inverseOf <https://ontology.architmitra.org/archimodel/flowsTo> ;
                                                        skos:prefLabel "flows from" .


###  https://ontology.architmitra.org/archimodel/flowsTo
<https://ontology.architmitra.org/archimodel/flowsTo> rdf:type owl:ObjectProperty ;
                                                      skos:prefLabel "flows to" .


###  https://ontology.architmitra.org/archimodel/frames
<https://ontology.architmitra.org/archimodel/frames> rdf:type owl:ObjectProperty ;
                                                     skos:prefLabel "frames" .


###  https://ontology.architmitra.org/archimodel/governs
<https://ontology.architmitra.org/archimodel/governs> rdf:type owl:ObjectProperty ;
                                                      skos:prefLabel "governs" .


###  https://ontology.architmitra.org/archimodel/hasAssigned
<https://ontology.architmitra.org/archimodel/hasAssigned> rdf:type owl:ObjectProperty ;
                                                          skos:prefLabel "has assigned" .


###  https://ontology.architmitra.org/archimodel/hasConcern
<https://ontology.architmitra.org/archimodel/hasConcern> rdf:type owl:ObjectProperty ;
                                                         skos:prefLabel "has concern" .


###  https://ontology.architmitra.org/archimodel/hasInterestIn
<https://ontology.architmitra.org/archimodel/hasInterestIn> rdf:type owl:ObjectProperty ;
                                                            skos:prefLabel "has interest in" .


###  https://ontology.architmitra.org/archimodel/influencedBy
<https://ontology.architmitra.org/archimodel/influencedBy> rdf:type owl:ObjectProperty ;
                                                           owl:inverseOf <https://ontology.architmitra.org/archimodel/influences> ;
                                                           skos:prefLabel "influenced by" .


###  https://ontology.architmitra.org/archimodel/influences
<https://ontology.architmitra.org/archimodel/influences> rdf:type owl:ObjectProperty ;
                                                         skos:prefLabel "influences" .


###  https://ontology.architmitra.org/archimodel/justifies
<https://ontology.architmitra.org/archimodel/justifies> rdf:type owl:ObjectProperty .


###  https://ontology.architmitra.org/archimodel/pertainsTo
<https://ontology.architmitra.org/archimodel/pertainsTo> rdf:type owl:ObjectProperty ;
                                                         skos:prefLabel "pertains to" .


###  https://ontology.architmitra.org/archimodel/raises
<https://ontology.architmitra.org/archimodel/raises> rdf:type owl:ObjectProperty ;
                                                     skos:prefLabel "raises" .


###  https://ontology.architmitra.org/archimodel/realizedBy
<https://ontology.architmitra.org/archimodel/realizedBy> rdf:type owl:ObjectProperty ;
                                                         owl:inverseOf <https://ontology.architmitra.org/archimodel/realizes> ;
                                                         skos:definition "The realization relationship represents that an entity plays a critical role in the creation, achievement, sustenance, or operation of a more abstract entity." ;
                                                         skos:prefLabel "realized by" .


###  https://ontology.architmitra.org/archimodel/realizes
<https://ontology.architmitra.org/archimodel/realizes> rdf:type owl:ObjectProperty ,
                                                                owl:TransitiveProperty ;
                                                       skos:definition "The realization relationship represents that an entity plays a critical role in the creation, achievement, sustenance, or operation of a more abstract entity." ;
                                                       skos:prefLabel "realizes" .


###  https://ontology.architmitra.org/archimodel/servedBy
<https://ontology.architmitra.org/archimodel/servedBy> rdf:type owl:ObjectProperty ;
                                                       owl:inverseOf <https://ontology.architmitra.org/archimodel/serves> ;
                                                       skos:prefLabel "served by" .


###  https://ontology.architmitra.org/archimodel/serves
<https://ontology.architmitra.org/archimodel/serves> rdf:type owl:ObjectProperty ;
                                                     skos:definition "The serving relationship represents that an element provides its functionality to another element." ;
                                                     skos:prefLabel "serves" .


###  https://ontology.architmitra.org/archimodel/situatedIn
<https://ontology.architmitra.org/archimodel/situatedIn> rdf:type owl:ObjectProperty ;
                                                         skos:prefLabel "situated In" .


###  https://ontology.architmitra.org/archimodel/specializedBy
<https://ontology.architmitra.org/archimodel/specializedBy> rdf:type owl:ObjectProperty ;
                                                            owl:inverseOf <https://ontology.architmitra.org/archimodel/specializes> ;
                                                            skos:prefLabel "specialized by" .


###  https://ontology.architmitra.org/archimodel/specializes
<https://ontology.architmitra.org/archimodel/specializes> rdf:type owl:ObjectProperty ,
                                                                   owl:TransitiveProperty .


###  https://ontology.architmitra.org/archimodel/triggeredBy
<https://ontology.architmitra.org/archimodel/triggeredBy> rdf:type owl:ObjectProperty ;
                                                          skos:prefLabel "triggered by" .


###  https://ontology.architmitra.org/archimodel/triggers
<https://ontology.architmitra.org/archimodel/triggers> rdf:type owl:ObjectProperty ;
                                                       skos:prefLabel "triggers" .


#################################################################
#    Data properties
#################################################################

###  https://ontologies.semanticarts.com/gist/actualEndDate
gist:actualEndDate rdf:type owl:DatatypeProperty ;
                   rdfs:subPropertyOf gist:actualEndDateTime ;
                   rdfs:range xsd:dateTime ;
                   rdfs:isDefinedBy <https://ontologies.semanticarts.com/o/gistCore> ;
                   skos:definition "The actual date that something ended, with precision of one day." ;
                   skos:example "'2021-06-01T00:00:00-6:00'^^xsd:dateTime" ;
                   skos:prefLabel "actual end date" ;
                   skos:scopeNote "Used for things where the precision of a date is sufficient, such as most projects, tasks, and the like. Recommended usage is to zero out the hours through microseconds to avoid spurious precision." .


###  https://ontologies.semanticarts.com/gist/actualEndDateTime
gist:actualEndDateTime rdf:type owl:DatatypeProperty ;
                       rdfs:subPropertyOf gist:endDateTime ;
                       rdfs:range xsd:dateTime ;
                       rdfs:isDefinedBy <https://ontologies.semanticarts.com/o/gistCore> ;
                       skos:definition "The actual date and time that something ended, with no implied precision." ;
                       skos:prefLabel "actual end date time" ;
                       skos:scopeNote "This is an abstraction over the various precisions of actual end time, and is not expected to be asserted directly. Values with different precisions can be compared since they all have the same format." .


###  https://ontologies.semanticarts.com/gist/actualEndMicrosecond
gist:actualEndMicrosecond rdf:type owl:DatatypeProperty ;
                          rdfs:subPropertyOf gist:actualEndDateTime ;
                          rdfs:range xsd:dateTime ;
                          rdfs:isDefinedBy <https://ontologies.semanticarts.com/o/gistCore> ;
                          skos:definition "The actual time that something ended, expressed as a system time used for timestamps." ;
                          skos:example "'2021-06-01T08:03:27.12324-6:00'^^xsd:dateTime" ;
                          skos:prefLabel "actual end microsecond" ;
                          skos:scopeNote "A system time will be as precise as the system can supply, typically at least milliseconds, sometimes microseconds. The convention for timestamps, such as recording a transaction, is to specify just the end point; the start time is rarely needed." .


###  https://ontologies.semanticarts.com/gist/actualEndMinute
gist:actualEndMinute rdf:type owl:DatatypeProperty ;
                     rdfs:subPropertyOf gist:actualEndDateTime ;
                     rdfs:range xsd:dateTime ;
                     rdfs:isDefinedBy <https://ontologies.semanticarts.com/o/gistCore> ;
                     skos:definition "The actual date and time that something ended, with precision of one minute." ;
                     skos:example "'2021-06-01T08:32:00-6:00'^^xsd:dateTime" ;
                     skos:prefLabel "actual end minute" ;
                     skos:scopeNote "Used for things like meetings and time card entries, where the hour and minute are important. Recommended usage is to zero out the seconds and microseconds to avoid spurious precision." .


###  https://ontologies.semanticarts.com/gist/actualEndYear
gist:actualEndYear rdf:type owl:DatatypeProperty ;
                   rdfs:subPropertyOf gist:actualEndDateTime ;
                   rdfs:range xsd:dateTime ;
                   rdfs:isDefinedBy <https://ontologies.semanticarts.com/o/gistCore> ;
                   skos:definition "The actual date that something ended, with precision of one year." ;
                   skos:example "'2021-01-01T00:00:00-6:00'^^xsd:dateTime" ,
                                "The tenure of the previous chairman of the board ended in 2021." ;
                   skos:prefLabel "actual end year" ;
                   skos:scopeNote "Used for things where the precision of a year is sufficient. Recommended usage is to zero out the hours through microseconds to avoid spurious precision. Note that it is not valid to zero out months and days, so arbitrary values must be included." .


###  https://ontologies.semanticarts.com/gist/actualStartDate
gist:actualStartDate rdf:type owl:DatatypeProperty ;
                     rdfs:subPropertyOf gist:actualStartDateTime ;
                     rdfs:range xsd:dateTime ;
                     rdfs:isDefinedBy <https://ontologies.semanticarts.com/o/gistCore> ;
                     skos:definition "The actual date that something started, with precision of one day." ;
                     skos:example "'2021-06-01T00:00:00-6:00'^^xsd:dateTime" ;
                     skos:prefLabel "actual start date" ;
                     skos:scopeNote "Used for things where the precision of a date is sufficient, such as most projects, tasks, and the like. Recommended usage is to zero out the hours through microseconds to avoid spurious precision." .


###  https://ontologies.semanticarts.com/gist/actualStartDateTime
gist:actualStartDateTime rdf:type owl:DatatypeProperty ;
                         rdfs:subPropertyOf gist:startDateTime ;
                         rdfs:range xsd:dateTime ;
                         rdfs:isDefinedBy <https://ontologies.semanticarts.com/o/gistCore> ;
                         skos:definition "The actual date and time that something started, with no implied precision." ;
                         skos:prefLabel "actual start date time" ;
                         skos:scopeNote "This is an abstraction over the various precisions of actual start time, and is not expected to be asserted directly. Values with different precisions can be compared since they all have the same format." .


###  https://ontologies.semanticarts.com/gist/actualStartMicrosecond
gist:actualStartMicrosecond rdf:type owl:DatatypeProperty ;
                            rdfs:subPropertyOf gist:actualStartDateTime ;
                            rdfs:range xsd:dateTime ;
                            rdfs:isDefinedBy <https://ontologies.semanticarts.com/o/gistCore> ;
                            skos:definition "The actual time that something started, expressed as a system time used for timestamps." ;
                            skos:example "'2021-06-01T08:03:27.12324-6:00'^^xsd:dateTime" ;
                            skos:prefLabel "actual start microsecond" ;
                            skos:scopeNote "A system time will be as precise as the system can supply, typically at least milliseconds, sometimes microseconds. The convention for timestamps, such as recording a transaction, is to specify just the end point; the start time is rarely needed. This property is defined for the cases when you do need to capture the runtime of a system process, and is then used in conjunction with gist:actualEndMicrosecond." .


###  https://ontologies.semanticarts.com/gist/actualStartMinute
gist:actualStartMinute rdf:type owl:DatatypeProperty ;
                       rdfs:subPropertyOf gist:actualStartDateTime ;
                       rdfs:range xsd:dateTime ;
                       rdfs:isDefinedBy <https://ontologies.semanticarts.com/o/gistCore> ;
                       skos:definition "The actual date and time that something started, with precision of one minute." ;
                       skos:example "'2021-06-01T08:32:00-6:00'^^xsd:dateTime" ;
                       skos:prefLabel "actual start minute" ;
                       skos:scopeNote "Used for things like meetings and time card entries, where the hour and minute are important. Recommended usage is to zero out the seconds and microseconds to avoid spurious precision." .


###  https://ontologies.semanticarts.com/gist/actualStartYear
gist:actualStartYear rdf:type owl:DatatypeProperty ;
                     rdfs:subPropertyOf gist:actualStartDateTime ;
                     rdfs:range xsd:dateTime ;
                     rdfs:isDefinedBy <https://ontologies.semanticarts.com/o/gistCore> ;
                     skos:definition "The actual date that something started, with precision of one year." ;
                     skos:example "'2021-01-01T00:00:00-6:00'^^xsd:dateTime" ,
                                  "The tenure of the current chairman of the board began in 2021." ;
                     skos:prefLabel "actual start year" ;
                     skos:scopeNote "Used for things where the precision of a year is sufficient. Recommended usage is to zero out the hours through microseconds to avoid spurious precision. Note that it is not valid to zero out months and days, so arbitrary values must be included." .


###  https://ontologies.semanticarts.com/gist/atDateTime
gist:atDateTime rdf:type owl:DatatypeProperty ;
                rdfs:range xsd:dateTime ;
                rdfs:isDefinedBy <https://ontologies.semanticarts.com/o/gistCore> ;
                skos:definition "The date and time at which something did or will occur, with variants for precision, start and end, and actual vs. planned." ;
                skos:prefLabel "at date time" ;
                skos:scopeNote """This is the top level property for asserting time, and is not expected to be asserted directly.

The subproperties allow the ontologist to do three things:
1) Distinguish start and end times.
2) Indicate whether a time is planned or actual. This is useful for everything from project management to calendar appointments and the like. It is also useful for date effectivities; i.e., something valid up to a planned date).
3) Distinguish varying levels of precision; sort of a simple version of the Allen functions.  

All datetimes are of the same format: '2021-06-01T08:03:27.12324-6:00'^^xsd:dateTime. This is compatible with and a subset of ISO 8601.

Time zone offset, such as -6:00 (of which there are a few dozen) is recognized in the date itself, as shown. The actual time zone standard (of which there are 131) may optionally be attached to the event or other object itself; see property gist:usesTimeZoneStandard.

There will be many historical dates that do not have a time zone offset (e.g., Lincoln's birthday, as well as about 75% of all legacy systems), and in that case the offset can be omitted. 

The conventions for precision that are repeated in each property name are as follows:
	- *DateTime is an abstraction over the various precisions of its subproperties.
	- *Date refers to a calendar date (e.g., birthdays and invoice dates) and is assumed to have precision of one day. Time zone offset is allowed.
	- *Minute refers to clock time; e.g., a meeting will start at 9:15 with a timezone offset. Precision is assumed to have precision of one minute.
	- *Microsecond refers to system time, and it will be as precise as the system can supply; typically at least milliseconds, sometime microseconds.

""" .


###  https://ontologies.semanticarts.com/gist/birthDate
gist:birthDate rdf:type owl:DatatypeProperty ;
               rdfs:subPropertyOf gist:startDateTime ;
               rdfs:range xsd:dateTime ;
               rdfs:isDefinedBy <https://ontologies.semanticarts.com/o/gistCore> ;
               skos:definition "The date some living thing was or will be born, with precision of one day." ;
               skos:example "'2021-06-01T00:00:00-6:00'^^xsd:dateTime" ;
               skos:prefLabel "birth date" ;
               skos:scopeNote "This is a subproperty of gist:startDateTime rather than gist:actualStartDate because some living things have yet to be born. This property refers to a calendar date and is assumed to precision of one day (time zone offset is allowed). It is recommended to zero out the hours through microseconds to avoid spurious precision. Implementations requiring a birthdate to the minute can define a subproperty." .


###  https://ontologies.semanticarts.com/gist/containedText
gist:containedText rdf:type owl:DatatypeProperty ;
                   rdfs:range xsd:string ;
                   rdfs:isDefinedBy <https://ontologies.semanticarts.com/o/gistCore> ;
                   skos:definition "Links to the string corresponding to Text" ;
                   skos:prefLabel "contained text" .


###  https://ontologies.semanticarts.com/gist/conversionFactor
gist:conversionFactor rdf:type owl:DatatypeProperty ;
                      rdfs:domain gist:UnitOfMeasure ;
                      rdfs:range xsd:double ;
                      rdfs:isDefinedBy <https://ontologies.semanticarts.com/o/gistCore> ;
                      skos:definition "The conversion factor used to convert a unit to its standard (i.e., coherent) unit (which could be a base unit.)" ;
                      skos:example "A value expressed in inches is multiplied by a conversion factor of 0.0254 to express the value in the base unit, meter." ,
                                   "An area expressed as 7 square kilometers is multiplied by a conversion factor of one million which results in 7 million square meters." ;
                      skos:prefLabel "conversion factor" ;
                      skos:scopeNote "Sometimes this property must be used in conjunction with conversionOffset. Kelvin =  (Degrees F - conversionOffset) * conversionFactor. Or K = (F-(-469.67)) * (5/9)." .


###  https://ontologies.semanticarts.com/gist/conversionOffset
gist:conversionOffset rdf:type owl:DatatypeProperty ;
                      rdfs:domain gist:UnitOfMeasure ;
                      rdfs:range xsd:double ;
                      rdfs:isDefinedBy <https://ontologies.semanticarts.com/o/gistCore> ;
                      skos:definition "Add this number to get to the zero point.  On the Celsius scale, the conversionOffset is -273.15 degrees C. On the Fahrenheit scale it is -459.67 degrees.  Is equal to 0 when the unit has the same zero point as the base unit. e.g. inch, meter." ;
                      skos:prefLabel "conversion offset" .


###  https://ontologies.semanticarts.com/gist/deathDate
gist:deathDate rdf:type owl:DatatypeProperty ;
               rdfs:subPropertyOf gist:actualEndDate ;
               rdfs:range xsd:dateTime ;
               rdfs:isDefinedBy <https://ontologies.semanticarts.com/o/gistCore> ;
               skos:definition "The date some living thing died." ;
               skos:example "'2021-06-01T00:00:00-6:00'^^xsd:dateTime" ;
               skos:prefLabel "death date" ;
               skos:scopeNote "Refers to a calendar date and is assumed to have precision of one day (time zone offset is allowed). Recommended usage is to zero out the hours through microseconds to avoid spurious precision. Implementations requiring a death date to the minute can define a subproperty." .


###  https://ontologies.semanticarts.com/gist/description
gist:description rdf:type owl:DatatypeProperty ;
                 rdfs:isDefinedBy <https://ontologies.semanticarts.com/o/gistCore> ;
                 skos:definition "A statement about someone or something's attributes or characteristics." ;
                 skos:example "The Empire State Building is a 102-story Art Deco skyscraper in Midtown Manhattan in New York City, United States. It was designed by Shreve, Lamb & Harmon and built from 1930 to 1931." ;
                 skos:prefLabel "description" ;
                 skos:scopeNote "This property is used to provide a description of an instance entity in greater detail than a label." .


###  https://ontologies.semanticarts.com/gist/encryptedText
gist:encryptedText rdf:type owl:DatatypeProperty ;
                   rdfs:subPropertyOf gist:containedText ;
                   rdfs:range xsd:string ;
                   rdfs:isDefinedBy <https://ontologies.semanticarts.com/o/gistCore> ;
                   skos:definition "Links to the string corresponding to EncryptedText" ;
                   skos:prefLabel "encrypted text" .


###  https://ontologies.semanticarts.com/gist/endDateTime
gist:endDateTime rdf:type owl:DatatypeProperty ;
                 rdfs:subPropertyOf gist:atDateTime ;
                 rdfs:range xsd:dateTime ;
                 rdfs:isDefinedBy <https://ontologies.semanticarts.com/o/gistCore> ;
                 skos:definition "The date and time that something ended." ;
                 skos:prefLabel "end date time" ;
                 skos:scopeNote "This is an abstraction over the various precisions of end time, and is not expected to be asserted directly. Values with different precisions can be compared since they all have the same format." ,
                                "We have looked at some extreme edge cases (e.g., did this meeting end before or after the trade was posted?) and we couldn't find any use case that required special processing. Those who have such use cases can implement them (and feel free to let us know)." .


###  https://ontologies.semanticarts.com/gist/isRecordedAt
gist:isRecordedAt rdf:type owl:DatatypeProperty ;
                  rdfs:subPropertyOf gist:atDateTime ;
                  rdfs:isDefinedBy <https://ontologies.semanticarts.com/o/gistCore> ;
                  skos:definition "Date that something was posted, not necessarily the date it occurred. Must be after the date of occurrence, but could be before or after the planned date. (Unusual, but I could record today that I expected to be paid last week.)" ;
                  skos:prefLabel "is recorded at" ;
                  skos:scopeNote "Precision may vary according to context." .


###  https://ontologies.semanticarts.com/gist/latitude
gist:latitude rdf:type owl:DatatypeProperty ;
              rdfs:domain gist:GeoPoint ;
              rdfs:range xsd:double ;
              rdfs:isDefinedBy <https://ontologies.semanticarts.com/o/gistCore> ;
              skos:definition "Degrees above or below equator" ;
              skos:prefLabel "latitude" .


###  https://ontologies.semanticarts.com/gist/longitude
gist:longitude rdf:type owl:DatatypeProperty ;
               rdfs:domain gist:GeoPoint ;
               rdfs:range xsd:double ;
               rdfs:isDefinedBy <https://ontologies.semanticarts.com/o/gistCore> ;
               skos:definition "Degrees from GM" ;
               skos:prefLabel "longitude" .


###  https://ontologies.semanticarts.com/gist/name
gist:name rdf:type owl:DatatypeProperty ;
          rdfs:range xsd:string ;
          rdfs:isDefinedBy <https://ontologies.semanticarts.com/o/gistCore> ;
          skos:definition "Relates an individual to (one of) its name(s)." ;
          skos:prefLabel "name" .


###  https://ontologies.semanticarts.com/gist/numericValue
gist:numericValue rdf:type owl:DatatypeProperty ;
                  rdfs:domain gist:Magnitude ;
                  rdfs:range [ rdf:type rdfs:Datatype ;
                               owl:unionOf ( xsd:byte
                                             xsd:decimal
                                             xsd:double
                                             xsd:float
                                             xsd:int
                                             xsd:integer
                                             xsd:long
                                             xsd:negativeInteger
                                             xsd:nonNegativeInteger
                                             xsd:nonPositiveInteger
                                             xsd:positiveInteger
                                             xsd:short
                                             xsd:unsignedByte
                                             xsd:unsignedInt
                                             xsd:unsignedLong
                                             xsd:unsignedShort
                                             owl:rational
                                             owl:real
                                           )
                             ] ;
                  rdfs:isDefinedBy <https://ontologies.semanticarts.com/o/gistCore> ;
                  skos:definition "The actual value of a magnitude." ;
                  skos:prefLabel "numeric value" .


###  https://ontologies.semanticarts.com/gist/plannedEndDate
gist:plannedEndDate rdf:type owl:DatatypeProperty ;
                    rdfs:subPropertyOf gist:plannedEndDateTime ;
                    rdfs:range xsd:dateTime ;
                    rdfs:isDefinedBy <https://ontologies.semanticarts.com/o/gistCore> ;
                    skos:definition "The date that something is or was planned to end, with precision of one day." ;
                    skos:example "'2021-06-01T00:00:00-6:00'^^xsd:dateTime" ;
                    skos:prefLabel "planned end date" ;
                    skos:scopeNote "Used for anything with a planned end date, such as when a lease will expire, when an offer is no longer available, etc. Typically a planned date is in the future when first captured, but when tasks run late, we leave the plan where it was and compare it to the actual. Recommended usage is to zero out the hours through microseconds to avoid spurious precision." .


###  https://ontologies.semanticarts.com/gist/plannedEndDateTime
gist:plannedEndDateTime rdf:type owl:DatatypeProperty ;
                        rdfs:subPropertyOf gist:endDateTime ;
                        rdfs:range xsd:dateTime ;
                        rdfs:isDefinedBy <https://ontologies.semanticarts.com/o/gistCore> ;
                        skos:definition "The date that something is or was planned to end, with no implied precision." ;
                        skos:prefLabel "planned end date time" ;
                        skos:scopeNote "This is an abstraction over the various precisions of planned end time, and is not expected to be asserted directly.  Values with different precisions can be compared since they all have the same format." ,
                                       "This property, unlike gist:actualEndDateTime, does not have a subproperty for microsecond precision, because planned times typically are not expressed at that level of granularity. Typically a planned date is in the future when first captured, but when tasks run late, we leave the plan where it was and compare it to the actual." .


###  https://ontologies.semanticarts.com/gist/plannedEndMinute
gist:plannedEndMinute rdf:type owl:DatatypeProperty ;
                      rdfs:subPropertyOf gist:plannedEndDateTime ;
                      rdfs:range xsd:dateTime ;
                      rdfs:isDefinedBy <https://ontologies.semanticarts.com/o/gistCore> ;
                      skos:definition "The date and time that something is or was planned to end, with precision of one minute." ;
                      skos:example "'2021-06-01T08:32:00-6:00'^^xsd:dateTime" ;
                      skos:prefLabel "planned end minute" ;
                      skos:scopeNote "Used for things like meetings and time card entries, where the hour and minute are important. Recommended usage is to zero out the seconds and microseconds to avoid spurious precision.Typically a planned date is in the future when first captured, but when tasks run late, we leave the plan where it was and compare it to the actual." .


###  https://ontologies.semanticarts.com/gist/plannedEndYear
gist:plannedEndYear rdf:type owl:DatatypeProperty ;
                    rdfs:subPropertyOf gist:plannedEndDateTime ;
                    rdfs:range xsd:dateTime ;
                    rdfs:isDefinedBy <https://ontologies.semanticarts.com/o/gistCore> ;
                    skos:definition "The date that something is or was planned to end, with precision of one year." ;
                    skos:example "'2021-01-01T00:00:00-6:00'^^xsd:dateTime" ,
                                 "The automobile manufacturer announced that it will stop producing gas-powered vehicles in 2035." ;
                    skos:prefLabel "planned end year" ;
                    skos:scopeNote "Used for anything with a planned end date where precision of one year is sufficient. Typically a planned date is in the future when first captured, but when tasks run late, we leave the plan where it was and compare it to the actual. Recommended usage is to zero out the hours through microseconds to avoid spurious precision. Note that it is not valid to zero out months and days, so arbitrary values must be included." .


###  https://ontologies.semanticarts.com/gist/plannedStartDate
gist:plannedStartDate rdf:type owl:DatatypeProperty ;
                      rdfs:subPropertyOf gist:plannedStartDateTime ;
                      rdfs:range xsd:dateTime ;
                      rdfs:isDefinedBy <https://ontologies.semanticarts.com/o/gistCore> ;
                      skos:definition "The date that something is or was planned to start, with precision of one day." ;
                      skos:example "'2021-06-01T00:00:00-6:00'^^xsd:dateTime" ;
                      skos:prefLabel "planned start date" ;
                      skos:scopeNote "Used for anything with a planned start date, such as when a lease will start, when a configuration becomes available, etc. Typically a planned date is in the future when first captured, but when tasks run late, we leave the plan where it was and compare it to the actual. Recommended usage is to zero out the hours through microseconds to avoid spurious precision." .


###  https://ontologies.semanticarts.com/gist/plannedStartDateTime
gist:plannedStartDateTime rdf:type owl:DatatypeProperty ;
                          rdfs:subPropertyOf gist:startDateTime ;
                          rdfs:range xsd:dateTime ;
                          rdfs:isDefinedBy <https://ontologies.semanticarts.com/o/gistCore> ;
                          skos:definition "The date and time that something is or was planned to start, with no implied precision." ;
                          skos:prefLabel "planned start date time" ;
                          skos:scopeNote "This is an abstraction over the various precisions of planned start time, and is not expected to be asserted directly. Values with different precisions can be compared since they all have the same format." ,
                                         "This property, unlike gist:actualStartDateTime, does not have a subproperty for microsecond precision, because planned times typically are not expressed at that level of granularity. Typically a planned date is in the future when first captured, but when tasks run late, we leave the plan where it was and compare it to the actual." .


###  https://ontologies.semanticarts.com/gist/plannedStartMinute
gist:plannedStartMinute rdf:type owl:DatatypeProperty ;
                        rdfs:subPropertyOf gist:plannedStartDateTime ;
                        rdfs:range xsd:dateTime ;
                        rdfs:isDefinedBy <https://ontologies.semanticarts.com/o/gistCore> ;
                        skos:definition "The date and time that something is or was planned to start, with precision of one minute." ;
                        skos:example "'2021-06-01T08:32:00-6:00'^^xsd:dateTime" ;
                        skos:prefLabel "planned start minute" ;
                        skos:scopeNote "Used for things like meetings and time card entries, where the hour and minute are important. Typically a planned date is in the future when first captured, but when tasks run late, we leave the plan where it was and compare it to the actual. Recommended usage is to zero out the seconds and microseconds to avoid spurious precision." .


###  https://ontologies.semanticarts.com/gist/plannedStartYear
gist:plannedStartYear rdf:type owl:DatatypeProperty ;
                      rdfs:subPropertyOf gist:plannedStartDateTime ;
                      rdfs:range xsd:dateTime ;
                      rdfs:isDefinedBy <https://ontologies.semanticarts.com/o/gistCore> ;
                      skos:definition "The date that something is or was planned to start, with precision of one year." ;
                      skos:example "'2021-01-01T00:00:00-6:00'^^xsd:dateTime" ,
                                   "The automobile manufacturer announced that its full line-up will include only electric cars starting in 2035." ;
                      skos:prefLabel "planned start year" ;
                      skos:scopeNote "Used for anything with a planned start date where precision of one year is sufficient. Typically a planned date is in the future when first captured, but when tasks run late, we leave the plan where it was and compare it to the actual. Recommended usage is to zero out the hours through microseconds to avoid spurious precision. Note that it is not valid to zero out months and days, so arbitrary values must be included." .


###  https://ontologies.semanticarts.com/gist/sequence
gist:sequence rdf:type owl:DatatypeProperty ;
              rdfs:range xsd:integer ;
              rdfs:isDefinedBy <https://ontologies.semanticarts.com/o/gistCore> ;
              skos:definition "For ordering ordered lists." ;
              skos:prefLabel "sequence" .


###  https://ontologies.semanticarts.com/gist/startDateTime
gist:startDateTime rdf:type owl:DatatypeProperty ;
                   rdfs:subPropertyOf gist:atDateTime ;
                   rdfs:range xsd:dateTime ;
                   rdfs:isDefinedBy <https://ontologies.semanticarts.com/o/gistCore> ;
                   skos:definition "The date and time that something started." ;
                   skos:prefLabel "start date time" ;
                   skos:scopeNote "This is an abstraction over the various precisions of start time, and is not expected to be asserted directly. Values with different precisions can be compared since they all have the same format." ,
                                  "We have looked at some extreme edge cases (e.g., did this meeting end before or after the trade was posted?) and we couldn't find any use case that required special processing. Those who have such use cases can implement them (and feel free to let us know)." .


###  https://ontologies.semanticarts.com/gist/tagText
gist:tagText rdf:type owl:DatatypeProperty ;
             rdfs:isDefinedBy <https://ontologies.semanticarts.com/o/gistCore> ;
             skos:definition "Used for folksonomy style categories (non controlled vocabulary)" ;
             skos:prefLabel "tag text" .


###  https://ontologies.semanticarts.com/gist/uniqueText
gist:uniqueText rdf:type owl:DatatypeProperty ,
                         owl:FunctionalProperty ;
                rdfs:range xsd:string ;
                rdfs:isDefinedBy <https://ontologies.semanticarts.com/o/gistCore> ;
                skos:definition "The unique string value of some content object; i.e., there is no possibility of having more than one value." ;
                skos:example "The unique string for a vehicle identification number." ;
                skos:prefLabel "unique text" ;
                gist:domainIncludes gist:ID ,
                                    gist:Text .


###  https://ontologies.semanticarts.com/gist/unitSymbol
gist:unitSymbol rdf:type owl:DatatypeProperty ;
                rdfs:domain gist:UnitOfMeasure ;
                rdfs:range xsd:string ;
                rdfs:isDefinedBy <https://ontologies.semanticarts.com/o/gistCore> ;
                skos:definition "The standard symbol for the unit NOT using any special characters.  E.g. square meter would be m^2 rather than m?." ;
                skos:prefLabel "unit symbol" .


###  https://ontologies.semanticarts.com/gist/unitSymbolHtml
gist:unitSymbolHtml rdf:type owl:DatatypeProperty ;
                    rdfs:domain gist:UnitOfMeasure ;
                    rdfs:range xsd:string ;
                    rdfs:isDefinedBy <https://ontologies.semanticarts.com/o/gistCore> ;
                    skos:definition "The standard symbol for the unit in HTML format for  pretty printing, may use special characters.  E.g. to show square meter as  m? rather than m^2, the value of this property would be \"m&sup2;\" This is for when Unicode not supported and the display will be HTML format." ;
                    skos:prefLabel "unit symbol HTML" .


###  https://ontologies.semanticarts.com/gist/unitSymbolUnicode
gist:unitSymbolUnicode rdf:type owl:DatatypeProperty ;
                       rdfs:domain gist:UnitOfMeasure ;
                       rdfs:range xsd:string ;
                       rdfs:isDefinedBy <https://ontologies.semanticarts.com/o/gistCore> ;
                       skos:definition "The standard symbol for the unit preferred for pretty printing, may use special characters.  E.g. square meter would be  m? rather than m^2." ;
                       skos:prefLabel "unit symbol Unicode" .


#################################################################
#    Classes
#################################################################

###  http://www.w3.org/ns/shacl#PrefixDeclaration
sh:PrefixDeclaration rdf:type owl:Class .


###  https://ontologies.semanticarts.com/gist/Account
gist:Account rdf:type owl:Class ;
             owl:equivalentClass [ owl:intersectionOf ( gist:Agreement
                                                        [ rdf:type owl:Restriction ;
                                                          owl:onProperty gist:hasMagnitude ;
                                                          owl:someValuesFrom gist:Balance
                                                        ]
                                                      ) ;
                                   rdf:type owl:Class
                                 ] ;
             rdfs:isDefinedBy <https://ontologies.semanticarts.com/o/gistCore> ;
             skos:definition "An agreement having a balance, as in a bank account, or credit card account, or Accounts Receivable account." ;
             skos:prefLabel "Account" .


###  https://ontologies.semanticarts.com/gist/Actuator
gist:Actuator rdf:type owl:Class ;
              rdfs:subClassOf gist:Equipment ;
              rdfs:isDefinedBy <https://ontologies.semanticarts.com/o/gistCore> ;
              skos:definition "A device that can affect the real world via a message interface" ;
              skos:prefLabel "Actuator" .


###  https://ontologies.semanticarts.com/gist/Address
gist:Address rdf:type owl:Class ;
             rdfs:subClassOf gist:Content ;
             rdfs:isDefinedBy <https://ontologies.semanticarts.com/o/gistCore> ;
             skos:definition "A reference to a place (real or virtual) that can be located by some routing algorithm, and where messages or things can be sent to or retrieved from. E.g. PO Box or URL to a PDF file." ;
             skos:prefLabel "Address" .


###  https://ontologies.semanticarts.com/gist/Agreement
gist:Agreement rdf:type owl:Class ;
               owl:equivalentClass [ owl:intersectionOf ( gist:Commitment
                                                          [ rdf:type owl:Restriction ;
                                                            owl:onProperty gist:hasParty ;
                                                            owl:someValuesFrom [ rdf:type owl:Class ;
                                                                                 owl:unionOf ( gist:Organization
                                                                                               gist:Person
                                                                                             )
                                                                               ]
                                                          ]
                                                          [ rdf:type owl:Restriction ;
                                                            owl:onProperty gist:hasDirectPart ;
                                                            owl:minQualifiedCardinality "2"^^xsd:nonNegativeInteger ;
                                                            owl:onClass gist:Obligation
                                                          ]
                                                        ) ;
                                     rdf:type owl:Class
                                   ] ;
               rdfs:isDefinedBy <https://ontologies.semanticarts.com/o/gistCore> ;
               skos:definition "Something which two or more People or Organizations mutually commit to do." ;
               skos:prefLabel "Agreement" .


###  https://ontologies.semanticarts.com/gist/Area
gist:Area rdf:type owl:Class ;
          owl:equivalentClass [ owl:intersectionOf ( gist:Magnitude
                                                     [ rdf:type owl:Restriction ;
                                                       owl:onProperty gist:hasUnitOfMeasure ;
                                                       owl:someValuesFrom gist:AreaUnit
                                                     ]
                                                   ) ;
                                rdf:type owl:Class
                              ] ;
          rdfs:isDefinedBy <https://ontologies.semanticarts.com/o/gistCore> ;
          skos:definition "A measurement of two-dimensional space." ;
          skos:prefLabel "Area" .


###  https://ontologies.semanticarts.com/gist/AreaUnit
gist:AreaUnit rdf:type owl:Class ;
              owl:equivalentClass [ owl:intersectionOf ( gist:ProductUnit
                                                         [ rdf:type owl:Restriction ;
                                                           owl:onProperty gist:hasMultiplicand ;
                                                           owl:qualifiedCardinality "1"^^xsd:nonNegativeInteger ;
                                                           owl:onClass gist:DistanceUnit
                                                         ]
                                                         [ rdf:type owl:Restriction ;
                                                           owl:onProperty gist:hasMultiplier ;
                                                           owl:qualifiedCardinality "1"^^xsd:nonNegativeInteger ;
                                                           owl:onClass gist:DistanceUnit
                                                         ]
                                                       ) ;
                                    rdf:type owl:Class
                                  ] ;
              rdfs:isDefinedBy <https://ontologies.semanticarts.com/o/gistCore> ;
              skos:definition "A unit of two-dimensional area, such as square inches or hectares." ;
              skos:prefLabel "Area Unit" .


###  https://ontologies.semanticarts.com/gist/Artifact
gist:Artifact rdf:type owl:Class ;
              rdfs:subClassOf [ rdf:type owl:Restriction ;
                                owl:onProperty gist:hasGoal ;
                                owl:someValuesFrom gist:Function
                              ] ;
              rdfs:isDefinedBy <https://ontologies.semanticarts.com/o/gistCore> ;
              skos:definition "An intentional, person-made thing, which could be physical or content" ;
              skos:prefLabel "Artifact" .


###  https://ontologies.semanticarts.com/gist/Aspect
gist:Aspect rdf:type owl:Class ;
            rdfs:subClassOf gist:Category ;
            rdfs:isDefinedBy <https://ontologies.semanticarts.com/o/gistCore> ;
            skos:definition "A very general term for the characteristic of something that is being measured.  E.g., property (height) or a process (cycle time) or a behavior (loyalty)." ;
            skos:prefLabel "Aspect" .


###  https://ontologies.semanticarts.com/gist/Balance
gist:Balance rdf:type owl:Class ;
             owl:equivalentClass [ owl:intersectionOf ( gist:Magnitude
                                                        [ rdf:type owl:Restriction ;
                                                          owl:onProperty gist:isAffectedBy ;
                                                          owl:someValuesFrom gist:Transaction
                                                        ]
                                                      ) ;
                                   rdf:type owl:Class
                                 ] ;
             rdfs:isDefinedBy <https://ontologies.semanticarts.com/o/gistCore> ;
             skos:definition "An amount decremented or incremented by a series of transactions." ;
             skos:prefLabel "Balance" .


###  https://ontologies.semanticarts.com/gist/BaseUnit
gist:BaseUnit rdf:type owl:Class ;
              owl:equivalentClass [ rdf:type owl:Class ;
                                    owl:oneOf ( gist:_USDollar
                                                gist:_ampere
                                                gist:_bit
                                                gist:_candela
                                                gist:_each
                                                gist:_kelvin
                                                gist:_kilogram
                                                gist:_meter
                                                gist:_mole
                                                gist:_second
                                              )
                                  ] ;
              rdfs:subClassOf gist:SimpleUnitOfMeasure ;
              rdfs:isDefinedBy <https://ontologies.semanticarts.com/o/gistCore> ;
              skos:definition "A primitive unit that cannot be decomposed into other units. It can be converted from one measurement system to another.  The base units in gist are the seven primitive units from the System Internationale (SI): (meter, second, kilogram, ampere, kelvin, mole, candela), plus three convenience ones: each. bit and usDollar." ;
              skos:prefLabel "Base Unit" .


###  https://ontologies.semanticarts.com/gist/Behavior
gist:Behavior rdf:type owl:Class ;
              rdfs:subClassOf gist:Category ;
              rdfs:isDefinedBy <https://ontologies.semanticarts.com/o/gistCore> ;
              skos:definition "A way of categorizing events.  E.g., differentiating drilling versus cutting." ;
              skos:prefLabel "Behavior" .


###  https://ontologies.semanticarts.com/gist/Building
gist:Building rdf:type owl:Class ;
              rdfs:subClassOf gist:Artifact ,
                              gist:Landmark ;
              rdfs:isDefinedBy <https://ontologies.semanticarts.com/o/gistCore> ;
              skos:definition "A relatively permanent man-made structure situated on a plot of land, having a roof and walls, commonly used for dwelling, entertaining, or working." ;
              skos:example "A house, school, store, factory, chicken coop." ,
                           "Negative examples: houseboats (not built on land), caves (not man-made), food trucks and RVs (not permanently situated)." ;
              skos:prefLabel "Building" ;
              skos:scopeNote "User discretion can be applied to edge cases: e.g., is a traditional yurt 'relatively permanently situated' although it is portable and has a tent-like construction?" .


###  https://ontologies.semanticarts.com/gist/BundledCatalogItem
gist:BundledCatalogItem rdf:type owl:Class ;
                        owl:equivalentClass [ owl:intersectionOf ( gist:CatalogItem
                                                                   [ rdf:type owl:Restriction ;
                                                                     owl:onProperty gist:hasDirectPart ;
                                                                     owl:someValuesFrom gist:CatalogItem
                                                                   ]
                                                                 ) ;
                                              rdf:type owl:Class
                                            ] ;
                        rdfs:isDefinedBy <https://ontologies.semanticarts.com/o/gistCore> ;
                        skos:definition "Any combination of descriptions of things offered together.  Could be a kit (several parts offered together), but could also be a product plus a warranty." ;
                        skos:prefLabel "Bundled Catalog Item" .


###  https://ontologies.semanticarts.com/gist/CatalogItem
gist:CatalogItem rdf:type owl:Class ;
                 rdfs:subClassOf gist:Specification ;
                 rdfs:isDefinedBy <https://ontologies.semanticarts.com/o/gistCore> ;
                 skos:definition "A description of a product or service to be delivered, given in a sufficient level of detail that a receiver could determine whether delivery constituted discharge of the obligation to deliver." ;
                 skos:prefLabel "Catalog Item" ;
                 skos:scopeNote "In short, an unambiguous characterization of what it is that a potential buyer is paying for." .


###  https://ontologies.semanticarts.com/gist/Category
gist:Category rdf:type owl:Class ;
              rdfs:subClassOf [ rdf:type owl:Restriction ;
                                owl:onProperty gist:isAllocatedBy ;
                                owl:someValuesFrom [ rdf:type owl:Class ;
                                                     owl:unionOf ( gist:IntellectualProperty
                                                                   gist:Organization
                                                                   gist:Person
                                                                 )
                                                   ]
                              ] ;
              rdfs:isDefinedBy <https://ontologies.semanticarts.com/o/gistCore> ;
              skos:definition "A concept or label used to categorize other instances informally. Things that can be thought of as types are usually Categories." ;
              skos:example "Tags used in folksonomies; formal definitions from other systems." ;
              skos:prefLabel "Category" ;
              skos:scopeNote "Often a 'bucket' can be modeled either as an owl:Class or as a gist:Category. Use the latter if you don't care much about the formal structure of the different types, or if there is a whole hierarchy of types that are going to be managed by a group separate from the ontology developers. The formal structure may be defined elsewhere and linked to, if necessary." .


###  https://ontologies.semanticarts.com/gist/CoherentProductUnit
gist:CoherentProductUnit rdf:type owl:Class ;
                         owl:equivalentClass [ owl:intersectionOf ( gist:ProductUnit
                                                                    [ rdf:type owl:Restriction ;
                                                                      owl:onProperty gist:hasMultiplicand ;
                                                                      owl:allValuesFrom [ rdf:type owl:Class ;
                                                                                          owl:unionOf ( gist:BaseUnit
                                                                                                        gist:CoherentProductUnit
                                                                                                        gist:CoherentRatioUnit
                                                                                                      )
                                                                                        ]
                                                                    ]
                                                                    [ rdf:type owl:Restriction ;
                                                                      owl:onProperty gist:hasMultiplier ;
                                                                      owl:allValuesFrom [ rdf:type owl:Class ;
                                                                                          owl:unionOf ( gist:BaseUnit
                                                                                                        gist:CoherentProductUnit
                                                                                                        gist:CoherentRatioUnit
                                                                                                      )
                                                                                        ]
                                                                    ]
                                                                  ) ;
                                               rdf:type owl:Class
                                             ] ;
                         rdfs:isDefinedBy <https://ontologies.semanticarts.com/o/gistCore> ;
                         skos:definition "A product unit both of whose factors are coherent units. The conversion factor is 1." ;
                         skos:example "Square meter, an area unit." ;
                         skos:prefLabel "Coherent Product Unit" .


###  https://ontologies.semanticarts.com/gist/CoherentRatioUnit
gist:CoherentRatioUnit rdf:type owl:Class ;
                       owl:equivalentClass [ owl:intersectionOf ( gist:RatioUnit
                                                                  [ rdf:type owl:Restriction ;
                                                                    owl:onProperty gist:hasDenominator ;
                                                                    owl:allValuesFrom [ rdf:type owl:Class ;
                                                                                        owl:unionOf ( gist:BaseUnit
                                                                                                      gist:CoherentProductUnit
                                                                                                      gist:CoherentRatioUnit
                                                                                                    )
                                                                                      ]
                                                                  ]
                                                                  [ rdf:type owl:Restriction ;
                                                                    owl:onProperty gist:hasNumerator ;
                                                                    owl:allValuesFrom [ rdf:type owl:Class ;
                                                                                        owl:unionOf ( gist:BaseUnit
                                                                                                      gist:CoherentProductUnit
                                                                                                      gist:CoherentRatioUnit
                                                                                                    )
                                                                                      ]
                                                                  ]
                                                                ) ;
                                             rdf:type owl:Class
                                           ] ;
                       rdfs:isDefinedBy <https://ontologies.semanticarts.com/o/gistCore> ;
                       skos:definition "A ratio unit whose conversion factor is 1." ;
                       skos:example "Newton, a force unit also expressed as kg-m/s^2" ;
                       skos:prefLabel "Coherent Ratio Unit" .


###  https://ontologies.semanticarts.com/gist/CoherentUnit
gist:CoherentUnit rdf:type owl:Class ;
                  owl:equivalentClass [ rdf:type owl:Class ;
                                        owl:unionOf ( gist:BaseUnit
                                                      gist:CoherentProductUnit
                                                      gist:CoherentRatioUnit
                                                    )
                                      ] ;
                  rdfs:isDefinedBy <https://ontologies.semanticarts.com/o/gistCore> ;
                  rdfs:seeAlso <http://www.eim.gr/metrology/measurement-units/si-derived-units/coherent-derived-units/> ;
                  skos:definition "A unit that is expressed in units that have no conversions.  It may be a simple unit.  It may also be a product or ratio unit that bottoms out in simple units." ;
                  skos:example "A simple unit: kilogram" ,
                               "The standard unit for acceleration is meters per square second (feet per square second  requires a conversion)" ;
                  skos:prefLabel "Coherent Unit" ;
                  skos:scopeNote "Coherent unit is the physics term for this, informally you might think of it as the standard unit for a given dimension." ,
                                 "In principle, the CoherentUnit for a ProductUnit or RatioUnit can be inferred by recursively decomposing the products and ratios into their respective CoherentUnits, bottoming out in SimpleUnits" .


###  https://ontologies.semanticarts.com/gist/Collection
gist:Collection rdf:type owl:Class ;
                rdfs:isDefinedBy <https://ontologies.semanticarts.com/o/gistCore> ;
                skos:definition "A grouping of things." ;
                skos:example "A jury is a group of people, a financial ledger is a collection of transaction entries; a route is an (ordered) collection of segments." ;
                skos:prefLabel "Collection" ;
                skos:scopeNote "Individuals are placed in the collection using the gist:hasMember property. Collections typically are created because the members are functionally connected in some way. This definition allows a collection to have zero members." .


###  https://ontologies.semanticarts.com/gist/Commitment
gist:Commitment rdf:type owl:Class ;
                owl:equivalentClass [ owl:intersectionOf ( [ rdf:type owl:Class ;
                                                             owl:unionOf ( gist:Requirement
                                                                           gist:Restriction
                                                                         )
                                                           ]
                                                           [ rdf:type owl:Restriction ;
                                                             owl:onProperty gist:hasGiver ;
                                                             owl:someValuesFrom [ rdf:type owl:Class ;
                                                                                  owl:unionOf ( gist:Organization
                                                                                                gist:Person
                                                                                              )
                                                                                ]
                                                           ]
                                                           [ rdf:type owl:Restriction ;
                                                             owl:onProperty gist:isCategorizedBy ;
                                                             owl:someValuesFrom gist:DegreeOfCommitment
                                                           ]
                                                         ) ;
                                      rdf:type owl:Class
                                    ] ;
                rdfs:isDefinedBy <https://ontologies.semanticarts.com/o/gistCore> ;
                skos:definition "An obligation (possibly unilateral)." ;
                skos:prefLabel "Commitment" .


###  https://ontologies.semanticarts.com/gist/Component
gist:Component rdf:type owl:Class ;
               owl:equivalentClass [ owl:intersectionOf ( gist:Artifact
                                                          [ rdf:type owl:Restriction ;
                                                            owl:onProperty gist:contributesTo ;
                                                            owl:someValuesFrom gist:System
                                                          ]
                                                        ) ;
                                     rdf:type owl:Class
                                   ] ;
               rdfs:isDefinedBy <https://ontologies.semanticarts.com/o/gistCore> ;
               skos:definition "A component is an artifact that contributes to a system.  Could be a simple mechanical component, such as the float contributing to the toilet tank maintaining a constant level, or much more complex as in the internet of things." ;
               skos:prefLabel "Component" .


###  https://ontologies.semanticarts.com/gist/ContemporaryEvent
gist:ContemporaryEvent rdf:type owl:Class ;
                       owl:equivalentClass [ owl:intersectionOf ( gist:Event
                                                                  [ rdf:type owl:Restriction ;
                                                                    owl:onProperty gist:actualStartDateTime ;
                                                                    owl:cardinality "1"^^xsd:nonNegativeInteger
                                                                  ]
                                                                  [ rdf:type owl:Restriction ;
                                                                    owl:onProperty gist:actualEndDateTime ;
                                                                    owl:maxCardinality "0"^^xsd:nonNegativeInteger
                                                                  ]
                                                                ) ;
                                             rdf:type owl:Class
                                           ] ;
                       rdfs:isDefinedBy <https://ontologies.semanticarts.com/o/gistCore> ;
                       skos:definition "An event that has started but has not yet ended." ;
                       skos:prefLabel "Contemporary Event" ;
                       skos:scopeNote "When the event actually ends, it will cease being contemporary." .


###  https://ontologies.semanticarts.com/gist/Content
gist:Content rdf:type owl:Class ;
             rdfs:subClassOf gist:Artifact ;
             owl:disjointWith gist:GeoPoint ,
                              gist:GeoRegion ,
                              gist:Organization ,
                              gist:PhysicalIdentifiableItem ,
                              gist:PhysicalSubstance ,
                              gist:UnitOfMeasure ;
             rdfs:isDefinedBy <https://ontologies.semanticarts.com/o/gistCore> ;
             skos:definition "A document, program, image, etc.  (Categories are not content until they are written down.)" ;
             skos:prefLabel "Content" .


###  https://ontologies.semanticarts.com/gist/ContentExpression
gist:ContentExpression rdf:type owl:Class ;
                       rdfs:subClassOf gist:Content ,
                                       [ rdf:type owl:Restriction ;
                                         owl:onProperty gist:isCategorizedBy ;
                                         owl:someValuesFrom gist:GeneralMediaType
                                       ] ,
                                       [ rdf:type owl:Restriction ;
                                         owl:onProperty gist:isExpressedIn ;
                                         owl:someValuesFrom gist:Language
                                       ] ;
                       rdfs:isDefinedBy <https://ontologies.semanticarts.com/o/gistCore> ;
                       skos:definition "Intellectual Property reduced to text, audio etc.  If it contains text (written or spoken), it may be in a language." ;
                       skos:prefLabel "Content Expression" .


###  https://ontologies.semanticarts.com/gist/ContingentEvent
gist:ContingentEvent rdf:type owl:Class ;
                     owl:equivalentClass [ owl:intersectionOf ( gist:Event
                                                                [ rdf:type owl:Restriction ;
                                                                  owl:onProperty gist:hasMagnitude ;
                                                                  owl:someValuesFrom gist:Percentage
                                                                ]
                                                                [ rdf:type owl:Restriction ;
                                                                  owl:onProperty gist:plannedEndDateTime ;
                                                                  owl:someValuesFrom xsd:dateTime
                                                                ]
                                                                [ rdf:type owl:Restriction ;
                                                                  owl:onProperty gist:plannedStartDateTime ;
                                                                  owl:someValuesFrom xsd:dateTime
                                                                ]
                                                              ) ;
                                           rdf:type owl:Class
                                         ] ;
                     rdfs:isDefinedBy <https://ontologies.semanticarts.com/o/gistCore> ;
                     skos:definition "An event with a probability of happening in the future, and usually dependent upon some other event or condition." ;
                     skos:prefLabel "Contingent Event" .


###  https://ontologies.semanticarts.com/gist/ContingentObligation
gist:ContingentObligation rdf:type owl:Class ;
                          owl:equivalentClass [ owl:intersectionOf ( gist:Commitment
                                                                     [ rdf:type owl:Restriction ;
                                                                       owl:onProperty gist:hasGiver ;
                                                                       owl:someValuesFrom [ rdf:type owl:Class ;
                                                                                            owl:unionOf ( gist:Organization
                                                                                                          gist:Person
                                                                                                        )
                                                                                          ]
                                                                     ]
                                                                     [ rdf:type owl:Restriction ;
                                                                       owl:onProperty gist:isTriggeredBy ;
                                                                       owl:someValuesFrom gist:Event
                                                                     ]
                                                                   ) ;
                                                rdf:type owl:Class
                                              ] ;
                          rdfs:isDefinedBy <https://ontologies.semanticarts.com/o/gistCore> ;
                          skos:definition "An obligation that is not yet firm.  There is some contingent event, the occurrence of which will cause the obligation to become firm." ;
                          skos:prefLabel "Contingent Obligation" ;
                          skos:scopeNote "A contingent obligation might have a getter counterparty (as in the case of insurance); but it might not (as in the case of an offer)." .


###  https://ontologies.semanticarts.com/gist/Contract
gist:Contract rdf:type owl:Class ;
              owl:equivalentClass [ owl:intersectionOf ( gist:Agreement
                                                         [ rdf:type owl:Restriction ;
                                                           owl:onProperty gist:isUnderJurisdictionOf ;
                                                           owl:someValuesFrom gist:GovernmentOrganization
                                                         ]
                                                       ) ;
                                    rdf:type owl:Class
                                  ] ;
              rdfs:isDefinedBy <https://ontologies.semanticarts.com/o/gistCore> ;
              skos:definition "An Agreement which can be enforced by law" ;
              skos:prefLabel "Contract" .


###  https://ontologies.semanticarts.com/gist/ContractTerm
gist:ContractTerm rdf:type owl:Class ;
                  rdfs:subClassOf gist:Specification ;
                  rdfs:isDefinedBy <https://ontologies.semanticarts.com/o/gistCore> ;
                  skos:definition "A specification of some aspect of a contract." ;
                  skos:prefLabel "Contract Term" .


###  https://ontologies.semanticarts.com/gist/ControlledVocabulary
gist:ControlledVocabulary rdf:type owl:Class ;
                          owl:equivalentClass [ owl:intersectionOf ( gist:Collection
                                                                     [ rdf:type owl:Restriction ;
                                                                       owl:onProperty gist:hasMember ;
                                                                       owl:someValuesFrom gist:Category
                                                                     ]
                                                                     [ rdf:type owl:Restriction ;
                                                                       owl:onProperty gist:isGovernedBy ;
                                                                       owl:someValuesFrom [ rdf:type owl:Class ;
                                                                                            owl:unionOf ( gist:Organization
                                                                                                          gist:Person
                                                                                                        )
                                                                                          ]
                                                                     ]
                                                                   ) ;
                                                rdf:type owl:Class
                                              ] ;
                          rdfs:isDefinedBy <https://ontologies.semanticarts.com/o/gistCore> ;
                          skos:definition "A collection of terms approved and managed by some organization or person." ;
                          skos:prefLabel "Controlled Vocabulary" .


###  https://ontologies.semanticarts.com/gist/Controller
gist:Controller rdf:type owl:Class ;
                owl:equivalentClass [ owl:intersectionOf ( gist:Equipment
                                                           [ rdf:type owl:Restriction ;
                                                             owl:onProperty gist:directs ;
                                                             owl:someValuesFrom gist:Actuator
                                                           ]
                                                           [ rdf:type owl:Restriction ;
                                                             owl:onProperty gist:isCategorizedBy ;
                                                             owl:someValuesFrom gist:ControllerType
                                                           ]
                                                           [ rdf:type owl:Restriction ;
                                                             owl:onProperty gist:respondsTo ;
                                                             owl:someValuesFrom gist:Sensor
                                                           ]
                                                         ) ;
                                      rdf:type owl:Class
                                    ] ;
                rdfs:isDefinedBy <https://ontologies.semanticarts.com/o/gistCore> ;
                skos:definition "A device that takes messages or signals from a sensor and decides through algorithms whether and which actuator to fire via messages" ;
                skos:prefLabel "Controller" .


###  https://ontologies.semanticarts.com/gist/ControllerType
gist:ControllerType rdf:type owl:Class ;
                    rdfs:subClassOf gist:Category ;
                    rdfs:isDefinedBy <https://ontologies.semanticarts.com/o/gistCore> ;
                    skos:definition "A kind of controller." ;
                    skos:prefLabel "Controller Type" .


###  https://ontologies.semanticarts.com/gist/Count
gist:Count rdf:type owl:Class ;
           owl:equivalentClass [ owl:intersectionOf ( gist:Magnitude
                                                      [ rdf:type owl:Restriction ;
                                                        owl:onProperty gist:hasUnitOfMeasure ;
                                                        owl:someValuesFrom gist:CountingUnit
                                                      ]
                                                    ) ;
                                 rdf:type owl:Class
                               ] ;
           rdfs:isDefinedBy <https://ontologies.semanticarts.com/o/gistCore> ;
           skos:definition "A measure that involves countable amounts (?eaches? as well as cases, etc.). Can be decimal." ;
           skos:prefLabel "Count" ;
           skos:scopeNote "Count is not disjoint with all the other magnitudes, as there are some magnitudes that could conceivably be counted." .


###  https://ontologies.semanticarts.com/gist/CountingUnit
gist:CountingUnit rdf:type owl:Class ;
                  owl:equivalentClass [ owl:intersectionOf ( gist:SimpleUnitOfMeasure
                                                             [ rdf:type owl:Restriction ;
                                                               owl:onProperty gist:hasBaseUnit ;
                                                               owl:hasValue gist:_each
                                                             ]
                                                           ) ;
                                        rdf:type owl:Class
                                      ] ;
                  rdfs:isDefinedBy <https://ontologies.semanticarts.com/o/gistCore> ;
                  skos:definition "A unit of counting, especially ?each?, but also units such as dozens." ;
                  skos:prefLabel "Counting Unit" .


###  https://ontologies.semanticarts.com/gist/CountryGeoRegion
gist:CountryGeoRegion rdf:type owl:Class ;
                      owl:equivalentClass [ owl:intersectionOf ( gist:GovernedGeoRegion
                                                                 [ rdf:type owl:Restriction ;
                                                                   owl:onProperty gist:isGovernedBy ;
                                                                   owl:qualifiedCardinality "1"^^xsd:nonNegativeInteger ;
                                                                   owl:onClass gist:CountryGovernment
                                                                 ]
                                                               ) ;
                                            rdf:type owl:Class
                                          ] ;
                      rdfs:isDefinedBy <https://ontologies.semanticarts.com/o/gistCore> ;
                      skos:definition "A defined geographical area (or areas) governed by exactly one country government." ;
                      skos:prefLabel "Country Geo-Region" .


###  https://ontologies.semanticarts.com/gist/CountryGovernment
gist:CountryGovernment rdf:type owl:Class ;
                       owl:equivalentClass [ owl:intersectionOf ( gist:GovernmentOrganization
                                                                  [ rdf:type owl:Restriction ;
                                                                    owl:onProperty gist:governs ;
                                                                    owl:qualifiedCardinality "1"^^xsd:nonNegativeInteger ;
                                                                    owl:onClass gist:CountryGeoRegion
                                                                  ]
                                                                  [ rdf:type owl:Restriction ;
                                                                    owl:onProperty gist:isGovernedBy ;
                                                                    owl:maxQualifiedCardinality "0"^^xsd:nonNegativeInteger ;
                                                                    owl:onClass gist:GovernmentOrganization
                                                                  ]
                                                                ) ;
                                             rdf:type owl:Class
                                           ] ;
                       owl:disjointWith gist:SubCountryGovernment ;
                       rdfs:isDefinedBy <https://ontologies.semanticarts.com/o/gistCore> ;
                       skos:definition "A Government Organization which asserts both sovereignty (i.e., it is not governed by some other government organization) and governance over an entity generally recognized as a 'country'." ;
                       skos:prefLabel "Country Government" ;
                       skos:scopeNote "While a country government may enter into treaties with other country governments, there are no governing relationships among the treaty members." .


###  https://ontologies.semanticarts.com/gist/CurrencyUnit
gist:CurrencyUnit rdf:type owl:Class ;
                  owl:equivalentClass [ owl:intersectionOf ( gist:SimpleUnitOfMeasure
                                                             [ rdf:type owl:Restriction ;
                                                               owl:onProperty gist:hasBaseUnit ;
                                                               owl:hasValue gist:_USDollar
                                                             ]
                                                           ) ;
                                        rdf:type owl:Class
                                      ] ;
                  owl:disjointWith gist:DataSizeUnit ,
                                   gist:DistanceUnit ,
                                   gist:DurationUnit ,
                                   gist:ElectricalCurrentUnit ,
                                   gist:LuminousIntensityUnit ,
                                   gist:MassUnit ,
                                   gist:MoleUnit ,
                                   gist:TemperatureUnit ;
                  rdfs:isDefinedBy <https://ontologies.semanticarts.com/o/gistCore> ;
                  skos:definition "A unit of money. Note: this is the only unit whose conversion factors include time (i.e., the conversion rates change on a daily basis)." ;
                  skos:prefLabel "Currency Unit" .


###  https://ontologies.semanticarts.com/gist/DataSizeUnit
gist:DataSizeUnit rdf:type owl:Class ;
                  owl:equivalentClass [ owl:intersectionOf ( gist:SimpleUnitOfMeasure
                                                             [ rdf:type owl:Restriction ;
                                                               owl:onProperty gist:hasBaseUnit ;
                                                               owl:hasValue gist:_bit
                                                             ]
                                                           ) ;
                                        rdf:type owl:Class
                                      ] ;
                  owl:disjointWith gist:DistanceUnit ,
                                   gist:DurationUnit ,
                                   gist:ElectricalCurrentUnit ,
                                   gist:LuminousIntensityUnit ,
                                   gist:MassUnit ,
                                   gist:MoleUnit ,
                                   gist:TemperatureUnit ;
                  rdfs:isDefinedBy <https://ontologies.semanticarts.com/o/gistCore> ;
                  skos:definition "A unit to measure amounts of digital information." ;
                  skos:prefLabel "Data Size Unit" .


###  https://ontologies.semanticarts.com/gist/DegreeOfCommitment
gist:DegreeOfCommitment rdf:type owl:Class ;
                        rdfs:subClassOf gist:Category ;
                        rdfs:isDefinedBy <https://ontologies.semanticarts.com/o/gistCore> ;
                        skos:definition "The difficulty of reversing a commitment." ;
                        skos:example "A car rental typically has a lower degree of commitment than an airfare reservation." ;
                        skos:prefLabel "Degree Of Commitment" .


###  https://ontologies.semanticarts.com/gist/DistanceUnit
gist:DistanceUnit rdf:type owl:Class ;
                  owl:equivalentClass [ owl:intersectionOf ( gist:SimpleUnitOfMeasure
                                                             [ rdf:type owl:Restriction ;
                                                               owl:onProperty gist:hasBaseUnit ;
                                                               owl:hasValue gist:_meter
                                                             ]
                                                           ) ;
                                        rdf:type owl:Class
                                      ] ;
                  owl:disjointWith gist:DurationUnit ,
                                   gist:ElectricalCurrentUnit ,
                                   gist:LuminousIntensityUnit ,
                                   gist:MassUnit ,
                                   gist:MoleUnit ,
                                   gist:TemperatureUnit ;
                  rdfs:isDefinedBy <https://ontologies.semanticarts.com/o/gistCore> ;
                  skos:definition "A unit to measure linear distance, such as feet or kilometers." ;
                  skos:prefLabel "Distance Unit" .


###  https://ontologies.semanticarts.com/gist/Duration
gist:Duration rdf:type owl:Class ;
              owl:equivalentClass [ owl:intersectionOf ( gist:Magnitude
                                                         [ rdf:type owl:Restriction ;
                                                           owl:onProperty gist:hasUnitOfMeasure ;
                                                           owl:someValuesFrom gist:DurationUnit
                                                         ]
                                                       ) ;
                                    rdf:type owl:Class
                                  ] ;
              rdfs:isDefinedBy <https://ontologies.semanticarts.com/o/gistCore> ;
              skos:definition "Time, but not on a timeline." ;
              skos:example "One week (or seven days), but not Jan 1, 2008 to Jan 7, 2008 (which is an interval)." ;
              skos:prefLabel "Duration" ;
              skos:scopeNote "Intervals have durations, but are not themselves durations." .


###  https://ontologies.semanticarts.com/gist/DurationUnit
gist:DurationUnit rdf:type owl:Class ;
                  owl:equivalentClass [ owl:intersectionOf ( gist:SimpleUnitOfMeasure
                                                             [ rdf:type owl:Restriction ;
                                                               owl:onProperty gist:hasBaseUnit ;
                                                               owl:hasValue gist:_second
                                                             ]
                                                           ) ;
                                        rdf:type owl:Class
                                      ] ;
                  owl:disjointWith gist:ElectricalCurrentUnit ,
                                   gist:LuminousIntensityUnit ,
                                   gist:MassUnit ,
                                   gist:MoleUnit ,
                                   gist:TemperatureUnit ;
                  rdfs:isDefinedBy <https://ontologies.semanticarts.com/o/gistCore> ;
                  skos:definition "A unit to measure passage of time: hours, days, years." ;
                  skos:prefLabel "Duration Unit" .


###  https://ontologies.semanticarts.com/gist/ElectricCurrent
gist:ElectricCurrent rdf:type owl:Class ;
                     owl:equivalentClass [ owl:intersectionOf ( gist:Magnitude
                                                                [ rdf:type owl:Restriction ;
                                                                  owl:onProperty gist:hasUnitOfMeasure ;
                                                                  owl:someValuesFrom gist:ElectricalCurrentUnit
                                                                ]
                                                              ) ;
                                           rdf:type owl:Class
                                         ] ;
                     rdfs:isDefinedBy <https://ontologies.semanticarts.com/o/gistCore> ;
                     skos:definition "A flow of electric charge." ;
                     skos:prefLabel "Electric Current" .


###  https://ontologies.semanticarts.com/gist/ElectricalCurrentUnit
gist:ElectricalCurrentUnit rdf:type owl:Class ;
                           owl:equivalentClass [ owl:intersectionOf ( gist:SimpleUnitOfMeasure
                                                                      [ rdf:type owl:Restriction ;
                                                                        owl:onProperty gist:hasBaseUnit ;
                                                                        owl:hasValue gist:_ampere
                                                                      ]
                                                                    ) ;
                                                 rdf:type owl:Class
                                               ] ;
                           owl:disjointWith gist:LuminousIntensityUnit ,
                                            gist:MassUnit ,
                                            gist:MoleUnit ,
                                            gist:TemperatureUnit ;
                           rdfs:isDefinedBy <https://ontologies.semanticarts.com/o/gistCore> ;
                           skos:definition "Unit of electrical current, which is charge per unit time.  The SI unit is the ampere.  (Note that electrical current is a composed unit.)" ;
                           skos:prefLabel "Electrical Current Unit" .


###  https://ontologies.semanticarts.com/gist/ElectronicMessageAddress
gist:ElectronicMessageAddress rdf:type owl:Class ;
                              rdfs:subClassOf gist:Address ;
                              rdfs:isDefinedBy <https://ontologies.semanticarts.com/o/gistCore> ;
                              skos:definition "Any place an electronic message (email, fax, etc.) can be sent." ;
                              skos:prefLabel "Electronic Message Address" .


###  https://ontologies.semanticarts.com/gist/EmailAddress
gist:EmailAddress rdf:type owl:Class ;
                  rdfs:subClassOf gist:ElectronicMessageAddress ;
                  rdfs:isDefinedBy <https://ontologies.semanticarts.com/o/gistCore> ;
                  skos:definition "An email address is a unique identifier for an email account. It is used to both send and receive email messages over the Internet." ;
                  skos:prefLabel "Email Address" .


###  https://ontologies.semanticarts.com/gist/Equipment
gist:Equipment rdf:type owl:Class ;
               owl:equivalentClass [ owl:intersectionOf ( gist:Artifact
                                                          gist:PhysicalIdentifiableItem
                                                          [ rdf:type owl:Restriction ;
                                                            owl:onProperty gist:isCategorizedBy ;
                                                            owl:someValuesFrom gist:EquipmentType
                                                          ]
                                                        ) ;
                                     rdf:type owl:Class
                                   ] ;
               rdfs:isDefinedBy <https://ontologies.semanticarts.com/o/gistCore> ;
               skos:definition "Tangible property other than land or buildings.  Any kind of equipment, could be machine, router, car etc." ;
               skos:prefLabel "Equipment" .


###  https://ontologies.semanticarts.com/gist/EquipmentType
gist:EquipmentType rdf:type owl:Class ;
                   rdfs:subClassOf gist:Category ;
                   rdfs:isDefinedBy <https://ontologies.semanticarts.com/o/gistCore> ;
                   skos:definition "Categories of equipment" ;
                   skos:prefLabel "Equipment Type" .


###  https://ontologies.semanticarts.com/gist/Event
gist:Event rdf:type owl:Class ;
           owl:equivalentClass [ owl:intersectionOf ( [ rdf:type owl:Restriction ;
                                                        owl:onProperty gist:isCharacterizedAs ;
                                                        owl:someValuesFrom gist:Behavior
                                                      ]
                                                      [ rdf:type owl:Restriction ;
                                                        owl:onProperty gist:endDateTime ;
                                                        owl:cardinality "1"^^xsd:nonNegativeInteger
                                                      ]
                                                      [ rdf:type owl:Restriction ;
                                                        owl:onProperty gist:startDateTime ;
                                                        owl:cardinality "1"^^xsd:nonNegativeInteger
                                                      ]
                                                    ) ;
                                 rdf:type owl:Class
                               ] ;
           rdfs:isDefinedBy <https://ontologies.semanticarts.com/o/gistCore> ;
           skos:definition "Something that occurs over some period of time, often characterized as an activity being carried out by some person, organization, or software application." ;
           skos:prefLabel "Event" .


###  https://ontologies.semanticarts.com/gist/Extent
gist:Extent rdf:type owl:Class ;
            owl:equivalentClass [ owl:intersectionOf ( gist:Magnitude
                                                       [ rdf:type owl:Restriction ;
                                                         owl:onProperty gist:hasUnitOfMeasure ;
                                                         owl:someValuesFrom gist:DistanceUnit
                                                       ]
                                                     ) ;
                                  rdf:type owl:Class
                                ] ;
            rdfs:isDefinedBy <https://ontologies.semanticarts.com/o/gistCore> ;
            skos:definition "A measure of distance, which could be distances over the Earth, and could also be height, width, length, depth, girth, etc." ;
            skos:prefLabel "Extent" .


###  https://ontologies.semanticarts.com/gist/FormattedContent
gist:FormattedContent rdf:type owl:Class ;
                      owl:equivalentClass [ owl:intersectionOf ( gist:ContentExpression
                                                                 [ rdf:type owl:Restriction ;
                                                                   owl:onProperty gist:isExpressedIn ;
                                                                   owl:someValuesFrom gist:MediaType
                                                                 ]
                                                               ) ;
                                            rdf:type owl:Class
                                          ] ;
                      rdfs:isDefinedBy <https://ontologies.semanticarts.com/o/gistCore> ;
                      skos:definition "Content which is in a particular format. (E.g., HTML, PDF, JPG.)" ;
                      skos:prefLabel "Formatted Content" .


###  https://ontologies.semanticarts.com/gist/Function
gist:Function rdf:type owl:Class ;
              rdfs:subClassOf gist:Intention ;
              rdfs:isDefinedBy <https://ontologies.semanticarts.com/o/gistCore> ;
              skos:definition "A function is what a specific made item is intended to do.  For instance: transmit electricity, provide ballast, control ambient temperature." ;
              skos:prefLabel "Function" .


###  https://ontologies.semanticarts.com/gist/GeneralMediaType
gist:GeneralMediaType rdf:type owl:Class ;
                      rdfs:subClassOf gist:Category ;
                      rdfs:isDefinedBy <https://ontologies.semanticarts.com/o/gistCore> ;
                      skos:definition "The real-world media type for content." ;
                      skos:example "Audio, still image, video, textual, physical (e.g., a statue), or performance (i.e. a play).  Or it could be oil or pastel for a painting." ;
                      skos:prefLabel "General Media Type" .


###  https://ontologies.semanticarts.com/gist/GeoPoint
gist:GeoPoint rdf:type owl:Class ;
              owl:equivalentClass [ owl:intersectionOf ( [ rdf:type owl:Restriction ;
                                                           owl:onProperty gist:hasAltitude ;
                                                           owl:someValuesFrom gist:Extent
                                                         ]
                                                         [ rdf:type owl:Restriction ;
                                                           owl:onProperty gist:latitude ;
                                                           owl:someValuesFrom xsd:double
                                                         ]
                                                         [ rdf:type owl:Restriction ;
                                                           owl:onProperty gist:longitude ;
                                                           owl:someValuesFrom xsd:double
                                                         ]
                                                       ) ;
                                    rdf:type owl:Class
                                  ] ;
              rdfs:subClassOf gist:Place ;
              owl:disjointWith gist:IntellectualProperty ,
                               gist:Intention ,
                               gist:Language ,
                               gist:Magnitude ,
                               gist:Organization ,
                               gist:PhysicalIdentifiableItem ,
                               gist:PhysicalSubstance ,
                               gist:UnitOfMeasure ;
              rdfs:isDefinedBy <https://ontologies.semanticarts.com/o/gistCore> ;
              skos:definition "An individual point on the Earth's surface, identified by latitude, longitude and altitude. If altitude is missing, it is assumed to be at the Earth's surface.  However, altitude is measured from sea level.  these points are to the WGS-84 coordinate system using the GPS decimal lat/long" ;
              skos:prefLabel "Geo Point" ;
              skos:scopeNote "Assume coordinate system used by Google (WGS 84 Web Mercator)." .


###  https://ontologies.semanticarts.com/gist/GeoRegion
gist:GeoRegion rdf:type owl:Class ;
               owl:equivalentClass [ owl:intersectionOf ( gist:Place
                                                          [ rdf:type owl:Restriction ;
                                                            owl:onProperty gist:hasMagnitude ;
                                                            owl:someValuesFrom gist:Area
                                                          ]
                                                        ) ;
                                     rdf:type owl:Class
                                   ] ;
               owl:disjointWith gist:IntellectualProperty ,
                                gist:Intention ,
                                gist:Language ,
                                gist:Magnitude ,
                                gist:Organization ,
                                gist:PhysicalIdentifiableItem ,
                                gist:PhysicalSubstance ,
                                gist:Template ,
                                gist:UnitOfMeasure ;
               rdfs:isDefinedBy <https://ontologies.semanticarts.com/o/gistCore> ;
               skos:definition "A bounded region (or set of regions) on the surface of the Earth." ;
               skos:example "The bounded shape that defines the region occupied by Crater Lake; the bounded area known as the contiguous USA." ;
               skos:prefLabel "Geo Region" ;
               skos:scopeNote "A GeoRegion could be non-contiguous; e.g. the region governed by the USA is the region governed by the lower 48 states plus that of Alaska and Hawaii.  Child classes in lower ontologies can make this distinction." ,
                              "A GeoRegion has an area, but it is not itself an instance of the Area class.  (Area in gist is a magnitude)." .


###  https://ontologies.semanticarts.com/gist/GeoRoute
gist:GeoRoute rdf:type owl:Class ;
              owl:equivalentClass [ owl:intersectionOf ( gist:OrderedCollection
                                                         gist:Place
                                                         [ rdf:type owl:Restriction ;
                                                           owl:onProperty gist:hasDirectPart ;
                                                           owl:someValuesFrom gist:GeoSegment
                                                         ]
                                                       ) ;
                                    rdf:type owl:Class
                                  ] ;
              rdfs:isDefinedBy <https://ontologies.semanticarts.com/o/gistCore> ;
              skos:definition "An ordered set of GeoPoints that defines a path from starting point to ending point." ;
              skos:prefLabel "Geo Route" .


###  https://ontologies.semanticarts.com/gist/GeoSegment
gist:GeoSegment rdf:type owl:Class ;
                owl:equivalentClass [ owl:intersectionOf ( [ rdf:type owl:Restriction ;
                                                             owl:onProperty gist:comesFromPlace ;
                                                             owl:qualifiedCardinality "1"^^xsd:nonNegativeInteger ;
                                                             owl:onClass gist:GeoPoint
                                                           ]
                                                           [ rdf:type owl:Restriction ;
                                                             owl:onProperty gist:goesToPlace ;
                                                             owl:qualifiedCardinality "1"^^xsd:nonNegativeInteger ;
                                                             owl:onClass gist:GeoPoint
                                                           ]
                                                         ) ;
                                      rdf:type owl:Class
                                    ] ;
                rdfs:subClassOf gist:Place ;
                rdfs:isDefinedBy <https://ontologies.semanticarts.com/o/gistCore> ;
                skos:definition "A single portion of a GeoRegion which has been divided (i.e., segmented)." ;
                skos:prefLabel "Geo Segment" .


###  https://ontologies.semanticarts.com/gist/GeoVolume
gist:GeoVolume rdf:type owl:Class ;
               owl:equivalentClass [ owl:intersectionOf ( [ rdf:type owl:Restriction ;
                                                            owl:onProperty gist:containsGeographically ;
                                                            owl:someValuesFrom gist:GeoPoint
                                                          ]
                                                          [ rdf:type owl:Restriction ;
                                                            owl:onProperty gist:hasMagnitude ;
                                                            owl:someValuesFrom gist:Volume
                                                          ]
                                                        ) ;
                                     rdf:type owl:Class
                                   ] ;
               rdfs:subClassOf gist:Place ;
               rdfs:isDefinedBy <https://ontologies.semanticarts.com/o/gistCore> ;
               skos:definition "A three-dimensional space on or near the surface of the Earth, such as an oil reservoir, the body of a lake, or an airspace." ;
               skos:prefLabel "Geo Volume" .


###  https://ontologies.semanticarts.com/gist/Goal
gist:Goal rdf:type owl:Class ;
          rdfs:subClassOf gist:Intention ;
          rdfs:isDefinedBy <https://ontologies.semanticarts.com/o/gistCore> ;
          skos:definition "A specific intentional endpoint.  One can tell whether it has been achieved, as opposed to an intention, which may not have an evaluation function." ;
          skos:prefLabel "Goal" .


###  https://ontologies.semanticarts.com/gist/GovernedGeoRegion
gist:GovernedGeoRegion rdf:type owl:Class ;
                       owl:equivalentClass [ owl:intersectionOf ( gist:GeoRegion
                                                                  [ rdf:type owl:Restriction ;
                                                                    owl:onProperty gist:isGovernedBy ;
                                                                    owl:minQualifiedCardinality "1"^^xsd:nonNegativeInteger ;
                                                                    owl:onClass gist:GovernmentOrganization
                                                                  ]
                                                                ) ;
                                             rdf:type owl:Class
                                           ] ;
                       rdfs:isDefinedBy <https://ontologies.semanticarts.com/o/gistCore> ;
                       skos:definition "A defined geographic area or areas governed by at least one government organization." ;
                       skos:prefLabel "Governed Geo-Region" ;
                       skos:scopeNote "Geographic regions do not need not be physically contiguous in order to constitute a governed geo-region; e.g., Alaska and Hawaii." .


###  https://ontologies.semanticarts.com/gist/GovernmentOrganization
gist:GovernmentOrganization rdf:type owl:Class ;
                            rdfs:subClassOf gist:Organization ;
                            owl:disjointWith gist:IntergovernmentalOrganization ,
                                             gist:TreatyOrganization ;
                            rdfs:isDefinedBy <https://ontologies.semanticarts.com/o/gistCore> ;
                            skos:definition "An organization which exercises political and/or regulatory authority over a political unit, people, geo-region, etc., as well as performing certain functions for this unit or body. Differs from a corporation in that it cannot be owned." ;
                            skos:example "The State of Washington Office of Financial Management; the Food and Drug Administration; the Scottish Parliament." ;
                            skos:prefLabel "Government Organization" ;
                            skos:scopeNote "Includes administrative, regulatory, and enforcement organizations created or sanctioned by Country or SubCountry Governments." .


###  https://ontologies.semanticarts.com/gist/HistoricalEvent
gist:HistoricalEvent rdf:type owl:Class ;
                     owl:equivalentClass [ owl:intersectionOf ( gist:Event
                                                                [ rdf:type owl:Restriction ;
                                                                  owl:onProperty gist:actualEndDateTime ;
                                                                  owl:cardinality "1"^^xsd:nonNegativeInteger
                                                                ]
                                                                [ rdf:type owl:Restriction ;
                                                                  owl:onProperty gist:actualStartDateTime ;
                                                                  owl:cardinality "1"^^xsd:nonNegativeInteger
                                                                ]
                                                              ) ;
                                           rdf:type owl:Class
                                         ] ;
                     rdfs:isDefinedBy <https://ontologies.semanticarts.com/o/gistCore> ;
                     skos:definition "An event which occurred in time, with an actual end earlier than the present moment." ;
                     skos:prefLabel "Historical Event" .


###  https://ontologies.semanticarts.com/gist/ID
gist:ID rdf:type owl:Class ;
        owl:equivalentClass [ owl:intersectionOf ( gist:Content
                                                   [ rdf:type owl:Restriction ;
                                                     owl:onProperty gist:isAllocatedBy ;
                                                     owl:someValuesFrom [ rdf:type owl:Class ;
                                                                          owl:unionOf ( gist:IntellectualProperty
                                                                                        gist:Organization
                                                                                        gist:Person
                                                                                      )
                                                                        ]
                                                   ]
                                                   [ rdf:type owl:Restriction ;
                                                     owl:onProperty gist:uniqueText ;
                                                     owl:someValuesFrom xsd:string
                                                   ]
                                                 ) ;
                              rdf:type owl:Class
                            ] ;
        rdfs:isDefinedBy <https://ontologies.semanticarts.com/o/gistCore> ;
        skos:definition "Content that is used to uniquely identify something or someone." ;
        skos:example "SSN for a person; serial number for a product; employee ID." ;
        skos:prefLabel "ID" ;
        skos:scopeNote "This is used in conjunction with gist:isIdentifiedBy" .


###  https://ontologies.semanticarts.com/gist/InformationQuantity
gist:InformationQuantity rdf:type owl:Class ;
                         owl:equivalentClass [ owl:intersectionOf ( gist:Magnitude
                                                                    [ rdf:type owl:Restriction ;
                                                                      owl:onProperty gist:hasUnitOfMeasure ;
                                                                      owl:someValuesFrom gist:DataSizeUnit
                                                                    ]
                                                                  ) ;
                                               rdf:type owl:Class
                                             ] ;
                         rdfs:isDefinedBy <https://ontologies.semanticarts.com/o/gistCore> ;
                         skos:definition "An amount of data, such as 6 petabytes, or 640KB." ;
                         skos:prefLabel "Information Quantity" .


###  https://ontologies.semanticarts.com/gist/IntellectualProperty
gist:IntellectualProperty rdf:type owl:Class ;
                          rdfs:subClassOf gist:Artifact ;
                          owl:disjointWith gist:Intention ,
                                           gist:Magnitude ,
                                           gist:Organization ,
                                           gist:PhysicalIdentifiableItem ,
                                           gist:PhysicalSubstance ,
                                           gist:UnitOfMeasure ;
                          rdfs:isDefinedBy <https://ontologies.semanticarts.com/o/gistCore> ;
                          skos:definition "A work, invention or concept, independent of its being expressed in text, audio, video, image, or live performance.  IP can also be tacit knowledge, know-how, or skill. Also includes Brands." ;
                          skos:example "The Old Man and The Sea; the Page Rank algorithm; Coca Cola" ;
                          skos:prefLabel "Intellectual Property" ;
                          skos:scopeNote "For literature this could be called the ?Work?, except that ?work? is a highly overloaded term (expenditure of energy, resource consumption, art).  Often the first expression precedes our recognition of the IP, but subsequent expressions are known to be derivatives of the IP, even if they are expression-to-expression translations (or copies)." .


###  https://ontologies.semanticarts.com/gist/Intention
gist:Intention rdf:type owl:Class ;
               owl:disjointWith gist:Magnitude ,
                                gist:Organization ,
                                gist:PhysicalIdentifiableItem ,
                                gist:PhysicalSubstance ,
                                gist:UnitOfMeasure ;
               rdfs:isDefinedBy <https://ontologies.semanticarts.com/o/gistCore> ;
               skos:definition "Goal, desire, aspiration. This is the \"teleologic\" aspect of the system that indicates things are done with a purpose." ;
               skos:prefLabel "Intention" .


###  https://ontologies.semanticarts.com/gist/IntergovernmentalOrganization
gist:IntergovernmentalOrganization rdf:type owl:Class ;
                                   owl:equivalentClass [ owl:intersectionOf ( gist:Organization
                                                                              [ rdf:type owl:Restriction ;
                                                                                owl:onProperty gist:hasMember ;
                                                                                owl:minQualifiedCardinality "2"^^xsd:nonNegativeInteger ;
                                                                                owl:onClass gist:GovernmentOrganization
                                                                              ]
                                                                            ) ;
                                                         rdf:type owl:Class
                                                       ] ;
                                   rdfs:isDefinedBy <https://ontologies.semanticarts.com/o/gistCore> ;
                                   skos:definition "An organization whose members are government organizations." ;
                                   skos:example "The United Nations, the European Union" ;
                                   skos:prefLabel "Inter-Governmental Organization" .


###  https://ontologies.semanticarts.com/gist/Landmark
gist:Landmark rdf:type owl:Class ;
              owl:equivalentClass [ owl:intersectionOf ( gist:PhysicalIdentifiableItem
                                                         [ rdf:type owl:Restriction ;
                                                           owl:onProperty gist:occupiesGeographicallyPermanently ;
                                                           owl:someValuesFrom [ rdf:type owl:Class ;
                                                                                owl:unionOf ( gist:GeoRegion
                                                                                              gist:GeoVolume
                                                                                            )
                                                                              ]
                                                         ]
                                                       ) ;
                                    rdf:type owl:Class
                                  ] ;
              rdfs:subClassOf gist:Place ;
              rdfs:isDefinedBy <https://ontologies.semanticarts.com/o/gistCore> ;
              skos:definition "Something permanently attached to the Earth." ;
              skos:prefLabel "Landmark" .


###  https://ontologies.semanticarts.com/gist/Language
gist:Language rdf:type owl:Class ;
              owl:disjointWith gist:Magnitude ,
                               gist:Organization ,
                               gist:PhysicalIdentifiableItem ,
                               gist:PhysicalSubstance ,
                               gist:UnitOfMeasure ;
              rdfs:isDefinedBy <https://ontologies.semanticarts.com/o/gistCore> ;
              skos:definition "A recognized, organized set of symbols and grammar." ;
              skos:example "Natural languages such as English and Spanish; computer languages such as OWL, Python, and XML." ;
              skos:prefLabel "Language" .


###  https://ontologies.semanticarts.com/gist/LivingThing
gist:LivingThing rdf:type owl:Class ;
                 owl:equivalentClass [ owl:intersectionOf ( gist:PhysicalIdentifiableItem
                                                            [ rdf:type owl:Restriction ;
                                                              owl:onProperty gist:hasBiologicalParent ;
                                                              owl:minCardinality "1"^^xsd:nonNegativeInteger
                                                            ]
                                                            [ rdf:type owl:Restriction ;
                                                              owl:onProperty gist:birthDate ;
                                                              owl:cardinality "1"^^xsd:nonNegativeInteger
                                                            ]
                                                          ) ;
                                       rdf:type owl:Class
                                     ] ;
                 rdfs:isDefinedBy <https://ontologies.semanticarts.com/o/gistCore> ;
                 skos:definition "Something that is currently, or at some point in time was, alive." ;
                 skos:example "A cat, a mushroom, a tree." ,
                              "Negative examples: fictional life forms such as unicorns or Mickey Mouse." ;
                 skos:prefLabel "Living Thing" ;
                 skos:scopeNote "Not all life forms have exactly two parents, so the restriction only specifies a minimum of one." .


###  https://ontologies.semanticarts.com/gist/LuminousIntensity
gist:LuminousIntensity rdf:type owl:Class ;
                       owl:equivalentClass [ owl:intersectionOf ( gist:Magnitude
                                                                  [ rdf:type owl:Restriction ;
                                                                    owl:onProperty gist:hasUnitOfMeasure ;
                                                                    owl:someValuesFrom gist:LuminousIntensityUnit
                                                                  ]
                                                                ) ;
                                             rdf:type owl:Class
                                           ] ;
                       rdfs:isDefinedBy <https://ontologies.semanticarts.com/o/gistCore> ;
                       skos:definition "A measure of the wavelength-weighted power emitted by a light source in a particular direction per unit solid angle.  This is based on the luminosity function, a standardized model of the sensitivity of the human eye." ;
                       skos:prefLabel "Luminous Intensity" .


###  https://ontologies.semanticarts.com/gist/LuminousIntensityUnit
gist:LuminousIntensityUnit rdf:type owl:Class ;
                           owl:equivalentClass [ owl:intersectionOf ( gist:SimpleUnitOfMeasure
                                                                      [ rdf:type owl:Restriction ;
                                                                        owl:onProperty gist:hasBaseUnit ;
                                                                        owl:hasValue gist:_candela
                                                                      ]
                                                                    ) ;
                                                 rdf:type owl:Class
                                               ] ;
                           owl:disjointWith gist:MassUnit ,
                                            gist:MoleUnit ,
                                            gist:TemperatureUnit ;
                           rdfs:isDefinedBy <https://ontologies.semanticarts.com/o/gistCore> ;
                           skos:definition "The measure of brightness. The SI unit is the candela." ;
                           skos:prefLabel "Luminous Intensity Unit" .


###  https://ontologies.semanticarts.com/gist/Magnitude
gist:Magnitude rdf:type owl:Class ;
               owl:equivalentClass [ owl:intersectionOf ( [ rdf:type owl:Restriction ;
                                                            owl:onProperty gist:hasPrecision ;
                                                            owl:someValuesFrom gist:Magnitude
                                                          ]
                                                          [ rdf:type owl:Restriction ;
                                                            owl:onProperty gist:hasUnitOfMeasure ;
                                                            owl:someValuesFrom gist:UnitOfMeasure
                                                          ]
                                                          [ rdf:type owl:Restriction ;
                                                            owl:onProperty gist:numericValue ;
                                                            owl:someValuesFrom xsd:double
                                                          ]
                                                        ) ;
                                     rdf:type owl:Class
                                   ] ;
               owl:disjointWith gist:Organization ,
                                gist:PhysicalIdentifiableItem ,
                                gist:PhysicalSubstance ,
                                gist:UnitOfMeasure ;
               rdfs:isDefinedBy <https://ontologies.semanticarts.com/o/gistCore> ;
               skos:definition "Base class for units which can be converted.  The primitive units can be converted from one measurement system to another; the complex units (ratio or product) have to decompose to their primitives." ;
               skos:prefLabel "Magnitude" ;
               skos:scopeNote "Magnitudes of the same dimensional type (i.e., duration or electric current) can be compared with a greater-than or less-than operator, but can still differ in their relationToTheWorld type.  (I.e., you can compare actuals to estimates or references, so long as the dimension is the same.)" ,
                              "The precision should be in the same type of unit as the magnitude." .


###  https://ontologies.semanticarts.com/gist/Mass
gist:Mass rdf:type owl:Class ;
          owl:equivalentClass [ owl:intersectionOf ( gist:Magnitude
                                                     [ rdf:type owl:Restriction ;
                                                       owl:onProperty gist:hasUnitOfMeasure ;
                                                       owl:someValuesFrom gist:MassUnit
                                                     ]
                                                   ) ;
                                rdf:type owl:Class
                              ] ;
          rdfs:isDefinedBy <https://ontologies.semanticarts.com/o/gistCore> ;
          skos:definition "Magnitude of mass." ;
          skos:prefLabel "Mass" .


###  https://ontologies.semanticarts.com/gist/MassUnit
gist:MassUnit rdf:type owl:Class ;
              owl:equivalentClass [ owl:intersectionOf ( gist:SimpleUnitOfMeasure
                                                         [ rdf:type owl:Restriction ;
                                                           owl:onProperty gist:hasBaseUnit ;
                                                           owl:hasValue gist:_kilogram
                                                         ]
                                                       ) ;
                                    rdf:type owl:Class
                                  ] ;
              owl:disjointWith gist:MoleUnit ,
                               gist:TemperatureUnit ;
              rdfs:isDefinedBy <https://ontologies.semanticarts.com/o/gistCore> ;
              skos:definition "A unit representing the amount of matter in a particle or object.  The SI unit of mass is the kilogram." ;
              skos:prefLabel "Mass Unit" .


###  https://ontologies.semanticarts.com/gist/MediaType
gist:MediaType rdf:type owl:Class ;
               rdfs:subClassOf gist:Category ;
               rdfs:isDefinedBy <https://ontologies.semanticarts.com/o/gistCore> ;
               rdfs:seeAlso <https://www.iana.org/assignments/media-types/media-types.xhtml> ;
               skos:definition "A digitized type that computer applications can recognize." ;
               skos:prefLabel "Media Type" .


###  https://ontologies.semanticarts.com/gist/Medium
gist:Medium rdf:type owl:Class ;
            rdfs:subClassOf gist:Category ;
            rdfs:isDefinedBy <https://ontologies.semanticarts.com/o/gistCore> ;
            skos:definition "A physicality on which a work could be implemented or exposed. E.g., paper, clay, or a computer monitor." ;
            skos:prefLabel "Medium" .


###  https://ontologies.semanticarts.com/gist/Message
gist:Message rdf:type owl:Class ;
             owl:equivalentClass [ owl:intersectionOf ( gist:ContentExpression
                                                        [ rdf:type owl:Restriction ;
                                                          owl:onProperty gist:comesFromAgent ;
                                                          owl:someValuesFrom [ rdf:type owl:Class ;
                                                                               owl:unionOf ( gist:Organization
                                                                                             gist:Person
                                                                                           )
                                                                             ]
                                                        ]
                                                        [ rdf:type owl:Restriction ;
                                                          owl:onProperty gist:goesToAgent ;
                                                          owl:someValuesFrom [ rdf:type owl:Class ;
                                                                               owl:unionOf ( gist:Organization
                                                                                             gist:Person
                                                                                           )
                                                                             ]
                                                        ]
                                                      ) ;
                                   rdf:type owl:Class
                                 ] ;
             rdfs:isDefinedBy <https://ontologies.semanticarts.com/o/gistCore> ;
             skos:definition "A specific instance of content sent from an Organization or Person to at least one other Organization or Person." ;
             skos:example "An email message, a phone call, a voice message, or a Web Service message." ;
             skos:prefLabel "Message" .


###  https://ontologies.semanticarts.com/gist/MessageDefinition
gist:MessageDefinition rdf:type owl:Class ;
                       rdfs:subClassOf gist:SchemaMetaData ;
                       rdfs:isDefinedBy <https://ontologies.semanticarts.com/o/gistCore> ;
                       skos:definition "Each pulse from a Sensor is reflected in a message, as well as each instruction to an Actuator" ;
                       skos:prefLabel "Message Definition" .


###  https://ontologies.semanticarts.com/gist/MolarQuantity
gist:MolarQuantity rdf:type owl:Class ;
                   owl:equivalentClass [ owl:intersectionOf ( gist:Magnitude
                                                              [ rdf:type owl:Restriction ;
                                                                owl:onProperty gist:hasUnitOfMeasure ;
                                                                owl:someValuesFrom gist:MoleUnit
                                                              ]
                                                            ) ;
                                         rdf:type owl:Class
                                       ] ;
                   rdfs:isDefinedBy <https://ontologies.semanticarts.com/o/gistCore> ;
                   skos:definition "Amount of a substance, as counted molecules." ;
                   skos:prefLabel "Molar Quantity" .


###  https://ontologies.semanticarts.com/gist/MoleUnit
gist:MoleUnit rdf:type owl:Class ;
              owl:equivalentClass [ owl:intersectionOf ( gist:SimpleUnitOfMeasure
                                                         [ rdf:type owl:Restriction ;
                                                           owl:onProperty gist:hasBaseUnit ;
                                                           owl:hasValue gist:_mole
                                                         ]
                                                       ) ;
                                    rdf:type owl:Class
                                  ] ;
              owl:disjointWith gist:TemperatureUnit ;
              rdfs:isDefinedBy <https://ontologies.semanticarts.com/o/gistCore> ;
              skos:definition "Amount of chemical material.  Measured in Avogadro units (moles) of 6.02 x 10^23 molecules." ;
              skos:prefLabel "Mole Unit" .


###  https://ontologies.semanticarts.com/gist/Monetary
gist:Monetary rdf:type owl:Class ;
              owl:equivalentClass [ owl:intersectionOf ( gist:Magnitude
                                                         [ rdf:type owl:Restriction ;
                                                           owl:onProperty gist:hasUnitOfMeasure ;
                                                           owl:someValuesFrom gist:CurrencyUnit
                                                         ]
                                                       ) ;
                                    rdf:type owl:Class
                                  ] ;
              rdfs:isDefinedBy <https://ontologies.semanticarts.com/o/gistCore> ;
              skos:definition "A special type of magnitude, due to the way rounding is handled in math and the temporal aspect of conversion." ;
              skos:prefLabel "Monetary" .


###  https://ontologies.semanticarts.com/gist/Network
gist:Network rdf:type owl:Class ;
             owl:equivalentClass [ owl:intersectionOf ( gist:Artifact
                                                        [ rdf:type owl:Restriction ;
                                                          owl:onProperty gist:hasMember ;
                                                          owl:someValuesFrom [ rdf:type owl:Class ;
                                                                               owl:unionOf ( gist:NetworkLink
                                                                                             gist:NetworkNode
                                                                                           )
                                                                             ]
                                                        ]
                                                      ) ;
                                   rdf:type owl:Class
                                 ] ;
             rdfs:isDefinedBy <https://ontologies.semanticarts.com/o/gistCore> ;
             skos:definition "A network is a set of nodes connected by links." ;
             skos:example "A physical network could include connected computers or routers, whereas a social network would consist of related Person or Organization instances." ;
             skos:prefLabel "Network" .


###  https://ontologies.semanticarts.com/gist/NetworkLink
gist:NetworkLink rdf:type owl:Class ;
                 owl:equivalentClass [ owl:intersectionOf ( [ rdf:type owl:Restriction ;
                                                              owl:onProperty gist:isMemberOf ;
                                                              owl:someValuesFrom gist:Network
                                                            ]
                                                            [ rdf:type owl:Restriction ;
                                                              owl:onProperty gist:links ;
                                                              owl:allValuesFrom gist:NetworkNode
                                                            ]
                                                            [ rdf:type owl:Restriction ;
                                                              owl:onProperty gist:links ;
                                                              owl:qualifiedCardinality "2"^^xsd:nonNegativeInteger ;
                                                              owl:onClass gist:NetworkNode
                                                            ]
                                                          ) ;
                                       rdf:type owl:Class
                                     ] ;
                 rdfs:isDefinedBy <https://ontologies.semanticarts.com/o/gistCore> ;
                 skos:definition "An abstract representation of the connection between two or more nodes in a network." ;
                 skos:example "A network link may be physical, such as pipes, wired or wireless networks, but may also be a link in a non-physical network, such as organizational structures or social networks." ;
                 skos:prefLabel "Network Link" ;
                 skos:scopeNote "Each NetworkLink is connected to a NetworkNode via the property 'gist:links' or one of its subproperties." .


###  https://ontologies.semanticarts.com/gist/NetworkNode
gist:NetworkNode rdf:type owl:Class ;
                 rdfs:subClassOf [ rdf:type owl:Restriction ;
                                   owl:onProperty gist:isMemberOf ;
                                   owl:someValuesFrom gist:Network
                                 ] ;
                 rdfs:isDefinedBy <https://ontologies.semanticarts.com/o/gistCore> ;
                 skos:definition "A node in a network." ;
                 skos:example "A person is a node in a social network; a valve is a node in a network of pipes." ;
                 skos:prefLabel "Network Node" .


###  https://ontologies.semanticarts.com/gist/Obligation
gist:Obligation rdf:type owl:Class ;
                owl:equivalentClass [ owl:intersectionOf ( gist:Commitment
                                                           [ rdf:type owl:Restriction ;
                                                             owl:onProperty gist:hasGiver ;
                                                             owl:someValuesFrom [ rdf:type owl:Class ;
                                                                                  owl:unionOf ( gist:Organization
                                                                                                gist:Person
                                                                                              )
                                                                                ]
                                                           ]
                                                           [ rdf:type owl:Restriction ;
                                                             owl:onProperty gist:hasRecipient ;
                                                             owl:someValuesFrom [ rdf:type owl:Class ;
                                                                                  owl:unionOf ( gist:Organization
                                                                                                gist:Person
                                                                                              )
                                                                                ]
                                                           ]
                                                         ) ;
                                      rdf:type owl:Class
                                    ] ;
                rdfs:isDefinedBy <https://ontologies.semanticarts.com/o/gistCore> ;
                skos:definition "A future commitment from one organization or person to another. Contracts are sets of obligations to do or forbear, or to indemnify or warrant." ;
                skos:prefLabel "Obligation" ;
                skos:scopeNote "Obligations will often be governed by some Agreement or Offer." .


###  https://ontologies.semanticarts.com/gist/Offer
gist:Offer rdf:type owl:Class ;
           owl:equivalentClass [ owl:intersectionOf ( gist:ContingentObligation
                                                      [ rdf:type owl:Restriction ;
                                                        owl:onProperty gist:hasDirectPart ;
                                                        owl:someValuesFrom gist:CatalogItem
                                                      ]
                                                      [ rdf:type owl:Restriction ;
                                                        owl:onProperty gist:hasGiver ;
                                                        owl:someValuesFrom [ rdf:type owl:Class ;
                                                                             owl:unionOf ( gist:Organization
                                                                                           gist:Person
                                                                                         )
                                                                           ]
                                                      ]
                                                      [ rdf:type owl:Restriction ;
                                                        owl:onProperty gist:hasMagnitude ;
                                                        owl:someValuesFrom gist:Monetary
                                                      ]
                                                      [ rdf:type owl:Restriction ;
                                                        owl:onProperty gist:plannedEndDateTime ;
                                                        owl:cardinality "1"^^xsd:nonNegativeInteger
                                                      ]
                                                      [ rdf:type owl:Restriction ;
                                                        owl:onProperty gist:plannedStartDateTime ;
                                                        owl:cardinality "1"^^xsd:nonNegativeInteger
                                                      ]
                                                    ) ;
                                 rdf:type owl:Class
                               ] ;
           rdfs:isDefinedBy <https://ontologies.semanticarts.com/o/gistCore> ;
           skos:definition "A commitment to buy or sell a described or identified part or service." ;
           skos:prefLabel "Offer" .


###  https://ontologies.semanticarts.com/gist/OrderedCollection
gist:OrderedCollection rdf:type owl:Class ;
                       owl:equivalentClass [ owl:intersectionOf ( gist:Collection
                                                                  [ rdf:type owl:Class ;
                                                                    owl:unionOf ( [ rdf:type owl:Restriction ;
                                                                                    owl:onProperty gist:hasFirstMember ;
                                                                                    owl:someValuesFrom owl:Thing
                                                                                  ]
                                                                                  [ rdf:type owl:Restriction ;
                                                                                    owl:onProperty gist:hasMember ;
                                                                                    owl:cardinality "0"^^xsd:nonNegativeInteger
                                                                                  ]
                                                                                )
                                                                  ]
                                                                  [ rdf:type owl:Restriction ;
                                                                    owl:onProperty gist:hasMember ;
                                                                    owl:allValuesFrom gist:OrderedMember
                                                                  ]
                                                                ) ;
                                             rdf:type owl:Class
                                           ] ;
                       rdfs:isDefinedBy <https://ontologies.semanticarts.com/o/gistCore> ;
                       skos:definition "A collection in which the members are sequentially ordered. All members of an OrderedCollection are OrderedMembers." ;
                       skos:prefLabel "Ordered Collection" ;
                       skos:scopeNote "Includes collections in which members occupy the same position in a 'tie.'" .


###  https://ontologies.semanticarts.com/gist/OrderedMember
gist:OrderedMember rdf:type owl:Class ;
                   owl:equivalentClass [ owl:intersectionOf ( [ rdf:type owl:Class ;
                                                                owl:unionOf ( [ rdf:type owl:Restriction ;
                                                                                owl:onProperty gist:followsDirectly ;
                                                                                owl:someValuesFrom gist:OrderedMember
                                                                              ]
                                                                              [ rdf:type owl:Restriction ;
                                                                                owl:onProperty gist:precedesDirectly ;
                                                                                owl:someValuesFrom gist:OrderedMember
                                                                              ]
                                                                              [ rdf:type owl:Restriction ;
                                                                                owl:onProperty gist:sequence ;
                                                                                owl:someValuesFrom xsd:integer
                                                                              ]
                                                                            )
                                                              ]
                                                              [ rdf:type owl:Restriction ;
                                                                owl:onProperty gist:isMemberOf ;
                                                                owl:allValuesFrom gist:OrderedCollection
                                                              ]
                                                              [ rdf:type owl:Restriction ;
                                                                owl:onProperty gist:isMemberOf ;
                                                                owl:cardinality "1"^^xsd:nonNegativeInteger
                                                              ]
                                                            ) ;
                                         rdf:type owl:Class
                                       ] ;
                   rdfs:isDefinedBy <https://ontologies.semanticarts.com/o/gistCore> ;
                   skos:definition "A member of an ordered collection serving as a proxy for a real world item, which can appear in different orders in different collections. The ordered member appears in exactly one ordered collection." ;
                   skos:example "A person may rank 12th in the Boston Marathon but 29th in the New York City Marathon." ;
                   skos:prefLabel "Ordered Member" ;
                   skos:scopeNote "An ordered member points to the real world item via the providesOrderFor property. Ordering information is represented either as a number in a sequence, or by preceding or following another ordered member." .


###  https://ontologies.semanticarts.com/gist/Organization
gist:Organization rdf:type owl:Class ;
                  owl:disjointWith gist:PhysicalIdentifiableItem ,
                                   gist:PhysicalSubstance ,
                                   gist:SchemaMetaData ,
                                   gist:UnitOfMeasure ;
                  rdfs:isDefinedBy <https://ontologies.semanticarts.com/o/gistCore> ;
                  skos:definition "A generic organization that can be formal or informal, legal or non-legal. It can have members, or not." ;
                  skos:example "Legal entities like companies; non-legal entities like clubs, committees, or departments." ;
                  skos:prefLabel "Organization" ;
                  skos:scopeNote "There are a plethora of different kinds of organizations that differ along many facets, including members, structure, purpose, legal vs. non-legal, etc." .


###  https://ontologies.semanticarts.com/gist/Percentage
gist:Percentage rdf:type owl:Class ;
                rdfs:subClassOf gist:RatioMagnitude ;
                rdfs:isDefinedBy <https://ontologies.semanticarts.com/o/gistCore> ;
                skos:definition "A ratio where the numerator and denominator are of the same unit of measure." ;
                skos:prefLabel "Percentage" ;
                skos:scopeNote "There are various ways to represent percentage: 50/100 could be represented as ?50? or ?0.5?.  gist uses the latter, as it involves fewer conversions for subsequent use." .


###  https://ontologies.semanticarts.com/gist/Permission
gist:Permission rdf:type owl:Class ;
                owl:equivalentClass [ owl:intersectionOf ( gist:Intention
                                                           [ rdf:type owl:Restriction ;
                                                             owl:onProperty gist:allows ;
                                                             owl:someValuesFrom gist:Behavior
                                                           ]
                                                         ) ;
                                      rdf:type owl:Class
                                    ] ;
                rdfs:isDefinedBy <https://ontologies.semanticarts.com/o/gistCore> ;
                skos:definition "A description of things one is permitted to do. This could be broad, such as free speech, but more often is very specific, such as the right of egress through a particular property." ;
                skos:prefLabel "Permission" .


###  https://ontologies.semanticarts.com/gist/Person
gist:Person rdf:type owl:Class ;
            owl:equivalentClass [ owl:intersectionOf ( gist:LivingThing
                                                       [ rdf:type owl:Restriction ;
                                                         owl:onProperty gist:hasBiologicalParent ;
                                                         owl:allValuesFrom gist:Person
                                                       ]
                                                     ) ;
                                  rdf:type owl:Class
                                ] ;
            rdfs:isDefinedBy <https://ontologies.semanticarts.com/o/gistCore> ;
            skos:definition "A human being that may or may not still be alive." ;
            skos:example "Negative example:fictional characters." ;
            skos:prefLabel "Person" .


###  https://ontologies.semanticarts.com/gist/PhenomenaType
gist:PhenomenaType rdf:type owl:Class ;
                   rdfs:subClassOf gist:Category ;
                   rdfs:isDefinedBy <https://ontologies.semanticarts.com/o/gistCore> ;
                   skos:definition "The things that a sensor can sense, such as light, heat, current, moisture, etc." ;
                   skos:prefLabel "Phenomena Type" .


###  https://ontologies.semanticarts.com/gist/PhysicalActionType
gist:PhysicalActionType rdf:type owl:Class ;
                        rdfs:subClassOf gist:Category ;
                        rdfs:isDefinedBy <https://ontologies.semanticarts.com/o/gistCore> ;
                        skos:definition "The effects to be realized in the real world, such as lifting a garage door, turning off a valve, dropping cadmium rods, etc." ;
                        skos:prefLabel "Physical Action Type" .


###  https://ontologies.semanticarts.com/gist/PhysicalEvent
gist:PhysicalEvent rdf:type owl:Class ;
                   owl:equivalentClass [ owl:intersectionOf ( gist:Event
                                                              [ rdf:type owl:Restriction ;
                                                                owl:onProperty gist:occursIn ;
                                                                owl:someValuesFrom gist:Place
                                                              ]
                                                            ) ;
                                         rdf:type owl:Class
                                       ] ;
                   rdfs:isDefinedBy <https://ontologies.semanticarts.com/o/gistCore> ;
                   skos:definition "An event that can be said to have occurred at some place in space." ;
                   skos:example "A meeting, a car accident." ,
                                "Negative examples: Excludes events that have no meaningful location, such as financial events or project milestones." ;
                   skos:prefLabel "Physical Event" .


###  https://ontologies.semanticarts.com/gist/PhysicalIdentifiableItem
gist:PhysicalIdentifiableItem rdf:type owl:Class ;
                              rdfs:subClassOf [ rdf:type owl:Restriction ;
                                                owl:onProperty gist:hasMagnitude ;
                                                owl:someValuesFrom gist:Mass
                                              ] ,
                                              [ rdf:type owl:Restriction ;
                                                owl:onProperty gist:hasMagnitude ;
                                                owl:someValuesFrom gist:Volume
                                              ] ,
                                              [ rdf:type owl:Restriction ;
                                                owl:onProperty gist:isMadeUpOf ;
                                                owl:someValuesFrom gist:PhysicalSubstance
                                              ] ;
                              owl:disjointWith gist:SchemaMetaData ,
                                               gist:UnitOfMeasure ;
                              rdfs:isDefinedBy <https://ontologies.semanticarts.com/o/gistCore> ;
                              skos:definition "A discrete physical object which, if subdivided, will result in parts that are distinguishable in nature from the whole and in general also from the other parts." ;
                              skos:example "A computer, book, car." ;
                              skos:prefLabel "Physical Identifiable Item" ;
                              skos:scopeNote "This concept generally corresponds to count nouns in English. By contrast, instances of PhysicalSubstance, such as an amount of water, flour, or sand, are mass nouns. PhysicalIdentifiableItems are made up of PhysicalSubstances; e.g., a cake is made up of butter, flour, and sugar; a statue is made of bronze. If you divide a PhysicalSubstance such as an amount of water into parts, you have two amounts of water otherwise indistinguishable from one another; if you divide a PhysicalIdentifiableItem such as a computer into parts, each part is different from the whole." .


###  https://ontologies.semanticarts.com/gist/PhysicalSubstance
gist:PhysicalSubstance rdf:type owl:Class ;
                       rdfs:subClassOf [ rdf:type owl:Restriction ;
                                         owl:onProperty gist:hasMagnitude ;
                                         owl:someValuesFrom gist:Mass
                                       ] ,
                                       [ rdf:type owl:Restriction ;
                                         owl:onProperty gist:hasMagnitude ;
                                         owl:someValuesFrom gist:Volume
                                       ] ;
                       owl:disjointWith gist:UnitOfMeasure ;
                       rdfs:isDefinedBy <https://ontologies.semanticarts.com/o/gistCore> ;
                       skos:definition "An undifferentiated amount of physical material which, when subdivided, results in each part being indistinguishable in nature from the whole and from every other part." ;
                       skos:example "An amount of water, penicillin, sand, gold: an actual piece of gold, not the concept of gold." ;
                       skos:prefLabel "Physical Substance" ;
                       skos:scopeNote "An instance of this class has weight and takes up space. We mean the physical gold in a ring, not the concept of gold that shows up in the periodic table." ,
                                      "This concept generally corresponds to mass nouns in English. By contrast, instances of PhysicalIdentifiableItem, such as a computer, book, or car, are count nouns. PhysicalIdentifiableItems are made up of PhysicalSubstances; e.g., a cake is made up of butter, flour, and sugar; a ring is made of gold. If you divide a PhysicalSubstance such as an amount of water into parts, you have different amounts of water otherwise indistinguishable from one another; if you divide a PhysicalIdentifiableItem such as a computer into parts, each part will be distinguishable from the original whole." .


###  https://ontologies.semanticarts.com/gist/Place
gist:Place rdf:type owl:Class ;
           rdfs:isDefinedBy <https://ontologies.semanticarts.com/o/gistCore> ;
           skos:definition "Union of all the geo classes" ;
           skos:prefLabel "Place" .


###  https://ontologies.semanticarts.com/gist/PlannedEvent
gist:PlannedEvent rdf:type owl:Class ;
                  owl:equivalentClass [ owl:intersectionOf ( gist:Event
                                                             [ rdf:type owl:Restriction ;
                                                               owl:onProperty gist:plannedEndDateTime ;
                                                               owl:cardinality "1"^^xsd:nonNegativeInteger
                                                             ]
                                                             [ rdf:type owl:Restriction ;
                                                               owl:onProperty gist:plannedStartDateTime ;
                                                               owl:cardinality "1"^^xsd:nonNegativeInteger
                                                             ]
                                                           ) ;
                                        rdf:type owl:Class
                                      ] ;
                  rdfs:isDefinedBy <https://ontologies.semanticarts.com/o/gistCore> ;
                  skos:definition "An event which, at the time it is created, is to occur in the future." ;
                  skos:prefLabel "Planned Event" .


###  https://ontologies.semanticarts.com/gist/PostalAddress
gist:PostalAddress rdf:type owl:Class ;
                   rdfs:subClassOf gist:Address ;
                   rdfs:isDefinedBy <https://ontologies.semanticarts.com/o/gistCore> ;
                   skos:definition "A set of codes the postal authorities can use to deliver physical mail." ;
                   skos:example "A street address, a PO Box, an FPO code, or the route codes." ;
                   skos:prefLabel "Postal Address" .


###  https://ontologies.semanticarts.com/gist/ProductCategory
gist:ProductCategory rdf:type owl:Class ;
                     rdfs:subClassOf gist:Category ;
                     rdfs:isDefinedBy <https://ontologies.semanticarts.com/o/gistCore> ;
                     skos:definition "Any of many ways of categorizing products, including models, NATO product codes, and the like." ;
                     skos:prefLabel "Product Category" .


###  https://ontologies.semanticarts.com/gist/ProductMagnitude
gist:ProductMagnitude rdf:type owl:Class ;
                      owl:equivalentClass [ owl:intersectionOf ( gist:Magnitude
                                                                 [ rdf:type owl:Restriction ;
                                                                   owl:onProperty gist:hasUnitOfMeasure ;
                                                                   owl:someValuesFrom gist:ProductUnit
                                                                 ]
                                                               ) ;
                                            rdf:type owl:Class
                                          ] ;
                      rdfs:isDefinedBy <https://ontologies.semanticarts.com/o/gistCore> ;
                      skos:definition "A magnitude expressed as a product of primitives.  (E.g., Force = M*A)." ;
                      skos:prefLabel "Product Magnitude" .


###  https://ontologies.semanticarts.com/gist/ProductSpecification
gist:ProductSpecification rdf:type owl:Class ;
                          owl:equivalentClass [ owl:intersectionOf ( gist:CatalogItem
                                                                     [ rdf:type owl:Restriction ;
                                                                       owl:onProperty gist:isCategorizedBy ;
                                                                       owl:someValuesFrom gist:ProductCategory
                                                                     ]
                                                                   ) ;
                                                rdf:type owl:Class
                                              ] ;
                          rdfs:isDefinedBy <https://ontologies.semanticarts.com/o/gistCore> ;
                          skos:definition "Offering something which could be physically warehoused or digitally stored." ;
                          skos:prefLabel "Product Specification" .


###  https://ontologies.semanticarts.com/gist/ProductUnit
gist:ProductUnit rdf:type owl:Class ;
                 owl:equivalentClass [ owl:intersectionOf ( gist:UnitOfMeasure
                                                            [ rdf:type owl:Restriction ;
                                                              owl:onProperty gist:hasMultiplicand ;
                                                              owl:someValuesFrom gist:UnitOfMeasure
                                                            ]
                                                            [ rdf:type owl:Restriction ;
                                                              owl:onProperty gist:hasMultiplier ;
                                                              owl:someValuesFrom gist:UnitOfMeasure
                                                            ]
                                                          ) ;
                                       rdf:type owl:Class
                                     ] ;
                 rdfs:isDefinedBy <https://ontologies.semanticarts.com/o/gistCore> ;
                 skos:definition "A unit of measure that is the product of two simpler ones." ;
                 skos:example "Area and Volume are the classic cases.  But other, more exotic cases exist, such as Newtons." ;
                 skos:prefLabel "Product Unit" ;
                 skos:scopeNote "A ProductUnit is intended have a value for conversionFactor." .


###  https://ontologies.semanticarts.com/gist/ProjectExecution
gist:ProjectExecution rdf:type owl:Class ;
                      owl:equivalentClass [ owl:intersectionOf ( gist:TaskExecution
                                                                 [ rdf:type owl:Restriction ;
                                                                   owl:onProperty gist:hasSubTask ;
                                                                   owl:someValuesFrom gist:TaskExecution
                                                                 ]
                                                               ) ;
                                            rdf:type owl:Class
                                          ] ;
                      rdfs:isDefinedBy <https://ontologies.semanticarts.com/o/gistCore> ;
                      skos:definition "A project execution is a task execution (usually a longer duration task) made up of other task executions." ;
                      skos:prefLabel "Project Execution" .


###  https://ontologies.semanticarts.com/gist/RatioMagnitude
gist:RatioMagnitude rdf:type owl:Class ;
                    owl:equivalentClass [ owl:intersectionOf ( gist:Magnitude
                                                               [ rdf:type owl:Restriction ;
                                                                 owl:onProperty gist:hasUnitOfMeasure ;
                                                                 owl:someValuesFrom gist:RatioUnit
                                                               ]
                                                             ) ;
                                          rdf:type owl:Class
                                        ] ;
                    rdfs:isDefinedBy <https://ontologies.semanticarts.com/o/gistCore> ;
                    skos:definition "This is a number whose unit of measure is a ratio." ;
                    skos:example "Speed.  The ratio magnitude is 60, the unit of measure might be MilesPerHour." ;
                    skos:prefLabel "Ratio Magnitude" ;
                    skos:scopeNote "A RatioMagnitude just has one decimal value." .


###  https://ontologies.semanticarts.com/gist/RatioUnit
gist:RatioUnit rdf:type owl:Class ;
               owl:equivalentClass [ owl:intersectionOf ( gist:UnitOfMeasure
                                                          [ rdf:type owl:Restriction ;
                                                            owl:onProperty gist:hasDenominator ;
                                                            owl:someValuesFrom gist:UnitOfMeasure
                                                          ]
                                                          [ rdf:type owl:Restriction ;
                                                            owl:onProperty gist:hasNumerator ;
                                                            owl:someValuesFrom gist:UnitOfMeasure
                                                          ]
                                                        ) ;
                                     rdf:type owl:Class
                                   ] ;
               rdfs:isDefinedBy <https://ontologies.semanticarts.com/o/gistCore> ;
               skos:definition "A UnitOfMeasure composed of a numerator unit and a denominator unit." ;
               skos:example "Miles per hour." ;
               skos:prefLabel "Ratio Unit" ;
               skos:scopeNote "If needed, a conversion factor for a RatioUnit can be (recursively) derived from the conversion factors of the numerator and denominator units.  E.g., the derived conversion factor from km/minute to meters/second is 1000/60 or 16 2/3." .


###  https://ontologies.semanticarts.com/gist/ReferenceValue
gist:ReferenceValue rdf:type owl:Class ;
                    rdfs:subClassOf gist:Magnitude ;
                    rdfs:isDefinedBy <https://ontologies.semanticarts.com/o/gistCore> ;
                    skos:definition "A measure that was neither measured nor estimated but set by fiat. For instance, a goal. There is no Measurement associated with a ReferenceValue." ;
                    skos:prefLabel "Reference Value" .


###  https://ontologies.semanticarts.com/gist/RenderedContent
gist:RenderedContent rdf:type owl:Class ;
                     owl:equivalentClass [ owl:intersectionOf ( gist:ContentExpression
                                                                [ rdf:type owl:Restriction ;
                                                                  owl:onProperty gist:isExpressedIn ;
                                                                  owl:someValuesFrom gist:MediaType
                                                                ]
                                                                [ rdf:type owl:Restriction ;
                                                                  owl:onProperty gist:isRenderedOn ;
                                                                  owl:someValuesFrom gist:Medium
                                                                ]
                                                              ) ;
                                           rdf:type owl:Class
                                         ] ;
                     rdfs:isDefinedBy <https://ontologies.semanticarts.com/o/gistCore> ;
                     skos:definition "Content which has been expressed, either to print, or through speakers, or on a monitor." ;
                     skos:prefLabel "Rendered Content" .


###  https://ontologies.semanticarts.com/gist/Requirement
gist:Requirement rdf:type owl:Class ;
                 rdfs:subClassOf gist:Intention ;
                 rdfs:isDefinedBy <https://ontologies.semanticarts.com/o/gistCore> ;
                 skos:definition "A documented physical or functional need that a particular design, product, or process must be able to perform.  Alternately, the obligation of a person or organization to behave in a certain way (i.e., drive on the right side of the road)." ;
                 skos:prefLabel "Requirement" .


###  https://ontologies.semanticarts.com/gist/Restriction
gist:Restriction rdf:type owl:Class ;
                 owl:equivalentClass [ owl:intersectionOf ( gist:Intention
                                                            [ rdf:type owl:Restriction ;
                                                              owl:onProperty gist:prevents ;
                                                              owl:someValuesFrom gist:Behavior
                                                            ]
                                                          ) ;
                                       rdf:type owl:Class
                                     ] ;
                 rdfs:isDefinedBy <https://ontologies.semanticarts.com/o/gistCore> ;
                 skos:definition "A description of things one is prevented from doing.  Most laws are restrictions." ;
                 skos:prefLabel "Restriction" .


###  https://ontologies.semanticarts.com/gist/ScheduledTaskExecution
gist:ScheduledTaskExecution rdf:type owl:Class ;
                            owl:equivalentClass [ owl:intersectionOf ( gist:PlannedEvent
                                                                       gist:TaskExecution
                                                                     ) ;
                                                  rdf:type owl:Class
                                                ] ;
                            rdfs:isDefinedBy <https://ontologies.semanticarts.com/o/gistCore> ;
                            skos:definition "The execution of a task that was planned to occur at a given time. When it was scheduled, it would have been in the future, but now might be in the past." ;
                            skos:prefLabel "Scheduled Task Execution" .


###  https://ontologies.semanticarts.com/gist/SchemaMetaData
gist:SchemaMetaData rdf:type owl:Class ;
                    owl:disjointWith gist:UnitOfMeasure ;
                    rdfs:isDefinedBy <https://ontologies.semanticarts.com/o/gistCore> ;
                    skos:definition "Superclass for all types of metadata, including owl concepts (such as class) and relational (tables, elements) and tool related (queries, R2RML maps etc etc)" ;
                    skos:prefLabel "Schema Meta Data" .


###  https://ontologies.semanticarts.com/gist/Sensor
gist:Sensor rdf:type owl:Class ;
            rdfs:subClassOf gist:Equipment ;
            rdfs:isDefinedBy <https://ontologies.semanticarts.com/o/gistCore> ;
            skos:definition "A device that can detect something and report it. Light sensors, temperature sensors," ;
            skos:prefLabel "Sensor" .


###  https://ontologies.semanticarts.com/gist/ServiceSpecification
gist:ServiceSpecification rdf:type owl:Class ;
                          owl:equivalentClass [ owl:intersectionOf ( gist:CatalogItem
                                                                     [ rdf:type owl:Restriction ;
                                                                       owl:onProperty gist:isBasisFor ;
                                                                       owl:someValuesFrom gist:Event
                                                                     ]
                                                                   ) ;
                                                rdf:type owl:Class
                                              ] ;
                          rdfs:isDefinedBy <https://ontologies.semanticarts.com/o/gistCore> ;
                          skos:definition "A description of something that can be done for a person or organization (which produces some form of an act)." ;
                          skos:prefLabel "Service Specification" .


###  https://ontologies.semanticarts.com/gist/SimpleUnitOfMeasure
gist:SimpleUnitOfMeasure rdf:type owl:Class ;
                         owl:equivalentClass [ owl:intersectionOf ( gist:UnitOfMeasure
                                                                    [ rdf:type owl:Restriction ;
                                                                      owl:onProperty gist:hasBaseUnit ;
                                                                      owl:qualifiedCardinality "1"^^xsd:nonNegativeInteger ;
                                                                      owl:onClass gist:BaseUnit
                                                                    ]
                                                                    [ rdf:type owl:Restriction ;
                                                                      owl:onProperty gist:conversionFactor ;
                                                                      owl:someValuesFrom xsd:double
                                                                    ]
                                                                  ) ;
                                               rdf:type owl:Class
                                             ] ;
                         rdfs:isDefinedBy <https://ontologies.semanticarts.com/o/gistCore> ;
                         skos:definition "Each simple unit has a base unit and a conversion factor to the base. The bases are from the System International (SI). The conversion factor is the number which one multiplies a Unit by to get to base, or divides by to get from base.  E.g., the conversionFactor for inch is 0.0254 to get to the base unit (meter)." ;
                         skos:prefLabel "Simple Unit Of Measure" .


###  https://ontologies.semanticarts.com/gist/Specification
gist:Specification rdf:type owl:Class ;
                   rdfs:subClassOf gist:Requirement ;
                   rdfs:isDefinedBy <https://ontologies.semanticarts.com/o/gistCore> ;
                   skos:definition "A set of requirements to be satisfied by a material, design, product, or service." ;
                   skos:prefLabel "Specification" .


###  https://ontologies.semanticarts.com/gist/StreetAddress
gist:StreetAddress rdf:type owl:Class ;
                   rdfs:subClassOf gist:PostalAddress ;
                   rdfs:isDefinedBy <https://ontologies.semanticarts.com/o/gistCore> ;
                   skos:definition "An address which references a fixed location in the physical world." ;
                   skos:example "The street address of a building, a park, campground, or an empty lot." ;
                   skos:prefLabel "Street Address" ;
                   skos:scopeNote "This excludes addresses not associated with a fixed location, such as a PO box or FPO code." .


###  https://ontologies.semanticarts.com/gist/SubCountryGovernment
gist:SubCountryGovernment rdf:type owl:Class ;
                          owl:equivalentClass [ owl:intersectionOf ( gist:GovernmentOrganization
                                                                     [ rdf:type owl:Restriction ;
                                                                       owl:onProperty gist:governs ;
                                                                       owl:someValuesFrom gist:GeoRegion
                                                                     ]
                                                                     [ rdf:type owl:Restriction ;
                                                                       owl:onProperty gist:isGovernedBy ;
                                                                       owl:someValuesFrom gist:CountryGovernment
                                                                     ]
                                                                   ) ;
                                                rdf:type owl:Class
                                              ] ;
                          rdfs:isDefinedBy <https://ontologies.semanticarts.com/o/gistCore> ;
                          skos:definition "A government of a governed geo-region other than a country, which is under the direct or indirect control of a country government." ;
                          skos:prefLabel "Sub-Country Government" ;
                          skos:scopeNote "Across the world, there are a variety of types of subsections of a country and the governments thereof (as well as different terms, like 'province' and 'state', which refer to essentially the same type of thing). We should not automatically assume 'state', 'county', and 'city'.  It is more future-proof just to mint the instances using the generic SubCountryGovernment and, where greater specificity is needed, define categories or subclasses." ,
                                         "Note that the predicate 'governs' is used both for the relationship a government has to a governed geo-region, and for the relationship one government has to the governments of its sub-regions." ,
                                         "This class applies only to organizations governing geo-regions. Regulatory and bureaucratic organizations are members of the more generic GovernmentOrganization class." .


###  https://ontologies.semanticarts.com/gist/System
gist:System rdf:type owl:Class ;
            owl:equivalentClass [ owl:intersectionOf ( gist:Artifact
                                                       [ rdf:type owl:Restriction ;
                                                         owl:onProperty gist:hasDirectPart ;
                                                         owl:someValuesFrom gist:Component
                                                       ]
                                                     ) ;
                                  rdf:type owl:Class
                                ] ,
                                [ rdf:type owl:Restriction ;
                                  owl:onProperty <https://ontology.architmitra.org/archimodel/exhibits> ;
                                  owl:someValuesFrom <https://ontology.architmitra.org/archimodel/Architecture>
                                ] ,
                                [ rdf:type owl:Restriction ;
                                  owl:onProperty <https://ontology.architmitra.org/archimodel/situatedIn> ;
                                  owl:someValuesFrom <https://ontology.architmitra.org/archimodel/Environment>
                                ] ;
            rdfs:isDefinedBy <https://ontologies.semanticarts.com/o/gistCore> ;
            skos:definition """A system is an artifact with component parts where the parts contribute to the goal of the system.
Systems can be man-made, natural or conceptual - ISO 42010-2011""" ;
            skos:prefLabel "System" .


###  https://ontologies.semanticarts.com/gist/Tag
gist:Tag rdf:type owl:Class ;
         owl:equivalentClass [ owl:intersectionOf ( gist:Category
                                                    [ rdf:type owl:Restriction ;
                                                      owl:onProperty gist:tagText ;
                                                      owl:someValuesFrom xsd:string
                                                    ]
                                                  ) ;
                               rdf:type owl:Class
                             ] ;
         rdfs:isDefinedBy <https://ontologies.semanticarts.com/o/gistCore> ;
         skos:definition "This is for folksonomy type terms, which can be made up on the fly by users." ;
         skos:prefLabel "Tag" .


###  https://ontologies.semanticarts.com/gist/TaskExecution
gist:TaskExecution rdf:type owl:Class ;
                   owl:equivalentClass [ owl:intersectionOf ( gist:Event
                                                              [ rdf:type owl:Restriction ;
                                                                owl:onProperty gist:hasGoal ;
                                                                owl:someValuesFrom gist:Intention
                                                              ]
                                                            ) ;
                                         rdf:type owl:Class
                                       ] ;
                   rdfs:isDefinedBy <https://ontologies.semanticarts.com/o/gistCore> ;
                   skos:definition "An event characterized by a defined piece of work that is either scheduled, accomplished, or both." ;
                   skos:prefLabel "Task Execution" .


###  https://ontologies.semanticarts.com/gist/TaskTemplate
gist:TaskTemplate rdf:type owl:Class ;
                  owl:equivalentClass [ owl:intersectionOf ( gist:Template
                                                             [ rdf:type owl:Restriction ;
                                                               owl:onProperty gist:hasGoal ;
                                                               owl:someValuesFrom gist:Intention
                                                             ]
                                                           ) ;
                                        rdf:type owl:Class
                                      ] ;
                  rdfs:isDefinedBy <https://ontologies.semanticarts.com/o/gistCore> ;
                  skos:definition "An outline of a task of a particular type, which is the basis for executing such tasks." ;
                  skos:prefLabel "Task Template" ;
                  skos:scopeNote "The class TaskExecution is used to represent the execution of the task. Use the property isBasedOn to link the TaskExecution back to the TaskTemplate." .


###  https://ontologies.semanticarts.com/gist/Taxonomy
gist:Taxonomy rdf:type owl:Class ;
              owl:equivalentClass [ owl:intersectionOf ( gist:ControlledVocabulary
                                                         [ rdf:type owl:Restriction ;
                                                           owl:onProperty gist:hasMember ;
                                                           owl:someValuesFrom [ owl:intersectionOf ( gist:Category
                                                                                                     [ rdf:type owl:Class ;
                                                                                                       owl:unionOf ( [ rdf:type owl:Restriction ;
                                                                                                                       owl:onProperty gist:hasSubCategory ;
                                                                                                                       owl:someValuesFrom gist:Category
                                                                                                                     ]
                                                                                                                     [ rdf:type owl:Restriction ;
                                                                                                                       owl:onProperty gist:hasSuperCategory ;
                                                                                                                       owl:someValuesFrom gist:Category
                                                                                                                     ]
                                                                                                                   )
                                                                                                     ]
                                                                                                   ) ;
                                                                                rdf:type owl:Class
                                                                              ]
                                                         ]
                                                       ) ;
                                    rdf:type owl:Class
                                  ] ;
              rdfs:isDefinedBy <https://ontologies.semanticarts.com/o/gistCore> ;
              skos:definition "A controlled vocabulary arranged as a hierarchy of concepts." ;
              skos:prefLabel "Taxonomy" .


###  https://ontologies.semanticarts.com/gist/TelephoneNumber
gist:TelephoneNumber rdf:type owl:Class ;
                     rdfs:subClassOf gist:Address ;
                     rdfs:isDefinedBy <https://ontologies.semanticarts.com/o/gistCore> ;
                     skos:definition "A numeric code a telephonic device uses for contacting another telephonic device." ;
                     skos:example "Mobile, fax, or landline phone number." ;
                     skos:prefLabel "Telephone Number" .


###  https://ontologies.semanticarts.com/gist/Temperature
gist:Temperature rdf:type owl:Class ;
                 owl:equivalentClass [ owl:intersectionOf ( gist:Magnitude
                                                            [ rdf:type owl:Restriction ;
                                                              owl:onProperty gist:hasUnitOfMeasure ;
                                                              owl:someValuesFrom gist:TemperatureUnit
                                                            ]
                                                          ) ;
                                       rdf:type owl:Class
                                     ] ;
                 rdfs:isDefinedBy <https://ontologies.semanticarts.com/o/gistCore> ;
                 skos:definition "The degree or intensity of heat present in a substance or object, especially as expressed according to a comparative scale." ;
                 skos:prefLabel "Temperature" .


###  https://ontologies.semanticarts.com/gist/TemperatureUnit
gist:TemperatureUnit rdf:type owl:Class ;
                     owl:equivalentClass [ owl:intersectionOf ( gist:SimpleUnitOfMeasure
                                                                [ rdf:type owl:Restriction ;
                                                                  owl:onProperty gist:hasBaseUnit ;
                                                                  owl:hasValue gist:_kelvin
                                                                ]
                                                                [ rdf:type owl:Restriction ;
                                                                  owl:onProperty gist:conversionOffset ;
                                                                  owl:someValuesFrom xsd:double
                                                                ]
                                                              ) ;
                                           rdf:type owl:Class
                                         ] ;
                     rdfs:isDefinedBy <https://ontologies.semanticarts.com/o/gistCore> ;
                     skos:definition "Unit of measurement for expressing temperature.  Per SI, the base of temperature is in Kelvin, to allow for all units to be expressed relative to a real (in this case absolute) zero." ;
                     skos:prefLabel "Temperature Unit" .


###  https://ontologies.semanticarts.com/gist/Template
gist:Template rdf:type owl:Class ;
              owl:disjointWith gist:UnitOfMeasure ;
              rdfs:isDefinedBy <https://ontologies.semanticarts.com/o/gistCore> ;
              skos:definition "Something used to make objects in its own image." ;
              skos:example "A die in manufacturing that is used to make stamped parts. " ,
                           "A form. A filled-in form has the structure of the form with data entered into some or all of the fields." ,
                           "Cookie cutters are templates for cookies." ;
              skos:prefLabel "Template" ;
              skos:scopeNote "Use gist:isBasedOn to link the object made from the template back to the template." .


###  https://ontologies.semanticarts.com/gist/TemporalRelation
gist:TemporalRelation rdf:type owl:Class ;
                      rdfs:subClassOf [ rdf:type owl:Restriction ;
                                        owl:onProperty gist:hasParticipant ;
                                        owl:minCardinality "2"^^xsd:nonNegativeInteger
                                      ] ,
                                      [ rdf:type owl:Restriction ;
                                        owl:onProperty gist:endDateTime ;
                                        owl:cardinality "1"^^xsd:nonNegativeInteger
                                      ] ,
                                      [ rdf:type owl:Restriction ;
                                        owl:onProperty gist:startDateTime ;
                                        owl:cardinality "1"^^xsd:nonNegativeInteger
                                      ] ;
                      rdfs:isDefinedBy <https://ontologies.semanticarts.com/o/gistCore> ;
                      skos:definition "A relationship existing for a period of time." ;
                      skos:example "employs-Employment, hasStreetAddress-EstablishedLocation. One important context for reifying a property." ;
                      skos:prefLabel "Temporal Relation" ;
                      skos:scopeNote "A temporal relation must have a minimum of two participants. For example, both the employer and the employee are participants in a temporal relation representing a period of employment." ,
                                     "Note that 'participant' does not imply agency; a non-sentient being can be participate in a temporal relation. For example, both a person and a house could be participants in a hypothetical relation 'lives at.'" .


###  https://ontologies.semanticarts.com/gist/Text
gist:Text rdf:type owl:Class ;
          owl:equivalentClass [ owl:intersectionOf ( gist:Content
                                                     [ rdf:type owl:Restriction ;
                                                       owl:onProperty gist:isExpressedIn ;
                                                       owl:someValuesFrom gist:Language
                                                     ]
                                                     [ rdf:type owl:Restriction ;
                                                       owl:onProperty gist:containedText ;
                                                       owl:someValuesFrom xsd:string
                                                     ]
                                                   ) ;
                                rdf:type owl:Class
                              ] ;
          rdfs:isDefinedBy <https://ontologies.semanticarts.com/o/gistCore> ;
          skos:definition "Content expressed as words and numbers (not graphics)." ;
          skos:prefLabel "Text" .


###  https://ontologies.semanticarts.com/gist/TimeZone
gist:TimeZone rdf:type owl:Class ;
              owl:equivalentClass [ owl:intersectionOf ( gist:GeoRegion
                                                         [ rdf:type owl:Restriction ;
                                                           owl:onProperty gist:hasOffsetToUniversal ;
                                                           owl:someValuesFrom gist:Duration
                                                         ]
                                                       ) ;
                                    rdf:type owl:Class
                                  ] ;
              rdfs:isDefinedBy <https://ontologies.semanticarts.com/o/gistCore> ;
              skos:definition "A region that observes a uniform standard time for legal, commercial, and social purposes.  A typical time zone averages 15? of longitude in width and typically observes a clock time one hour earlier than the zone immediately to the east." ;
              skos:prefLabel "Time Zone" .


###  https://ontologies.semanticarts.com/gist/TimeZoneStandard
gist:TimeZoneStandard rdf:type owl:Class ;
                      owl:equivalentClass [ owl:intersectionOf ( gist:Specification
                                                                 [ rdf:type owl:Restriction ;
                                                                   owl:onProperty gist:isBasedOn ;
                                                                   owl:someValuesFrom gist:TimeZone
                                                                 ]
                                                               ) ;
                                            rdf:type owl:Class
                                          ] ;
                      rdfs:isDefinedBy <https://ontologies.semanticarts.com/o/gistCore> ;
                      skos:definition "The algorithm for getting from Greenwich Mean Time to local time, which includes the time zone offset and rules about daylight savings time." ;
                      skos:prefLabel "Time Zone Standard" .


###  https://ontologies.semanticarts.com/gist/Transaction
gist:Transaction rdf:type owl:Class ;
                 rdfs:subClassOf gist:Event ;
                 rdfs:isDefinedBy <https://ontologies.semanticarts.com/o/gistCore> ;
                 skos:definition "An event which has an effect on at least one accumulator." ;
                 skos:prefLabel "Transaction" .


###  https://ontologies.semanticarts.com/gist/TreatyOrganization
gist:TreatyOrganization rdf:type owl:Class ;
                        owl:equivalentClass [ owl:intersectionOf ( gist:IntergovernmentalOrganization
                                                                   [ rdf:type owl:Restriction ;
                                                                     owl:onProperty gist:hasMember ;
                                                                     owl:allValuesFrom gist:CountryGovernment
                                                                   ]
                                                                   [ rdf:type owl:Restriction ;
                                                                     owl:onProperty gist:hasMember ;
                                                                     owl:minCardinality "2"^^xsd:nonNegativeInteger
                                                                   ]
                                                                 ) ;
                                              rdf:type owl:Class
                                            ] ;
                        rdfs:isDefinedBy <https://ontologies.semanticarts.com/o/gistCore> ;
                        skos:definition "An organization whose members are country governments." ;
                        skos:example "NATO, the Louisiana Purchase, the Treaty of Versailles" ;
                        skos:prefLabel "Treaty Organization" .


###  https://ontologies.semanticarts.com/gist/UnitOfMeasure
gist:UnitOfMeasure rdf:type owl:Class ;
                   rdfs:isDefinedBy <https://ontologies.semanticarts.com/o/gistCore> ;
                   skos:definition "Standard unit by which we measure things" ;
                   skos:prefLabel "Unit of Measure" .


###  https://ontologies.semanticarts.com/gist/Volume
gist:Volume rdf:type owl:Class ;
            owl:equivalentClass [ owl:intersectionOf ( gist:Magnitude
                                                       [ rdf:type owl:Restriction ;
                                                         owl:onProperty gist:hasUnitOfMeasure ;
                                                         owl:someValuesFrom gist:VolumeUnit
                                                       ]
                                                     ) ;
                                  rdf:type owl:Class
                                ] ;
            rdfs:isDefinedBy <https://ontologies.semanticarts.com/o/gistCore> ;
            skos:definition "Three-dimensional space, or equivalent fluid measurement." ;
            skos:prefLabel "Volume" .


###  https://ontologies.semanticarts.com/gist/VolumeUnit
gist:VolumeUnit rdf:type owl:Class ;
                owl:equivalentClass [ owl:intersectionOf ( gist:ProductUnit
                                                           [ rdf:type owl:Restriction ;
                                                             owl:onProperty gist:hasMultiplicand ;
                                                             owl:qualifiedCardinality "1"^^xsd:nonNegativeInteger ;
                                                             owl:onClass gist:AreaUnit
                                                           ]
                                                           [ rdf:type owl:Restriction ;
                                                             owl:onProperty gist:hasMultiplier ;
                                                             owl:qualifiedCardinality "1"^^xsd:nonNegativeInteger ;
                                                             owl:onClass gist:DistanceUnit
                                                           ]
                                                         ) ;
                                      rdf:type owl:Class
                                    ] ;
                rdfs:isDefinedBy <https://ontologies.semanticarts.com/o/gistCore> ;
                skos:definition "Units of three-dimensional space, expressed here as an area times a distance." ;
                skos:prefLabel "Volume Unit" .


###  https://ontology.architmitra.org/archimodel/ADElement
<https://ontology.architmitra.org/archimodel/ADElement> rdf:type owl:Class ;
                                                        skos:definition """\"Architecture Description (AD)\" Element
AD Elements are the most primitive constructs of an Architectural Description
An AD Element is any construct in an architecture description
Every Stakeholder, Concern, Architecture Viewpoint, Architecture View, System, Environment and AD is considered an AD Element
AD Elements and their relationships are exposed in Architectural Views in the attempt to address Stakeholder Concerns""" ;
                                                        skos:prefLabel "AD Element" .


###  https://ontology.architmitra.org/archimodel/ActiveStructure
<https://ontology.architmitra.org/archimodel/ActiveStructure> rdf:type owl:Class ;
                                                              owl:equivalentClass [ rdf:type owl:Restriction ;
                                                                                    owl:onProperty <https://ontology.architmitra.org/archimodel/accesses> ;
                                                                                    owl:someValuesFrom <https://ontology.architmitra.org/archimodel/PassiveStructure>
                                                                                  ] ,
                                                                                  [ rdf:type owl:Restriction ;
                                                                                    owl:onProperty <https://ontology.architmitra.org/archimodel/realizes> ;
                                                                                    owl:someValuesFrom <https://ontology.architmitra.org/archimodel/Resource>
                                                                                  ] ;
                                                              rdfs:subClassOf <https://ontology.architmitra.org/archimodel/Structure> ;
                                                              skos:definition "Active structure elements are the subjects that can perform behavior. These can be subdivided into internal active structure elements; i.e., the business actors, application components, nodes, etc., that realize this behavior, and external active structure elements; i.e., the interfaces that expose this behavior to the environment. An interface provides an external view on the service provider and hides its internal structure." ;
                                                              skos:prefLabel "Active Structure" .


###  https://ontology.architmitra.org/archimodel/ApplicationCollaboration
<https://ontology.architmitra.org/archimodel/ApplicationCollaboration> rdf:type owl:Class ;
                                                                       owl:equivalentClass [ rdf:type owl:Restriction ;
                                                                                             owl:onProperty <https://ontology.architmitra.org/archimodel/aggregates> ;
                                                                                             owl:someValuesFrom <https://ontology.architmitra.org/archimodel/ApplicationInternalActiveStructure>
                                                                                           ] ;
                                                                       rdfs:subClassOf <https://ontology.architmitra.org/archimodel/ApplicationInternalActiveStructure> ;
                                                                       skos:definition "An application collaboration represents an aggregate of two or more application internal active structure elements that work together to perform collective application behavior." ;
                                                                       skos:prefLabel "Application Collaboration" .


###  https://ontology.architmitra.org/archimodel/ApplicationComponent
<https://ontology.architmitra.org/archimodel/ApplicationComponent> rdf:type owl:Class ;
                                                                   owl:equivalentClass [ rdf:type owl:Restriction ;
                                                                                         owl:onProperty <https://ontology.architmitra.org/archimodel/realizes> ;
                                                                                         owl:someValuesFrom <https://ontology.architmitra.org/archimodel/ApplicationComponent>
                                                                                       ] ;
                                                                   rdfs:subClassOf <https://ontology.architmitra.org/archimodel/ApplicationInternalActiveStructure> ;
                                                                   skos:definition "An application component represents an encapsulation of application functionality aligned to implementation structure, which is modular and replaceable." ;
                                                                   skos:prefLabel "Application Component" .


###  https://ontology.architmitra.org/archimodel/ApplicationEvent
<https://ontology.architmitra.org/archimodel/ApplicationEvent> rdf:type owl:Class ;
                                                               owl:equivalentClass [ rdf:type owl:Restriction ;
                                                                                     owl:onProperty <https://ontology.architmitra.org/archimodel/accesses> ;
                                                                                     owl:someValuesFrom <https://ontology.architmitra.org/archimodel/DataObject>
                                                                                   ] ,
                                                                                   [ rdf:type owl:Restriction ;
                                                                                     owl:onProperty <https://ontology.architmitra.org/archimodel/realizes> ;
                                                                                     owl:someValuesFrom <https://ontology.architmitra.org/archimodel/BusinessEvent>
                                                                                   ] ,
                                                                                   [ rdf:type owl:Restriction ;
                                                                                     owl:onProperty <https://ontology.architmitra.org/archimodel/triggers> ;
                                                                                     owl:someValuesFrom <https://ontology.architmitra.org/archimodel/ApplicationEvent>
                                                                                   ] ,
                                                                                   [ rdf:type owl:Restriction ;
                                                                                     owl:onProperty <https://ontology.architmitra.org/archimodel/triggers> ;
                                                                                     owl:someValuesFrom <https://ontology.architmitra.org/archimodel/ApplicationInternalBehavior>
                                                                                   ] ,
                                                                                   [ rdf:type owl:Restriction ;
                                                                                     owl:onProperty <https://ontology.architmitra.org/archimodel/triggers> ;
                                                                                     owl:someValuesFrom <https://ontology.architmitra.org/archimodel/ApplicationService>
                                                                                   ] ;
                                                               rdfs:subClassOf <https://ontology.architmitra.org/archimodel/Event> .


###  https://ontology.architmitra.org/archimodel/ApplicationFunction
<https://ontology.architmitra.org/archimodel/ApplicationFunction> rdf:type owl:Class ;
                                                                  rdfs:subClassOf <https://ontology.architmitra.org/archimodel/ApplicationInternalBehavior> .


###  https://ontology.architmitra.org/archimodel/ApplicationInteraction
<https://ontology.architmitra.org/archimodel/ApplicationInteraction> rdf:type owl:Class ;
                                                                     rdfs:subClassOf <https://ontology.architmitra.org/archimodel/ApplicationInternalBehavior> .


###  https://ontology.architmitra.org/archimodel/ApplicationInterface
<https://ontology.architmitra.org/archimodel/ApplicationInterface> rdf:type owl:Class ;
                                                                   owl:equivalentClass [ rdf:type owl:Restriction ;
                                                                                         owl:onProperty <https://ontology.architmitra.org/archimodel/serves> ;
                                                                                         owl:someValuesFrom <https://ontology.architmitra.org/archimodel/ApplicationInternalActiveStructure>
                                                                                       ] ,
                                                                                       [ rdf:type owl:Restriction ;
                                                                                         owl:onProperty <https://ontology.architmitra.org/archimodel/serves> ;
                                                                                         owl:someValuesFrom <https://ontology.architmitra.org/archimodel/BusinessInternalActivStructure>
                                                                                       ] ,
                                                                                       [ rdf:type owl:Restriction ;
                                                                                         owl:onProperty <https://ontology.architmitra.org/archimodel/serves> ;
                                                                                         owl:someValuesFrom <https://ontology.architmitra.org/archimodel/TechnologyInternalActiveStructure>
                                                                                       ] ;
                                                                   rdfs:subClassOf <https://ontology.architmitra.org/archimodel/ExternalActiveStructure> ;
                                                                   skos:prefLabel "Application Interface" .


###  https://ontology.architmitra.org/archimodel/ApplicationInternalActiveStructure
<https://ontology.architmitra.org/archimodel/ApplicationInternalActiveStructure> rdf:type owl:Class ;
                                                                                 owl:equivalentClass [ rdf:type owl:Restriction ;
                                                                                                       owl:onProperty <https://ontology.architmitra.org/archimodel/assignedTo> ;
                                                                                                       owl:someValuesFrom <https://ontology.architmitra.org/archimodel/ApplicationEvent>
                                                                                                     ] ,
                                                                                                     [ rdf:type owl:Restriction ;
                                                                                                       owl:onProperty <https://ontology.architmitra.org/archimodel/assignedTo> ;
                                                                                                       owl:someValuesFrom <https://ontology.architmitra.org/archimodel/ApplicationInternalBehavior>
                                                                                                     ] ,
                                                                                                     [ rdf:type owl:Restriction ;
                                                                                                       owl:onProperty <https://ontology.architmitra.org/archimodel/composedOf> ;
                                                                                                       owl:someValuesFrom <https://ontology.architmitra.org/archimodel/ApplicationInterface>
                                                                                                     ] ;
                                                                                 rdfs:subClassOf <https://ontology.architmitra.org/archimodel/InternalActiveStructure> ;
                                                                                 skos:prefLabel "Application Internal Active Structure" .


###  https://ontology.architmitra.org/archimodel/ApplicationInternalBehavior
<https://ontology.architmitra.org/archimodel/ApplicationInternalBehavior> rdf:type owl:Class ;
                                                                          owl:equivalentClass [ rdf:type owl:Restriction ;
                                                                                                owl:onProperty <https://ontology.architmitra.org/archimodel/accesses> ;
                                                                                                owl:someValuesFrom <https://ontology.architmitra.org/archimodel/DataObject>
                                                                                              ] ,
                                                                                              [ rdf:type owl:Restriction ;
                                                                                                owl:onProperty <https://ontology.architmitra.org/archimodel/aggregates> ;
                                                                                                owl:someValuesFrom <https://ontology.architmitra.org/archimodel/ApplicationInternalBehavior>
                                                                                              ] ,
                                                                                              [ rdf:type owl:Restriction ;
                                                                                                owl:onProperty <https://ontology.architmitra.org/archimodel/composedOf> ;
                                                                                                owl:someValuesFrom <https://ontology.architmitra.org/archimodel/ApplicationInternalBehavior>
                                                                                              ] ,
                                                                                              [ rdf:type owl:Restriction ;
                                                                                                owl:onProperty <https://ontology.architmitra.org/archimodel/realizes> ;
                                                                                                owl:someValuesFrom <https://ontology.architmitra.org/archimodel/ApplicationService>
                                                                                              ] ,
                                                                                              [ rdf:type owl:Restriction ;
                                                                                                owl:onProperty <https://ontology.architmitra.org/archimodel/realizes> ;
                                                                                                owl:someValuesFrom <https://ontology.architmitra.org/archimodel/BusinessinternalBehavior>
                                                                                              ] ,
                                                                                              [ rdf:type owl:Restriction ;
                                                                                                owl:onProperty <https://ontology.architmitra.org/archimodel/triggers> ;
                                                                                                owl:someValuesFrom <https://ontology.architmitra.org/archimodel/ApplicationEvent>
                                                                                              ] ,
                                                                                              [ rdf:type owl:Restriction ;
                                                                                                owl:onProperty <https://ontology.architmitra.org/archimodel/triggers> ;
                                                                                                owl:someValuesFrom <https://ontology.architmitra.org/archimodel/ApplicationInternalBehavior>
                                                                                              ] ;
                                                                          rdfs:subClassOf <https://ontology.architmitra.org/archimodel/InternalBehavior> ;
                                                                          skos:prefLabel "Application Internal Behavior" .


###  https://ontology.architmitra.org/archimodel/ApplicationProcess
<https://ontology.architmitra.org/archimodel/ApplicationProcess> rdf:type owl:Class ;
                                                                 rdfs:subClassOf <https://ontology.architmitra.org/archimodel/ApplicationInternalBehavior> .


###  https://ontology.architmitra.org/archimodel/ApplicationService
<https://ontology.architmitra.org/archimodel/ApplicationService> rdf:type owl:Class ;
                                                                 owl:equivalentClass [ rdf:type owl:Restriction ;
                                                                                       owl:onProperty <https://ontology.architmitra.org/archimodel/accesses> ;
                                                                                       owl:someValuesFrom <https://ontology.architmitra.org/archimodel/DataObject>
                                                                                     ] ,
                                                                                     [ rdf:type owl:Restriction ;
                                                                                       owl:onProperty <https://ontology.architmitra.org/archimodel/assignedTo> ;
                                                                                       owl:someValuesFrom <https://ontology.architmitra.org/archimodel/ApplicationInternalActiveStructure>
                                                                                     ] ,
                                                                                     [ rdf:type owl:Restriction ;
                                                                                       owl:onProperty <https://ontology.architmitra.org/archimodel/realizes> ;
                                                                                       owl:someValuesFrom <https://ontology.architmitra.org/archimodel/BusinessService>
                                                                                     ] ,
                                                                                     [ rdf:type owl:Restriction ;
                                                                                       owl:onProperty <https://ontology.architmitra.org/archimodel/serves> ;
                                                                                       owl:someValuesFrom <https://ontology.architmitra.org/archimodel/ApplicationInternalActiveStructure>
                                                                                     ] ,
                                                                                     [ rdf:type owl:Restriction ;
                                                                                       owl:onProperty <https://ontology.architmitra.org/archimodel/serves> ;
                                                                                       owl:someValuesFrom <https://ontology.architmitra.org/archimodel/ApplicationInternalBehavior>
                                                                                     ] ,
                                                                                     [ rdf:type owl:Restriction ;
                                                                                       owl:onProperty <https://ontology.architmitra.org/archimodel/serves> ;
                                                                                       owl:someValuesFrom <https://ontology.architmitra.org/archimodel/BusinessInternalActivStructure>
                                                                                     ] ,
                                                                                     [ rdf:type owl:Restriction ;
                                                                                       owl:onProperty <https://ontology.architmitra.org/archimodel/serves> ;
                                                                                       owl:someValuesFrom <https://ontology.architmitra.org/archimodel/BusinessinternalBehavior>
                                                                                     ] ,
                                                                                     [ rdf:type owl:Restriction ;
                                                                                       owl:onProperty <https://ontology.architmitra.org/archimodel/serves> ;
                                                                                       owl:someValuesFrom <https://ontology.architmitra.org/archimodel/TechnologyInternalActiveStructure>
                                                                                     ] ,
                                                                                     [ rdf:type owl:Restriction ;
                                                                                       owl:onProperty <https://ontology.architmitra.org/archimodel/serves> ;
                                                                                       owl:someValuesFrom <https://ontology.architmitra.org/archimodel/TechnologyInternalBehavior>
                                                                                     ] ,
                                                                                     [ rdf:type owl:Restriction ;
                                                                                       owl:onProperty <https://ontology.architmitra.org/archimodel/triggers> ;
                                                                                       owl:someValuesFrom <https://ontology.architmitra.org/archimodel/ApplicationService>
                                                                                     ] ;
                                                                 rdfs:subClassOf <https://ontology.architmitra.org/archimodel/ExternalBehavior> .


###  https://ontology.architmitra.org/archimodel/ArchitecturalStyle
<https://ontology.architmitra.org/archimodel/ArchitecturalStyle> rdf:type owl:Class ;
                                                                 rdfs:subClassOf <https://ontology.architmitra.org/archimodel/ADElement> ;
                                                                 skos:prefLabel "Architectural Style" .


###  https://ontology.architmitra.org/archimodel/Architecture
<https://ontology.architmitra.org/archimodel/Architecture> rdf:type owl:Class ;
                                                           skos:definition """An Architecture is an abstraction of a System of Interest. An Architecture represents the fundamental concepts or properties of a System in its Envronment, embodied in its elements, relationships, and in the principles of its design and evolution.
A System has an Architecture even if that Architecture is not written down""" .


###  https://ontology.architmitra.org/archimodel/ArchitectureDecision
<https://ontology.architmitra.org/archimodel/ArchitectureDecision> rdf:type owl:Class ;
                                                                   owl:equivalentClass [ rdf:type owl:Restriction ;
                                                                                         owl:onProperty gist:affects ;
                                                                                         owl:someValuesFrom <https://ontology.architmitra.org/archimodel/ADElement>
                                                                                       ] ,
                                                                                       [ rdf:type owl:Restriction ;
                                                                                         owl:onProperty <https://ontology.architmitra.org/archimodel/dependsOn> ;
                                                                                         owl:someValuesFrom <https://ontology.architmitra.org/archimodel/ArchitectureDecision>
                                                                                       ] ,
                                                                                       [ rdf:type owl:Restriction ;
                                                                                         owl:onProperty <https://ontology.architmitra.org/archimodel/pertainsTo> ;
                                                                                         owl:someValuesFrom <https://ontology.architmitra.org/archimodel/Concern>
                                                                                       ] ,
                                                                                       [ rdf:type owl:Restriction ;
                                                                                         owl:onProperty <https://ontology.architmitra.org/archimodel/raises> ;
                                                                                         owl:someValuesFrom <https://ontology.architmitra.org/archimodel/Concern>
                                                                                       ] ;
                                                                   rdfs:subClassOf <https://ontology.architmitra.org/archimodel/ADElement> ;
                                                                   skos:definition """Architecture Decisions pertain to Stakeholder Concerns
Useful to record relationship dependencies between architecture decisions:
- constrains, influences, enables, triggers, forces, subsumes, refines, conflicts-with, is-compatible-with""" ;
                                                                   skos:prefLabel "Architecture Decision" .


###  https://ontology.architmitra.org/archimodel/ArchitectureDescription
<https://ontology.architmitra.org/archimodel/ArchitectureDescription> rdf:type owl:Class ;
                                                                      owl:equivalentClass [ rdf:type owl:Restriction ;
                                                                                            owl:onProperty gist:identifies ;
                                                                                            owl:someValuesFrom <https://ontology.architmitra.org/archimodel/Concern>
                                                                                          ] ,
                                                                                          [ rdf:type owl:Restriction ;
                                                                                            owl:onProperty gist:identifies ;
                                                                                            owl:someValuesFrom <https://ontology.architmitra.org/archimodel/Stakeholder>
                                                                                          ] ,
                                                                                          [ rdf:type owl:Restriction ;
                                                                                            owl:onProperty gist:identifies ;
                                                                                            owl:someValuesFrom <https://ontology.architmitra.org/archimodel/SystemOfInterest>
                                                                                          ] ,
                                                                                          [ rdf:type owl:Restriction ;
                                                                                            owl:onProperty <https://ontology.architmitra.org/archimodel/aggregates> ;
                                                                                            owl:someValuesFrom <https://ontology.architmitra.org/archimodel/ADElement>
                                                                                          ] ,
                                                                                          [ rdf:type owl:Restriction ;
                                                                                            owl:onProperty <https://ontology.architmitra.org/archimodel/composedOf> ;
                                                                                            owl:someValuesFrom <https://ontology.architmitra.org/archimodel/ArchitectureDecision>
                                                                                          ] ,
                                                                                          [ rdf:type owl:Restriction ;
                                                                                            owl:onProperty <https://ontology.architmitra.org/archimodel/composedOf> ;
                                                                                            owl:someValuesFrom <https://ontology.architmitra.org/archimodel/ArchitectureRationale>
                                                                                          ] ,
                                                                                          [ rdf:type owl:Restriction ;
                                                                                            owl:onProperty <https://ontology.architmitra.org/archimodel/composedOf> ;
                                                                                            owl:someValuesFrom <https://ontology.architmitra.org/archimodel/ArchitectureView>
                                                                                          ] ,
                                                                                          [ rdf:type owl:Restriction ;
                                                                                            owl:onProperty <https://ontology.architmitra.org/archimodel/composedOf> ;
                                                                                            owl:someValuesFrom <https://ontology.architmitra.org/archimodel/ArchitectureViewpoint>
                                                                                          ] ,
                                                                                          [ rdf:type owl:Restriction ;
                                                                                            owl:onProperty <https://ontology.architmitra.org/archimodel/expresses> ;
                                                                                            owl:someValuesFrom <https://ontology.architmitra.org/archimodel/Architecture>
                                                                                          ] ;
                                                                      rdfs:subClassOf <https://ontology.architmitra.org/archimodel/ADElement> ,
                                                                                      <https://ontology.architmitra.org/archimodel/ArchitectureModel> ;
                                                                      skos:definition """Architectural Descriptions should address the relevant Stakeholder Concerns of the System of Interest.
Stakeholders use Architecture Descriptions to understand, analyze, and compare System Architectures.
An AD may take the form of documents, models, simulations or other forms.
An Architecture Description results from the execution of architecting activities within the lifecycle of the System of Interest.
An AD can document the essential aspects of a System:
- intended use and environment
- principles, assumptions and constraints on structure and behavior
- points of flexibility or limitations of the system
- architecture decisions, their rationale and impacts
Possible uses of AD:
- analyze and evaluate existing system performance
- review, analysis and evaluation of the system across its lifecycle
Architecture Descriptions are comprised of Architecture Views of AD Elements
Stakeholder concerns are addressed when an Architecture Description exposes AD Elements in Architecture Views that satisfies the conventions established by an Arcitecture Viewpoint
An Architecture Description is itself an Architecture Model. It contains AD Elements necessary for addressing System Stakeholder Concerns""" ;
                                                                      skos:prefLabel "Architecture Description" .


###  https://ontology.architmitra.org/archimodel/ArchitectureModel
<https://ontology.architmitra.org/archimodel/ArchitectureModel> rdf:type owl:Class ;
                                                                owl:equivalentClass [ rdf:type owl:Restriction ;
                                                                                      owl:onProperty gist:governs ;
                                                                                      owl:someValuesFrom <https://ontology.architmitra.org/archimodel/ArchitectureModel>
                                                                                    ] ,
                                                                                    [ rdf:type owl:Restriction ;
                                                                                      owl:onProperty <https://ontology.architmitra.org/archimodel/composedOf> ;
                                                                                      owl:someValuesFrom <https://ontology.architmitra.org/archimodel/ADElement>
                                                                                    ] ;
                                                                rdfs:subClassOf <https://ontology.architmitra.org/archimodel/ADElement> ;
                                                                skos:definition """An Architecture Model uses modeling conventions appropriate to the concerns to be addressed. These conventions are specified by the Model Kind governing that model
Architecture Models and architecting are specialized forms of models and modeling""" ;
                                                                skos:prefLabel "Architecture Model" .


###  https://ontology.architmitra.org/archimodel/ArchitectureRationale
<https://ontology.architmitra.org/archimodel/ArchitectureRationale> rdf:type owl:Class ;
                                                                    owl:equivalentClass [ rdf:type owl:Restriction ;
                                                                                          owl:onProperty <https://ontology.architmitra.org/archimodel/justifies> ;
                                                                                          owl:someValuesFrom <https://ontology.architmitra.org/archimodel/ArchitectureDecision>
                                                                                        ] ;
                                                                    rdfs:subClassOf <https://ontology.architmitra.org/archimodel/ADElement> ;
                                                                    skos:definition """Architecture Rationale records explanation, justification or reasoning about Architecture Decisions that have been made
The Architecture Rationale for an Architecture Decision can include:
- the basis for a Decision
- alternatives and trade-offs considered
- potential consequences of the decision
- citations to sources of additional information""" ;
                                                                    skos:prefLabel "Architecture Rationale" .


###  https://ontology.architmitra.org/archimodel/ArchitectureView
<https://ontology.architmitra.org/archimodel/ArchitectureView> rdf:type owl:Class ;
                                                               owl:equivalentClass [ rdf:type owl:Restriction ;
                                                                                     owl:onProperty <https://ontology.architmitra.org/archimodel/addresses> ;
                                                                                     owl:someValuesFrom <https://ontology.architmitra.org/archimodel/Concern>
                                                                                   ] ,
                                                                                   [ rdf:type owl:Restriction ;
                                                                                     owl:onProperty <https://ontology.architmitra.org/archimodel/aggregates> ;
                                                                                     owl:someValuesFrom <https://ontology.architmitra.org/archimodel/ArchitectureModel>
                                                                                   ] ,
                                                                                   [ rdf:type owl:Restriction ;
                                                                                     owl:onProperty <https://ontology.architmitra.org/archimodel/exposes> ;
                                                                                     owl:someValuesFrom <https://ontology.architmitra.org/archimodel/ADElement>
                                                                                   ] ;
                                                               rdfs:subClassOf <https://ontology.architmitra.org/archimodel/ADElement> ;
                                                               skos:definition """An Architecture View exposes a limited set of AD elements and relationships
An Architecture View addresses one or more of the Concerns held by the System of Interest's Stakeholders - when it confirms to an Architectural Viewpoint
An Architecture Description includes one or more Architecture Views
Separating Concerns addressed by Architecture Views offers a means to manage complexity
An Architecture View is created through the aggregation of one or more Architecture Models""" ;
                                                               skos:prefLabel "Architecture View" .


###  https://ontology.architmitra.org/archimodel/ArchitectureViewpoint
<https://ontology.architmitra.org/archimodel/ArchitectureViewpoint> rdf:type owl:Class ;
                                                                    owl:equivalentClass [ rdf:type owl:Restriction ;
                                                                                          owl:onProperty gist:governs ;
                                                                                          owl:someValuesFrom <https://ontology.architmitra.org/archimodel/ArchitectureView>
                                                                                        ] ,
                                                                                        [ rdf:type owl:Restriction ;
                                                                                          owl:onProperty <https://ontology.architmitra.org/archimodel/aggregates> ;
                                                                                          owl:someValuesFrom <https://ontology.architmitra.org/archimodel/ModelKind>
                                                                                        ] ,
                                                                                        [ rdf:type owl:Restriction ;
                                                                                          owl:onProperty <https://ontology.architmitra.org/archimodel/frames> ;
                                                                                          owl:someValuesFrom <https://ontology.architmitra.org/archimodel/Concern>
                                                                                        ] ;
                                                                    rdfs:subClassOf <https://ontology.architmitra.org/archimodel/ADElement> ;
                                                                    skos:definition """An Architecture Viewpoint frames a specific set of Concerns
An Architecture View is governed by its Viewpoint
An Archiecture Viewpoint is a way of looking at a System of Interest'
An Architecture Viewpoint is a set of conventions for constructing, interpreting, using and analyzing Architecture Views
An Architecture Viewpoint scopes these conventions to frame a specific set of Concerns
Viewpoints codify application-specific, method-specific or organization-specific approaches to capture, organize and share system of interest knowledge
Requirement: Each Concern identified shall be framed by at least one viewpoint
An AD shall include exactly one Architecture View for each Architecture Viewpoint used""" ;
                                                                    skos:prefLabel "Architecture Viewpoint" .


###  https://ontology.architmitra.org/archimodel/Artifact
<https://ontology.architmitra.org/archimodel/Artifact> rdf:type owl:Class ;
                                                       owl:equivalentClass [ rdf:type owl:Restriction ;
                                                                             owl:onProperty <https://ontology.architmitra.org/archimodel/realizes> ;
                                                                             owl:someValuesFrom <https://ontology.architmitra.org/archimodel/ApplicationInternalActiveStructure>
                                                                           ] ,
                                                                           [ rdf:type owl:Restriction ;
                                                                             owl:onProperty <https://ontology.architmitra.org/archimodel/realizes> ;
                                                                             owl:someValuesFrom <https://ontology.architmitra.org/archimodel/DataObject>
                                                                           ] ,
                                                                           [ rdf:type owl:Restriction ;
                                                                             owl:onProperty <https://ontology.architmitra.org/archimodel/realizes> ;
                                                                             owl:someValuesFrom <https://ontology.architmitra.org/archimodel/SystemSoftware>
                                                                           ] ;
                                                       rdfs:subClassOf <https://ontology.architmitra.org/archimodel/TechnologyObject> ;
                                                       skos:definition "An artifact represents a piece of data that is used or produced in a software development process, or by deployment and operation of an IT system." .


###  https://ontology.architmitra.org/archimodel/Assessment
<https://ontology.architmitra.org/archimodel/Assessment> rdf:type owl:Class ;
                                                         rdfs:subClassOf <https://ontology.architmitra.org/archimodel/Motivation> ;
                                                         skos:definition "An assessment represents the result of an analysis of the state of affairs of the enterprise with respect to some driver." .


###  https://ontology.architmitra.org/archimodel/Behavior
<https://ontology.architmitra.org/archimodel/Behavior> rdf:type owl:Class ;
                                                       owl:equivalentClass [ rdf:type owl:Restriction ;
                                                                             owl:onProperty <https://ontology.architmitra.org/archimodel/accesses> ;
                                                                             owl:someValuesFrom <https://ontology.architmitra.org/archimodel/PassiveStructure>
                                                                           ] ,
                                                                           [ rdf:type owl:Restriction ;
                                                                             owl:onProperty <https://ontology.architmitra.org/archimodel/influences> ;
                                                                             owl:someValuesFrom <https://ontology.architmitra.org/archimodel/Requirement>
                                                                           ] ,
                                                                           [ rdf:type owl:Restriction ;
                                                                             owl:onProperty <https://ontology.architmitra.org/archimodel/realizes> ;
                                                                             owl:someValuesFrom <https://ontology.architmitra.org/archimodel/Requirement>
                                                                           ] ;
                                                       rdfs:subClassOf <https://ontology.architmitra.org/archimodel/Element> ;
                                                       skos:definition "Behavior elements represent the dynamic aspects of the enterprise. Similar to active structure elements, behavior elements can be subdivided into internal behavior elements and external behavior elements; i.e., the services that are exposed to the environment." ;
                                                       skos:prefLabel "Behavior" .


###  https://ontology.architmitra.org/archimodel/BusinessActor
<https://ontology.architmitra.org/archimodel/BusinessActor> rdf:type owl:Class ;
                                                            owl:equivalentClass [ rdf:type owl:Restriction ;
                                                                                  owl:onProperty <https://ontology.architmitra.org/archimodel/assignedTo> ;
                                                                                  owl:someValuesFrom <https://ontology.architmitra.org/archimodel/BusinessRole>
                                                                                ] ;
                                                            rdfs:subClassOf <https://ontology.architmitra.org/archimodel/BusinessInternalActivStructure> ;
                                                            skos:definition "A business actor represents a business entity that is capable of performing behavior." ;
                                                            skos:prefLabel "Business Actor" .


###  https://ontology.architmitra.org/archimodel/BusinessCollaboration
<https://ontology.architmitra.org/archimodel/BusinessCollaboration> rdf:type owl:Class ;
                                                                    owl:equivalentClass [ rdf:type owl:Restriction ;
                                                                                          owl:onProperty <https://ontology.architmitra.org/archimodel/aggregates> ;
                                                                                          owl:someValuesFrom <https://ontology.architmitra.org/archimodel/BusinessInternalActivStructure>
                                                                                        ] ;
                                                                    rdfs:subClassOf <https://ontology.architmitra.org/archimodel/BusinessInternalActivStructure> ;
                                                                    skos:definition "A business collaboration represents an aggregate of two or more business internal active structure elements that work together to perform collective behavior." ;
                                                                    skos:prefLabel "Business Collaboration" .


###  https://ontology.architmitra.org/archimodel/BusinessEvent
<https://ontology.architmitra.org/archimodel/BusinessEvent> rdf:type owl:Class ;
                                                            owl:equivalentClass [ rdf:type owl:Restriction ;
                                                                                  owl:onProperty <https://ontology.architmitra.org/archimodel/accesses> ;
                                                                                  owl:someValuesFrom <https://ontology.architmitra.org/archimodel/BusinessPassiveStructure>
                                                                                ] ,
                                                                                [ rdf:type owl:Restriction ;
                                                                                  owl:onProperty <https://ontology.architmitra.org/archimodel/triggers> ;
                                                                                  owl:someValuesFrom <https://ontology.architmitra.org/archimodel/BusinessEvent>
                                                                                ] ,
                                                                                [ rdf:type owl:Restriction ;
                                                                                  owl:onProperty <https://ontology.architmitra.org/archimodel/triggers> ;
                                                                                  owl:someValuesFrom <https://ontology.architmitra.org/archimodel/BusinessService>
                                                                                ] ,
                                                                                [ rdf:type owl:Restriction ;
                                                                                  owl:onProperty <https://ontology.architmitra.org/archimodel/triggers> ;
                                                                                  owl:someValuesFrom <https://ontology.architmitra.org/archimodel/BusinessinternalBehavior>
                                                                                ] ;
                                                            rdfs:subClassOf <https://ontology.architmitra.org/archimodel/Event> ;
                                                            skos:definition "A business event represents an organizational state change." ;
                                                            skos:prefLabel "Business Event" .


###  https://ontology.architmitra.org/archimodel/BusinessFunction
<https://ontology.architmitra.org/archimodel/BusinessFunction> rdf:type owl:Class ;
                                                               rdfs:subClassOf <https://ontology.architmitra.org/archimodel/BusinessinternalBehavior> ;
                                                               skos:definition "A business function represents a collection of business behavior based on a chosen set of criteria (typically required business resources and/or competencies), closely aligned to an organization, but not necessarily explicitly governed by the organization." ;
                                                               skos:prefLabel "Business Function" .


###  https://ontology.architmitra.org/archimodel/BusinessInteraction
<https://ontology.architmitra.org/archimodel/BusinessInteraction> rdf:type owl:Class ;
                                                                  rdfs:subClassOf <https://ontology.architmitra.org/archimodel/BusinessinternalBehavior> ;
                                                                  skos:definition "A business interaction represents a unit of collective business behavior performed by (a collaboration of) two or more business actors, business roles, or business collaborations." ;
                                                                  skos:prefLabel "Business Interaction" .


###  https://ontology.architmitra.org/archimodel/BusinessInterface
<https://ontology.architmitra.org/archimodel/BusinessInterface> rdf:type owl:Class ;
                                                                owl:equivalentClass [ rdf:type owl:Restriction ;
                                                                                      owl:onProperty <https://ontology.architmitra.org/archimodel/assignedTo> ;
                                                                                      owl:someValuesFrom <https://ontology.architmitra.org/archimodel/BusinessService>
                                                                                    ] ,
                                                                                    [ rdf:type owl:Restriction ;
                                                                                      owl:onProperty <https://ontology.architmitra.org/archimodel/serves> ;
                                                                                      owl:someValuesFrom <https://ontology.architmitra.org/archimodel/ApplicationInternalActiveStructure>
                                                                                    ] ,
                                                                                    [ rdf:type owl:Restriction ;
                                                                                      owl:onProperty <https://ontology.architmitra.org/archimodel/serves> ;
                                                                                      owl:someValuesFrom <https://ontology.architmitra.org/archimodel/TechnologyInternalActiveStructure>
                                                                                    ] ;
                                                                rdfs:subClassOf <https://ontology.architmitra.org/archimodel/ExternalActiveStructure> ;
                                                                skos:definition "A business interface represents a point of access where a business service is made available to the environment." ;
                                                                skos:prefLabel "Business Interface" .


###  https://ontology.architmitra.org/archimodel/BusinessInternalActivStructure
<https://ontology.architmitra.org/archimodel/BusinessInternalActivStructure> rdf:type owl:Class ;
                                                                             owl:equivalentClass [ rdf:type owl:Restriction ;
                                                                                                   owl:onProperty <https://ontology.architmitra.org/archimodel/assignedTo> ;
                                                                                                   owl:someValuesFrom <https://ontology.architmitra.org/archimodel/BusinessEvent>
                                                                                                 ] ,
                                                                                                 [ rdf:type owl:Restriction ;
                                                                                                   owl:onProperty <https://ontology.architmitra.org/archimodel/assignedTo> ;
                                                                                                   owl:someValuesFrom <https://ontology.architmitra.org/archimodel/BusinessinternalBehavior>
                                                                                                 ] ,
                                                                                                 [ rdf:type owl:Restriction ;
                                                                                                   owl:onProperty <https://ontology.architmitra.org/archimodel/assignedTo> ;
                                                                                                   owl:someValuesFrom <https://ontology.architmitra.org/archimodel/ImplementationEvent>
                                                                                                 ] ,
                                                                                                 [ rdf:type owl:Restriction ;
                                                                                                   owl:onProperty <https://ontology.architmitra.org/archimodel/assignedTo> ;
                                                                                                   owl:someValuesFrom <https://ontology.architmitra.org/archimodel/WorkPackage>
                                                                                                 ] ,
                                                                                                 [ rdf:type owl:Restriction ;
                                                                                                   owl:onProperty <https://ontology.architmitra.org/archimodel/composedOf> ;
                                                                                                   owl:someValuesFrom <https://ontology.architmitra.org/archimodel/BusinessInterface>
                                                                                                 ] ;
                                                                             rdfs:subClassOf <https://ontology.architmitra.org/archimodel/InternalActiveStructure> ;
                                                                             skos:definition "The active structure aspect of the Business Layer refers to the static structure of an organization, in terms of the entities that make up the organization and their relationships. The active entities are the subjects (e.g., business actors or business roles) that perform behavior such as business processes or functions (capabilities). Business actors may be individual persons (e.g., customers or employees), but also groups of people (organization units) and resources that have a permanent (or at least long-term) status within the organizations. Typical examples of the latter are a department and a business unit." ;
                                                                             skos:prefLabel "Business Internal Active Structure" .


###  https://ontology.architmitra.org/archimodel/BusinessObject
<https://ontology.architmitra.org/archimodel/BusinessObject> rdf:type owl:Class ;
                                                             rdfs:subClassOf <https://ontology.architmitra.org/archimodel/BusinessPassiveStructure> ;
                                                             skos:definition "A business object represents a concept used within a particular business domain." ;
                                                             skos:prefLabel "Business Object" .


###  https://ontology.architmitra.org/archimodel/BusinessPassiveStructure
<https://ontology.architmitra.org/archimodel/BusinessPassiveStructure> rdf:type owl:Class ;
                                                                       rdfs:subClassOf <https://ontology.architmitra.org/archimodel/PassiveStructure> ;
                                                                       skos:prefLabel "Business Passive Structure" .


###  https://ontology.architmitra.org/archimodel/BusinessProcess
<https://ontology.architmitra.org/archimodel/BusinessProcess> rdf:type owl:Class ;
                                                              rdfs:subClassOf <https://ontology.architmitra.org/archimodel/BusinessinternalBehavior> ;
                                                              skos:definition "A business process represents a sequence of business behaviors that achieves a specific result such as a defined set of products or business services." ;
                                                              skos:prefLabel "Business Process" .


###  https://ontology.architmitra.org/archimodel/BusinessRole
<https://ontology.architmitra.org/archimodel/BusinessRole> rdf:type owl:Class ;
                                                           rdfs:subClassOf <https://ontology.architmitra.org/archimodel/BusinessInternalActivStructure> ;
                                                           skos:definition "A business role represents the responsibility for performing specific behavior, to which an actor can be assigned, or the part an actor plays in a particular action or event." ;
                                                           skos:prefLabel "Business Role" .


###  https://ontology.architmitra.org/archimodel/BusinessService
<https://ontology.architmitra.org/archimodel/BusinessService> rdf:type owl:Class ;
                                                              owl:equivalentClass [ rdf:type owl:Restriction ;
                                                                                    owl:onProperty <https://ontology.architmitra.org/archimodel/accesses> ;
                                                                                    owl:someValuesFrom <https://ontology.architmitra.org/archimodel/BusinessPassiveStructure>
                                                                                  ] ,
                                                                                  [ rdf:type owl:Restriction ;
                                                                                    owl:onProperty <https://ontology.architmitra.org/archimodel/serves> ;
                                                                                    owl:someValuesFrom <https://ontology.architmitra.org/archimodel/ApplicationInternalActiveStructure>
                                                                                  ] ,
                                                                                  [ rdf:type owl:Restriction ;
                                                                                    owl:onProperty <https://ontology.architmitra.org/archimodel/serves> ;
                                                                                    owl:someValuesFrom <https://ontology.architmitra.org/archimodel/ApplicationInternalBehavior>
                                                                                  ] ,
                                                                                  [ rdf:type owl:Restriction ;
                                                                                    owl:onProperty <https://ontology.architmitra.org/archimodel/serves> ;
                                                                                    owl:someValuesFrom <https://ontology.architmitra.org/archimodel/BusinessInternalActivStructure>
                                                                                  ] ,
                                                                                  [ rdf:type owl:Restriction ;
                                                                                    owl:onProperty <https://ontology.architmitra.org/archimodel/serves> ;
                                                                                    owl:someValuesFrom <https://ontology.architmitra.org/archimodel/BusinessinternalBehavior>
                                                                                  ] ,
                                                                                  [ rdf:type owl:Restriction ;
                                                                                    owl:onProperty <https://ontology.architmitra.org/archimodel/serves> ;
                                                                                    owl:someValuesFrom <https://ontology.architmitra.org/archimodel/TechnologyInternalActiveStructure>
                                                                                  ] ,
                                                                                  [ rdf:type owl:Restriction ;
                                                                                    owl:onProperty <https://ontology.architmitra.org/archimodel/serves> ;
                                                                                    owl:someValuesFrom <https://ontology.architmitra.org/archimodel/TechnologyInternalBehavior>
                                                                                  ] ,
                                                                                  [ rdf:type owl:Restriction ;
                                                                                    owl:onProperty <https://ontology.architmitra.org/archimodel/triggers> ;
                                                                                    owl:someValuesFrom <https://ontology.architmitra.org/archimodel/BusinessEvent>
                                                                                  ] ,
                                                                                  [ rdf:type owl:Restriction ;
                                                                                    owl:onProperty <https://ontology.architmitra.org/archimodel/triggers> ;
                                                                                    owl:someValuesFrom <https://ontology.architmitra.org/archimodel/BusinessService>
                                                                                  ] ;
                                                              rdfs:subClassOf <https://ontology.architmitra.org/archimodel/ExternalBehavior> ;
                                                              skos:definition "A business service represents explicitly defined behavior that a business role, business actor, or business collaboration exposes to its environment." ;
                                                              skos:prefLabel "Business Service" .


###  https://ontology.architmitra.org/archimodel/BusinessinternalBehavior
<https://ontology.architmitra.org/archimodel/BusinessinternalBehavior> rdf:type owl:Class ;
                                                                       owl:equivalentClass [ rdf:type owl:Restriction ;
                                                                                             owl:onProperty <https://ontology.architmitra.org/archimodel/accesses> ;
                                                                                             owl:someValuesFrom <https://ontology.architmitra.org/archimodel/BusinessPassiveStructure>
                                                                                           ] ,
                                                                                           [ rdf:type owl:Restriction ;
                                                                                             owl:onProperty <https://ontology.architmitra.org/archimodel/triggers> ;
                                                                                             owl:someValuesFrom <https://ontology.architmitra.org/archimodel/BusinessEvent>
                                                                                           ] ,
                                                                                           [ rdf:type owl:Restriction ;
                                                                                             owl:onProperty <https://ontology.architmitra.org/archimodel/triggers> ;
                                                                                             owl:someValuesFrom <https://ontology.architmitra.org/archimodel/BusinessinternalBehavior>
                                                                                           ] ;
                                                                       rdfs:subClassOf <https://ontology.architmitra.org/archimodel/InternalBehavior> ;
                                                                       skos:prefLabel "Business Internal Behavior" .


###  https://ontology.architmitra.org/archimodel/Capability
<https://ontology.architmitra.org/archimodel/Capability> rdf:type owl:Class ;
                                                         rdfs:subClassOf <https://ontology.architmitra.org/archimodel/Strategy> ;
                                                         skos:definition "A capability represents an ability that an active structure element, such as an organization, person, or system, possesses." .


###  https://ontology.architmitra.org/archimodel/Collaboration
<https://ontology.architmitra.org/archimodel/Collaboration> rdf:type owl:Class ;
                                                            rdfs:subClassOf <https://ontology.architmitra.org/archimodel/InternalActiveStructure> ;
                                                            skos:definition "A collaboration represents an aggregate of two or more internal active structure elements, working together to perform some collective behavior." ;
                                                            skos:prefLabel "Collaboration" .


###  https://ontology.architmitra.org/archimodel/CommunicationNetwork
<https://ontology.architmitra.org/archimodel/CommunicationNetwork> rdf:type owl:Class ;
                                                                   owl:equivalentClass [ rdf:type owl:Restriction ;
                                                                                         owl:onProperty <https://ontology.architmitra.org/archimodel/aggregates> ;
                                                                                         owl:someValuesFrom <https://ontology.architmitra.org/archimodel/Device>
                                                                                       ] ,
                                                                                       [ rdf:type owl:Restriction ;
                                                                                         owl:onProperty <https://ontology.architmitra.org/archimodel/aggregates> ;
                                                                                         owl:someValuesFrom <https://ontology.architmitra.org/archimodel/SystemSoftware>
                                                                                       ] ,
                                                                                       [ rdf:type owl:Restriction ;
                                                                                         owl:onProperty <https://ontology.architmitra.org/archimodel/associatedWith> ;
                                                                                         owl:someValuesFrom <https://ontology.architmitra.org/archimodel/Device>
                                                                                       ] ,
                                                                                       [ rdf:type owl:Restriction ;
                                                                                         owl:onProperty <https://ontology.architmitra.org/archimodel/associatedWith> ;
                                                                                         owl:someValuesFrom <https://ontology.architmitra.org/archimodel/SystemSoftware>
                                                                                       ] ,
                                                                                       [ rdf:type owl:Restriction ;
                                                                                         owl:onProperty <https://ontology.architmitra.org/archimodel/realizes> ;
                                                                                         owl:someValuesFrom <https://ontology.architmitra.org/archimodel/Path>
                                                                                       ] ;
                                                                   rdfs:subClassOf <https://ontology.architmitra.org/archimodel/TechnologyActiveStructure> ;
                                                                   skos:definition "A communication network represents a set of structures that connects nodes for transmission, routing, and reception of data." ;
                                                                   skos:prefLabel "Communication Network" .


###  https://ontology.architmitra.org/archimodel/Composite
<https://ontology.architmitra.org/archimodel/Composite> rdf:type owl:Class ;
                                                        owl:equivalentClass [ rdf:type owl:Restriction ;
                                                                              owl:onProperty <https://ontology.architmitra.org/archimodel/influences> ;
                                                                              owl:someValuesFrom <https://ontology.architmitra.org/archimodel/Requirement>
                                                                            ] ,
                                                                            [ rdf:type owl:Restriction ;
                                                                              owl:onProperty <https://ontology.architmitra.org/archimodel/realizes> ;
                                                                              owl:someValuesFrom <https://ontology.architmitra.org/archimodel/Requirement>
                                                                            ] ;
                                                        rdfs:subClassOf <https://ontology.architmitra.org/archimodel/Element> ;
                                                        skos:definition "Composite elements consist of other concepts, possibly from multiple aspects or layers of the language. Grouping and location are generic composite elements. Composite elements can themselves aggregate or compose other composite elements." ;
                                                        skos:prefLabel "Composite" .


###  https://ontology.architmitra.org/archimodel/Concern
<https://ontology.architmitra.org/archimodel/Concern> rdf:type owl:Class ;
                                                      rdfs:subClassOf <https://ontology.architmitra.org/archimodel/ADElement> ;
                                                      skos:definition "A Concern is any interest in a System by one or more Stakeholders. A Concern pertains to any influence of a System in its Environment" ;
                                                      skos:prefLabel "Concern" .


###  https://ontology.architmitra.org/archimodel/Constraint
<https://ontology.architmitra.org/archimodel/Constraint> rdf:type owl:Class ;
                                                         rdfs:subClassOf <https://ontology.architmitra.org/archimodel/Requirement> ;
                                                         skos:definition "A constraint represents a factor that limits the realization of goals." .


###  https://ontology.architmitra.org/archimodel/Contract
<https://ontology.architmitra.org/archimodel/Contract> rdf:type owl:Class ;
                                                       rdfs:subClassOf <https://ontology.architmitra.org/archimodel/BusinessObject> ;
                                                       skos:definition "A contract represents a formal or informal specification of an agreement between a provider and a consumer that specifies the rights and obligations associated with a product and establishes functional and non-functional parameters for interaction." .


###  https://ontology.architmitra.org/archimodel/CourseOfAction
<https://ontology.architmitra.org/archimodel/CourseOfAction> rdf:type owl:Class ;
                                                             owl:equivalentClass [ rdf:type owl:Restriction ;
                                                                                   owl:onProperty <https://ontology.architmitra.org/archimodel/flowsTo> ;
                                                                                   owl:someValuesFrom <https://ontology.architmitra.org/archimodel/CourseOfAction>
                                                                                 ] ,
                                                                                 [ rdf:type owl:Restriction ;
                                                                                   owl:onProperty <https://ontology.architmitra.org/archimodel/realizes> ;
                                                                                   owl:someValuesFrom <https://ontology.architmitra.org/archimodel/Outcome>
                                                                                 ] ,
                                                                                 [ rdf:type owl:Restriction ;
                                                                                   owl:onProperty <https://ontology.architmitra.org/archimodel/realizes> ;
                                                                                   owl:someValuesFrom <https://ontology.architmitra.org/archimodel/Requirement>
                                                                                 ] ,
                                                                                 [ rdf:type owl:Restriction ;
                                                                                   owl:onProperty <https://ontology.architmitra.org/archimodel/serves> ;
                                                                                   owl:someValuesFrom <https://ontology.architmitra.org/archimodel/CourseOfAction>
                                                                                 ] ,
                                                                                 [ rdf:type owl:Restriction ;
                                                                                   owl:onProperty <https://ontology.architmitra.org/archimodel/triggers> ;
                                                                                   owl:someValuesFrom <https://ontology.architmitra.org/archimodel/CourseOfAction>
                                                                                 ] ;
                                                             rdfs:subClassOf <https://ontology.architmitra.org/archimodel/Behavior> ;
                                                             skos:definition "A course of action represents an approach or plan for configuring some capabilities and resources of the enterprise, undertaken to achieve a goal." ;
                                                             skos:prefLabel "Course Of Action" .


###  https://ontology.architmitra.org/archimodel/DataObject
<https://ontology.architmitra.org/archimodel/DataObject> rdf:type owl:Class ;
                                                         owl:equivalentClass [ rdf:type owl:Restriction ;
                                                                               owl:onProperty <https://ontology.architmitra.org/archimodel/realizes> ;
                                                                               owl:someValuesFrom <https://ontology.architmitra.org/archimodel/BusinessObject>
                                                                             ] ;
                                                         rdfs:subClassOf <https://ontology.architmitra.org/archimodel/PassiveStructure> ;
                                                         skos:prefLabel "Data Object" .


###  https://ontology.architmitra.org/archimodel/Deliverable
<https://ontology.architmitra.org/archimodel/Deliverable> rdf:type owl:Class ;
                                                          owl:equivalentClass [ rdf:type owl:Restriction ;
                                                                                owl:onProperty <https://ontology.architmitra.org/archimodel/realizes> ;
                                                                                owl:someValuesFrom <https://ontology.architmitra.org/archimodel/ExternalBehavior>
                                                                              ] ,
                                                                              [ rdf:type owl:Restriction ;
                                                                                owl:onProperty <https://ontology.architmitra.org/archimodel/realizes> ;
                                                                                owl:someValuesFrom <https://ontology.architmitra.org/archimodel/InternalBehavior>
                                                                              ] ,
                                                                              [ rdf:type owl:Restriction ;
                                                                                owl:onProperty <https://ontology.architmitra.org/archimodel/realizes> ;
                                                                                owl:someValuesFrom <https://ontology.architmitra.org/archimodel/Location>
                                                                              ] ,
                                                                              [ rdf:type owl:Restriction ;
                                                                                owl:onProperty <https://ontology.architmitra.org/archimodel/realizes> ;
                                                                                owl:someValuesFrom <https://ontology.architmitra.org/archimodel/Plateau>
                                                                              ] ,
                                                                              [ rdf:type owl:Restriction ;
                                                                                owl:onProperty <https://ontology.architmitra.org/archimodel/realizes> ;
                                                                                owl:someValuesFrom <https://ontology.architmitra.org/archimodel/Product>
                                                                              ] ,
                                                                              [ rdf:type owl:Restriction ;
                                                                                owl:onProperty <https://ontology.architmitra.org/archimodel/realizes> ;
                                                                                owl:someValuesFrom <https://ontology.architmitra.org/archimodel/Requirement>
                                                                              ] ,
                                                                              [ rdf:type owl:Restriction ;
                                                                                owl:onProperty <https://ontology.architmitra.org/archimodel/realizes> ;
                                                                                owl:someValuesFrom <https://ontology.architmitra.org/archimodel/Strategy>
                                                                              ] ,
                                                                              [ rdf:type owl:Restriction ;
                                                                                owl:onProperty <https://ontology.architmitra.org/archimodel/realizes> ;
                                                                                owl:someValuesFrom <https://ontology.architmitra.org/archimodel/Structure>
                                                                              ] ;
                                                          rdfs:subClassOf <https://ontology.architmitra.org/archimodel/PassiveStructure> .


###  https://ontology.architmitra.org/archimodel/Device
<https://ontology.architmitra.org/archimodel/Device> rdf:type owl:Class ;
                                                     owl:equivalentClass [ rdf:type owl:Restriction ;
                                                                           owl:onProperty <https://ontology.architmitra.org/archimodel/assignedTo> ;
                                                                           owl:someValuesFrom <https://ontology.architmitra.org/archimodel/SystemSoftware>
                                                                         ] ;
                                                     rdfs:subClassOf <https://ontology.architmitra.org/archimodel/Node> ;
                                                     skos:definition "A device represents a physical IT resource upon which system software and artifacts may be stored or deployed for execution." .


###  https://ontology.architmitra.org/archimodel/DistributionNetwork
<https://ontology.architmitra.org/archimodel/DistributionNetwork> rdf:type owl:Class ;
                                                                  owl:equivalentClass [ rdf:type owl:Restriction ;
                                                                                        owl:onProperty <https://ontology.architmitra.org/archimodel/aggregates> ;
                                                                                        owl:someValuesFrom <https://ontology.architmitra.org/archimodel/Facility>
                                                                                      ] ,
                                                                                      [ rdf:type owl:Restriction ;
                                                                                        owl:onProperty <https://ontology.architmitra.org/archimodel/associatedWith> ;
                                                                                        owl:someValuesFrom <https://ontology.architmitra.org/archimodel/Material>
                                                                                      ] ,
                                                                                      [ rdf:type owl:Restriction ;
                                                                                        owl:onProperty <https://ontology.architmitra.org/archimodel/realizes> ;
                                                                                        owl:someValuesFrom <https://ontology.architmitra.org/archimodel/Equipment>
                                                                                      ] ,
                                                                                      [ rdf:type owl:Restriction ;
                                                                                        owl:onProperty <https://ontology.architmitra.org/archimodel/realizes> ;
                                                                                        owl:someValuesFrom <https://ontology.architmitra.org/archimodel/Path>
                                                                                      ] ;
                                                                  rdfs:subClassOf <https://ontology.architmitra.org/archimodel/TechnologyActiveStructure> ;
                                                                  skos:prefLabel "Distribution Network" .


###  https://ontology.architmitra.org/archimodel/Driver
<https://ontology.architmitra.org/archimodel/Driver> rdf:type owl:Class ;
                                                     rdfs:subClassOf <https://ontology.architmitra.org/archimodel/Motivation> ;
                                                     skos:definition "A driver represents an external or internal condition that motivates an organization to define its goals and implement the changes necessary to achieve them." .


###  https://ontology.architmitra.org/archimodel/Element
<https://ontology.architmitra.org/archimodel/Element> rdf:type owl:Class ;
                                                      rdfs:subClassOf <https://ontology.architmitra.org/archimodel/ADElement> ;
                                                      skos:definition "An element is either a behavior element, a structure element, a motivation element, or a composite element" ;
                                                      skos:prefLabel "Element" .


###  https://ontology.architmitra.org/archimodel/Environment
<https://ontology.architmitra.org/archimodel/Environment> rdf:type owl:Class ;
                                                          rdfs:subClassOf <https://ontology.architmitra.org/archimodel/ADElement> ;
                                                          skos:definition "Environment determines the totality of influences upon the System throughout its life cycle. The Environment of a System is bounded by and understood through the identification and analysis of System's stakeholders and their concerns" ;
                                                          skos:prefLabel "Environment" .


###  https://ontology.architmitra.org/archimodel/Equipment
<https://ontology.architmitra.org/archimodel/Equipment> rdf:type owl:Class ;
                                                        owl:equivalentClass [ rdf:type owl:Restriction ;
                                                                              owl:onProperty <https://ontology.architmitra.org/archimodel/assignedTo> ;
                                                                              owl:someValuesFrom <https://ontology.architmitra.org/archimodel/Material>
                                                                            ] ,
                                                                            [ rdf:type owl:Restriction ;
                                                                              owl:onProperty <https://ontology.architmitra.org/archimodel/assignedTo> ;
                                                                              owl:someValuesFrom <https://ontology.architmitra.org/archimodel/TechnologyInternalBehavior>
                                                                            ] ;
                                                        rdfs:subClassOf <https://ontology.architmitra.org/archimodel/Node> .


###  https://ontology.architmitra.org/archimodel/Event
<https://ontology.architmitra.org/archimodel/Event> rdf:type owl:Class ;
                                                    owl:equivalentClass [ rdf:type owl:Restriction ;
                                                                          owl:onProperty <https://ontology.architmitra.org/archimodel/triggers> ;
                                                                          owl:someValuesFrom <https://ontology.architmitra.org/archimodel/Event>
                                                                        ] ,
                                                                        [ rdf:type owl:Restriction ;
                                                                          owl:onProperty <https://ontology.architmitra.org/archimodel/triggers> ;
                                                                          owl:someValuesFrom <https://ontology.architmitra.org/archimodel/ExternalBehavior>
                                                                        ] ,
                                                                        [ rdf:type owl:Restriction ;
                                                                          owl:onProperty <https://ontology.architmitra.org/archimodel/triggers> ;
                                                                          owl:someValuesFrom <https://ontology.architmitra.org/archimodel/InternalBehavior>
                                                                        ] ;
                                                    rdfs:subClassOf <https://ontology.architmitra.org/archimodel/Behavior> ;
                                                    skos:definition "An event represents a state change." ;
                                                    skos:prefLabel "Event" .


###  https://ontology.architmitra.org/archimodel/ExternalActiveStructure
<https://ontology.architmitra.org/archimodel/ExternalActiveStructure> rdf:type owl:Class ;
                                                                      owl:equivalentClass [ rdf:type owl:Restriction ;
                                                                                            owl:onProperty <https://ontology.architmitra.org/archimodel/assignedTo> ;
                                                                                            owl:someValuesFrom <https://ontology.architmitra.org/archimodel/ExternalBehavior>
                                                                                          ] ,
                                                                                          [ rdf:type owl:Restriction ;
                                                                                            owl:onProperty <https://ontology.architmitra.org/archimodel/serves> ;
                                                                                            owl:someValuesFrom <https://ontology.architmitra.org/archimodel/InternalActiveStructure>
                                                                                          ] ;
                                                                      rdfs:subClassOf <https://ontology.architmitra.org/archimodel/ActiveStructure> ;
                                                                      skos:definition "An external active structure element, called an interface, represents a point of access where one or more services are provided to the environment." ;
                                                                      skos:prefLabel "External Active Structure" .


###  https://ontology.architmitra.org/archimodel/ExternalBehavior
<https://ontology.architmitra.org/archimodel/ExternalBehavior> rdf:type owl:Class ;
                                                               owl:equivalentClass [ rdf:type owl:Restriction ;
                                                                                     owl:onProperty <https://ontology.architmitra.org/archimodel/realizes> ;
                                                                                     owl:someValuesFrom <https://ontology.architmitra.org/archimodel/Strategy>
                                                                                   ] ,
                                                                                   [ rdf:type owl:Restriction ;
                                                                                     owl:onProperty <https://ontology.architmitra.org/archimodel/serves> ;
                                                                                     owl:someValuesFrom <https://ontology.architmitra.org/archimodel/InternalActiveStructure>
                                                                                   ] ,
                                                                                   [ rdf:type owl:Restriction ;
                                                                                     owl:onProperty <https://ontology.architmitra.org/archimodel/serves> ;
                                                                                     owl:someValuesFrom <https://ontology.architmitra.org/archimodel/InternalBehavior>
                                                                                   ] ,
                                                                                   [ rdf:type owl:Restriction ;
                                                                                     owl:onProperty <https://ontology.architmitra.org/archimodel/triggers> ;
                                                                                     owl:someValuesFrom <https://ontology.architmitra.org/archimodel/Event>
                                                                                   ] ,
                                                                                   [ rdf:type owl:Restriction ;
                                                                                     owl:onProperty <https://ontology.architmitra.org/archimodel/triggers> ;
                                                                                     owl:someValuesFrom <https://ontology.architmitra.org/archimodel/ExternalBehavior>
                                                                                   ] ;
                                                               rdfs:subClassOf <https://ontology.architmitra.org/archimodel/Behavior> ;
                                                               skos:definition "An external behavior element, called a service, represents an explicitly defined exposed behavior." ;
                                                               skos:prefLabel "External Behavior" .


###  https://ontology.architmitra.org/archimodel/Facility
<https://ontology.architmitra.org/archimodel/Facility> rdf:type owl:Class ;
                                                       owl:equivalentClass [ rdf:type owl:Restriction ;
                                                                             owl:onProperty <https://ontology.architmitra.org/archimodel/assignedTo> ;
                                                                             owl:someValuesFrom <https://ontology.architmitra.org/archimodel/Node>
                                                                           ] ,
                                                                           [ rdf:type owl:Restriction ;
                                                                             owl:onProperty <https://ontology.architmitra.org/archimodel/assignedTo> ;
                                                                             owl:someValuesFrom <https://ontology.architmitra.org/archimodel/TechnologyInternalActiveStructure>
                                                                           ] ,
                                                                           [ rdf:type owl:Restriction ;
                                                                             owl:onProperty <https://ontology.architmitra.org/archimodel/associatedWith> ;
                                                                             owl:someValuesFrom <https://ontology.architmitra.org/archimodel/DistributionNetwork>
                                                                           ] ;
                                                       rdfs:subClassOf <https://ontology.architmitra.org/archimodel/Node> .


###  https://ontology.architmitra.org/archimodel/Function
<https://ontology.architmitra.org/archimodel/Function> rdf:type owl:Class ;
                                                       owl:equivalentClass [ rdf:type owl:Restriction ;
                                                                             owl:onProperty <https://ontology.architmitra.org/archimodel/aggregates> ;
                                                                             owl:someValuesFrom <https://ontology.architmitra.org/archimodel/Function>
                                                                           ] ,
                                                                           [ rdf:type owl:Restriction ;
                                                                             owl:onProperty <https://ontology.architmitra.org/archimodel/composedOf> ;
                                                                             owl:someValuesFrom <https://ontology.architmitra.org/archimodel/Function>
                                                                           ] ,
                                                                           [ rdf:type owl:Restriction ;
                                                                             owl:onProperty <https://ontology.architmitra.org/archimodel/specializes> ;
                                                                             owl:someValuesFrom <https://ontology.architmitra.org/archimodel/Function>
                                                                           ] ;
                                                       rdfs:subClassOf <https://ontology.architmitra.org/archimodel/InternalBehavior> ;
                                                       skos:definition "A function represents a collection of behavior based on specific criteria, such as required resources, competencies, or location." ;
                                                       skos:prefLabel "Function" .


###  https://ontology.architmitra.org/archimodel/Gap
<https://ontology.architmitra.org/archimodel/Gap> rdf:type owl:Class ;
                                                  owl:equivalentClass [ rdf:type owl:Restriction ;
                                                                        owl:onProperty <https://ontology.architmitra.org/archimodel/associatedWith> ;
                                                                        owl:someValuesFrom <https://ontology.architmitra.org/archimodel/Plateau>
                                                                      ] ;
                                                  rdfs:subClassOf <https://ontology.architmitra.org/archimodel/PassiveStructure> .


###  https://ontology.architmitra.org/archimodel/Goal
<https://ontology.architmitra.org/archimodel/Goal> rdf:type owl:Class ;
                                                   owl:equivalentClass [ rdf:type owl:Restriction ;
                                                                         owl:onProperty <https://ontology.architmitra.org/archimodel/associatedWith> ;
                                                                         owl:someValuesFrom <https://ontology.architmitra.org/archimodel/Assessment>
                                                                       ] ,
                                                                       [ rdf:type owl:Restriction ;
                                                                         owl:onProperty <https://ontology.architmitra.org/archimodel/associatedWith> ;
                                                                         owl:someValuesFrom <https://ontology.architmitra.org/archimodel/Driver>
                                                                       ] ;
                                                   rdfs:subClassOf <https://ontology.architmitra.org/archimodel/Motivation> ,
                                                                   [ rdf:type owl:Restriction ;
                                                                     owl:onProperty <https://ontology.architmitra.org/archimodel/associatedWith> ;
                                                                     owl:someValuesFrom <https://ontology.architmitra.org/archimodel/Assessment>
                                                                   ] ,
                                                                   [ rdf:type owl:Restriction ;
                                                                     owl:onProperty <https://ontology.architmitra.org/archimodel/associatedWith> ;
                                                                     owl:someValuesFrom <https://ontology.architmitra.org/archimodel/Driver>
                                                                   ] ;
                                                   skos:definition "A goal represents a high-level statement of intent, direction, or desired end state for an organization and its stakeholders." .


###  https://ontology.architmitra.org/archimodel/Grouping
<https://ontology.architmitra.org/archimodel/Grouping> rdf:type owl:Class ;
                                                       rdfs:subClassOf <https://ontology.architmitra.org/archimodel/Composite> ;
                                                       skos:definition "The grouping element aggregates or composes concepts that belong together based on some common characteristic." ;
                                                       skos:prefLabel "Grouping" .


###  https://ontology.architmitra.org/archimodel/ImplementationEvent
<https://ontology.architmitra.org/archimodel/ImplementationEvent> rdf:type owl:Class ;
                                                                  owl:equivalentClass [ rdf:type owl:Restriction ;
                                                                                        owl:onProperty <https://ontology.architmitra.org/archimodel/accesses> ;
                                                                                        owl:someValuesFrom <https://ontology.architmitra.org/archimodel/Deliverable>
                                                                                      ] ,
                                                                                      [ rdf:type owl:Restriction ;
                                                                                        owl:onProperty <https://ontology.architmitra.org/archimodel/accesses> ;
                                                                                        owl:someValuesFrom <https://ontology.architmitra.org/archimodel/WorkPackage>
                                                                                      ] ,
                                                                                      [ rdf:type owl:Restriction ;
                                                                                        owl:onProperty <https://ontology.architmitra.org/archimodel/realizes> ;
                                                                                        owl:someValuesFrom <https://ontology.architmitra.org/archimodel/ExternalBehavior>
                                                                                      ] ,
                                                                                      [ rdf:type owl:Restriction ;
                                                                                        owl:onProperty <https://ontology.architmitra.org/archimodel/realizes> ;
                                                                                        owl:someValuesFrom <https://ontology.architmitra.org/archimodel/InternalBehavior>
                                                                                      ] ,
                                                                                      [ rdf:type owl:Restriction ;
                                                                                        owl:onProperty <https://ontology.architmitra.org/archimodel/realizes> ;
                                                                                        owl:someValuesFrom <https://ontology.architmitra.org/archimodel/Location>
                                                                                      ] ,
                                                                                      [ rdf:type owl:Restriction ;
                                                                                        owl:onProperty <https://ontology.architmitra.org/archimodel/realizes> ;
                                                                                        owl:someValuesFrom <https://ontology.architmitra.org/archimodel/Product>
                                                                                      ] ,
                                                                                      [ rdf:type owl:Restriction ;
                                                                                        owl:onProperty <https://ontology.architmitra.org/archimodel/realizes> ;
                                                                                        owl:someValuesFrom <https://ontology.architmitra.org/archimodel/Strategy>
                                                                                      ] ,
                                                                                      [ rdf:type owl:Restriction ;
                                                                                        owl:onProperty <https://ontology.architmitra.org/archimodel/triggers> ;
                                                                                        owl:someValuesFrom <https://ontology.architmitra.org/archimodel/ImplementationEvent>
                                                                                      ] ,
                                                                                      [ rdf:type owl:Restriction ;
                                                                                        owl:onProperty <https://ontology.architmitra.org/archimodel/triggers> ;
                                                                                        owl:someValuesFrom <https://ontology.architmitra.org/archimodel/Plateau>
                                                                                      ] ;
                                                                  rdfs:subClassOf <https://ontology.architmitra.org/archimodel/Event> .


###  https://ontology.architmitra.org/archimodel/Interaction
<https://ontology.architmitra.org/archimodel/Interaction> rdf:type owl:Class ;
                                                          owl:equivalentClass [ rdf:type owl:Restriction ;
                                                                                owl:onProperty <https://ontology.architmitra.org/archimodel/aggregates> ;
                                                                                owl:someValuesFrom <https://ontology.architmitra.org/archimodel/Interaction>
                                                                              ] ,
                                                                              [ rdf:type owl:Restriction ;
                                                                                owl:onProperty <https://ontology.architmitra.org/archimodel/composedOf> ;
                                                                                owl:someValuesFrom <https://ontology.architmitra.org/archimodel/Interaction>
                                                                              ] ,
                                                                              [ rdf:type owl:Restriction ;
                                                                                owl:onProperty <https://ontology.architmitra.org/archimodel/specializes> ;
                                                                                owl:someValuesFrom <https://ontology.architmitra.org/archimodel/Interaction>
                                                                              ] ;
                                                          rdfs:subClassOf <https://ontology.architmitra.org/archimodel/InternalBehavior> ;
                                                          skos:definition "An interaction represents a unit of collective behavior that must be performed by two or more internal active structure elements, either assigned directly or aggregated in a collaboration." ;
                                                          skos:prefLabel "Interaction" .


###  https://ontology.architmitra.org/archimodel/InternalActiveStructure
<https://ontology.architmitra.org/archimodel/InternalActiveStructure> rdf:type owl:Class ;
                                                                      owl:equivalentClass [ rdf:type owl:Restriction ;
                                                                                            owl:onProperty <https://ontology.architmitra.org/archimodel/aggregates> ;
                                                                                            owl:someValuesFrom <https://ontology.architmitra.org/archimodel/InternalActiveStructure>
                                                                                          ] ,
                                                                                          [ rdf:type owl:Restriction ;
                                                                                            owl:onProperty <https://ontology.architmitra.org/archimodel/assignedTo> ;
                                                                                            owl:someValuesFrom <https://ontology.architmitra.org/archimodel/Event>
                                                                                          ] ,
                                                                                          [ rdf:type owl:Restriction ;
                                                                                            owl:onProperty <https://ontology.architmitra.org/archimodel/assignedTo> ;
                                                                                            owl:someValuesFrom <https://ontology.architmitra.org/archimodel/InternalBehavior>
                                                                                          ] ,
                                                                                          [ rdf:type owl:Restriction ;
                                                                                            owl:onProperty <https://ontology.architmitra.org/archimodel/composedOf> ;
                                                                                            owl:someValuesFrom <https://ontology.architmitra.org/archimodel/ExternalActiveStructure>
                                                                                          ] ,
                                                                                          [ rdf:type owl:Restriction ;
                                                                                            owl:onProperty <https://ontology.architmitra.org/archimodel/composedOf> ;
                                                                                            owl:someValuesFrom <https://ontology.architmitra.org/archimodel/InternalActiveStructure>
                                                                                          ] ;
                                                                      rdfs:subClassOf <https://ontology.architmitra.org/archimodel/ActiveStructure> ;
                                                                      skos:definition "An internal active structure element represents an entity that is capable of performing behavior." ;
                                                                      skos:prefLabel "Internal Active Structure" .


###  https://ontology.architmitra.org/archimodel/InternalBehavior
<https://ontology.architmitra.org/archimodel/InternalBehavior> rdf:type owl:Class ;
                                                               owl:equivalentClass [ rdf:type owl:Restriction ;
                                                                                     owl:onProperty <https://ontology.architmitra.org/archimodel/realizes> ;
                                                                                     owl:someValuesFrom <https://ontology.architmitra.org/archimodel/ExternalBehavior>
                                                                                   ] ,
                                                                                   [ rdf:type owl:Restriction ;
                                                                                     owl:onProperty <https://ontology.architmitra.org/archimodel/realizes> ;
                                                                                     owl:someValuesFrom <https://ontology.architmitra.org/archimodel/Strategy>
                                                                                   ] ,
                                                                                   [ rdf:type owl:Restriction ;
                                                                                     owl:onProperty <https://ontology.architmitra.org/archimodel/serves> ;
                                                                                     owl:someValuesFrom <https://ontology.architmitra.org/archimodel/TechnologyInternalBehavior>
                                                                                   ] ,
                                                                                   [ rdf:type owl:Restriction ;
                                                                                     owl:onProperty <https://ontology.architmitra.org/archimodel/triggers> ;
                                                                                     owl:someValuesFrom <https://ontology.architmitra.org/archimodel/Event>
                                                                                   ] ,
                                                                                   [ rdf:type owl:Restriction ;
                                                                                     owl:onProperty <https://ontology.architmitra.org/archimodel/triggers> ;
                                                                                     owl:someValuesFrom <https://ontology.architmitra.org/archimodel/InternalBehavior>
                                                                                   ] ;
                                                               rdfs:subClassOf <https://ontology.architmitra.org/archimodel/Behavior> ;
                                                               skos:definition "An internal behavior element represents a unit of activity that can be performed by one or more active structure elements." ;
                                                               skos:prefLabel "Internal Behavior" .


###  https://ontology.architmitra.org/archimodel/Location
<https://ontology.architmitra.org/archimodel/Location> rdf:type owl:Class ;
                                                       rdfs:subClassOf <https://ontology.architmitra.org/archimodel/Composite> ;
                                                       skos:definition "A location represents a conceptual or physical place or position where concepts are located (e.g., structure elements) or performed (e.g., behavior elements)." ;
                                                       skos:prefLabel "Location" .


###  https://ontology.architmitra.org/archimodel/Material
<https://ontology.architmitra.org/archimodel/Material> rdf:type owl:Class ;
                                                       rdfs:subClassOf <https://ontology.architmitra.org/archimodel/TechnologyObject> .


###  https://ontology.architmitra.org/archimodel/Meaning
<https://ontology.architmitra.org/archimodel/Meaning> rdf:type owl:Class ;
                                                      owl:equivalentClass [ rdf:type owl:Restriction ;
                                                                            owl:onProperty <https://ontology.architmitra.org/archimodel/associatedWith> ;
                                                                            owl:someValuesFrom <https://ontology.architmitra.org/archimodel/Behavior>
                                                                          ] ,
                                                                          [ rdf:type owl:Restriction ;
                                                                            owl:onProperty <https://ontology.architmitra.org/archimodel/associatedWith> ;
                                                                            owl:someValuesFrom <https://ontology.architmitra.org/archimodel/Composite>
                                                                          ] ,
                                                                          [ rdf:type owl:Restriction ;
                                                                            owl:onProperty <https://ontology.architmitra.org/archimodel/associatedWith> ;
                                                                            owl:someValuesFrom <https://ontology.architmitra.org/archimodel/Structure>
                                                                          ] ;
                                                      rdfs:subClassOf <https://ontology.architmitra.org/archimodel/Motivation> ;
                                                      skos:definition "Meaning represents the knowledge or expertise present in, or the interpretation given to, a concept in a particular context." .


###  https://ontology.architmitra.org/archimodel/ModelKind
<https://ontology.architmitra.org/archimodel/ModelKind> rdf:type owl:Class ;
                                                        rdfs:subClassOf <https://ontology.architmitra.org/archimodel/ADElement> ;
                                                        skos:definition """The conventions governing a model are specified by its Model Kind
A Model Kind specifies:
- Languages
- notations
- conventions
- modeling
- techniques
- analytical methods and/or other operations""" ;
                                                        skos:prefLabel "Model Kind" .


###  https://ontology.architmitra.org/archimodel/Motivation
<https://ontology.architmitra.org/archimodel/Motivation> rdf:type owl:Class ;
                                                         owl:equivalentClass [ rdf:type owl:Restriction ;
                                                                               owl:onProperty <https://ontology.architmitra.org/archimodel/influences> ;
                                                                               owl:someValuesFrom <https://ontology.architmitra.org/archimodel/Motivation>
                                                                             ] ;
                                                         rdfs:subClassOf <https://ontology.architmitra.org/archimodel/Element> ;
                                                         skos:definition "A motivation element represents the context of or reason behind the architecture of an enterprise." ;
                                                         skos:prefLabel "Motivation" .


###  https://ontology.architmitra.org/archimodel/Node
<https://ontology.architmitra.org/archimodel/Node> rdf:type owl:Class ;
                                                   owl:equivalentClass [ rdf:type owl:Restriction ;
                                                                         owl:onProperty <https://ontology.architmitra.org/archimodel/realizes> ;
                                                                         owl:someValuesFrom <https://ontology.architmitra.org/archimodel/Node>
                                                                       ] ;
                                                   rdfs:subClassOf <https://ontology.architmitra.org/archimodel/TechnologyInternalActiveStructure> ;
                                                   skos:definition "A node represents a computational or physical resource that hosts, manipulates, or interacts with other computational or physical resources." .


###  https://ontology.architmitra.org/archimodel/Outcome
<https://ontology.architmitra.org/archimodel/Outcome> rdf:type owl:Class ;
                                                      owl:equivalentClass [ rdf:type owl:Restriction ;
                                                                            owl:onProperty <https://ontology.architmitra.org/archimodel/associatedWith> ;
                                                                            owl:someValuesFrom <https://ontology.architmitra.org/archimodel/Goal>
                                                                          ] ,
                                                                          [ rdf:type owl:Restriction ;
                                                                            owl:onProperty <https://ontology.architmitra.org/archimodel/associatedWith> ;
                                                                            owl:someValuesFrom <https://ontology.architmitra.org/archimodel/Value>
                                                                          ] ,
                                                                          [ rdf:type owl:Restriction ;
                                                                            owl:onProperty <https://ontology.architmitra.org/archimodel/realizes> ;
                                                                            owl:someValuesFrom <https://ontology.architmitra.org/archimodel/Value>
                                                                          ] ;
                                                      rdfs:subClassOf <https://ontology.architmitra.org/archimodel/Motivation> ;
                                                      skos:definition "An outcome represents an end result." .


###  https://ontology.architmitra.org/archimodel/PassiveStructure
<https://ontology.architmitra.org/archimodel/PassiveStructure> rdf:type owl:Class ;
                                                               owl:equivalentClass [ rdf:type owl:Restriction ;
                                                                                     owl:onProperty <https://ontology.architmitra.org/archimodel/realizes> ;
                                                                                     owl:someValuesFrom <https://ontology.architmitra.org/archimodel/Resource>
                                                                                   ] ;
                                                               rdfs:subClassOf <https://ontology.architmitra.org/archimodel/Structure> ;
                                                               skos:definition "A passive structure element represents an element on which behavior is performed. A passive structure element is a structural element that cannot perform behavior. Active structure elements can perform behavior on passive structure elements. Passive structure elements are often information or data objects, but they can also represent physical objects." ;
                                                               skos:prefLabel "Passive Structure" .


###  https://ontology.architmitra.org/archimodel/Path
<https://ontology.architmitra.org/archimodel/Path> rdf:type owl:Class ;
                                                   owl:equivalentClass [ rdf:type owl:Restriction ;
                                                                         owl:onProperty <https://ontology.architmitra.org/archimodel/aggregates> ;
                                                                         owl:someValuesFrom <https://ontology.architmitra.org/archimodel/TechnologyInternalActiveStructure>
                                                                       ] ,
                                                                       [ rdf:type owl:Restriction ;
                                                                         owl:onProperty <https://ontology.architmitra.org/archimodel/associatedWith> ;
                                                                         owl:someValuesFrom <https://ontology.architmitra.org/archimodel/TechnologyInternalActiveStructure>
                                                                       ] ;
                                                   rdfs:subClassOf <https://ontology.architmitra.org/archimodel/TechnologyActiveStructure> ;
                                                   skos:definition "A path represents a link between two or more nodes, through which these nodes can exchange data, energy, or material." .


###  https://ontology.architmitra.org/archimodel/Plateau
<https://ontology.architmitra.org/archimodel/Plateau> rdf:type owl:Class ;
                                                      owl:equivalentClass [ rdf:type owl:Restriction ;
                                                                            owl:onProperty <https://ontology.architmitra.org/archimodel/composedOf> ;
                                                                            owl:someValuesFrom <https://ontology.architmitra.org/archimodel/Goal>
                                                                          ] ,
                                                                          [ rdf:type owl:Restriction ;
                                                                            owl:onProperty <https://ontology.architmitra.org/archimodel/composedOf> ;
                                                                            owl:someValuesFrom <https://ontology.architmitra.org/archimodel/Requirement>
                                                                          ] ,
                                                                          [ rdf:type owl:Restriction ;
                                                                            owl:onProperty <https://ontology.architmitra.org/archimodel/realizes> ;
                                                                            owl:someValuesFrom <https://ontology.architmitra.org/archimodel/Structure>
                                                                          ] ,
                                                                          [ rdf:type owl:Restriction ;
                                                                            owl:onProperty <https://ontology.architmitra.org/archimodel/triggers> ;
                                                                            owl:someValuesFrom <https://ontology.architmitra.org/archimodel/ImplementationEvent>
                                                                          ] ,
                                                                          [ rdf:type owl:Restriction ;
                                                                            owl:onProperty <https://ontology.architmitra.org/archimodel/triggers> ;
                                                                            owl:someValuesFrom <https://ontology.architmitra.org/archimodel/Plateau>
                                                                          ] ;
                                                      rdfs:subClassOf <https://ontology.architmitra.org/archimodel/Composite> .


###  https://ontology.architmitra.org/archimodel/Principle
<https://ontology.architmitra.org/archimodel/Principle> rdf:type owl:Class ;
                                                        owl:equivalentClass [ rdf:type owl:Restriction ;
                                                                              owl:onProperty <https://ontology.architmitra.org/archimodel/realizes> ;
                                                                              owl:someValuesFrom <https://ontology.architmitra.org/archimodel/Outcome>
                                                                            ] ;
                                                        rdfs:subClassOf <https://ontology.architmitra.org/archimodel/Motivation> ;
                                                        skos:definition "A principle represents a statement of intent defining a general property that applies to any system in a certain context in the architecture." .


###  https://ontology.architmitra.org/archimodel/Process
<https://ontology.architmitra.org/archimodel/Process> rdf:type owl:Class ;
                                                      owl:equivalentClass [ rdf:type owl:Restriction ;
                                                                            owl:onProperty <https://ontology.architmitra.org/archimodel/aggregates> ;
                                                                            owl:someValuesFrom <https://ontology.architmitra.org/archimodel/Process>
                                                                          ] ,
                                                                          [ rdf:type owl:Restriction ;
                                                                            owl:onProperty <https://ontology.architmitra.org/archimodel/composedOf> ;
                                                                            owl:someValuesFrom <https://ontology.architmitra.org/archimodel/Process>
                                                                          ] ,
                                                                          [ rdf:type owl:Restriction ;
                                                                            owl:onProperty <https://ontology.architmitra.org/archimodel/specializes> ;
                                                                            owl:someValuesFrom <https://ontology.architmitra.org/archimodel/Process>
                                                                          ] ;
                                                      rdfs:subClassOf <https://ontology.architmitra.org/archimodel/InternalBehavior> ;
                                                      skos:definition "A process represents a sequence of behaviors that achieves a specific result." ;
                                                      skos:prefLabel "Process" .


###  https://ontology.architmitra.org/archimodel/Product
<https://ontology.architmitra.org/archimodel/Product> rdf:type owl:Class ;
                                                      owl:equivalentClass [ rdf:type owl:Restriction ;
                                                                            owl:onProperty <https://ontology.architmitra.org/archimodel/aggregates> ;
                                                                            owl:someValuesFrom <https://ontology.architmitra.org/archimodel/BusinessPassiveStructure>
                                                                          ] ,
                                                                          [ rdf:type owl:Restriction ;
                                                                            owl:onProperty <https://ontology.architmitra.org/archimodel/aggregates> ;
                                                                            owl:someValuesFrom <https://ontology.architmitra.org/archimodel/BusinessService>
                                                                          ] ,
                                                                          [ rdf:type owl:Restriction ;
                                                                            owl:onProperty <https://ontology.architmitra.org/archimodel/composedOf> ;
                                                                            owl:someValuesFrom <https://ontology.architmitra.org/archimodel/BusinessPassiveStructure>
                                                                          ] ,
                                                                          [ rdf:type owl:Restriction ;
                                                                            owl:onProperty <https://ontology.architmitra.org/archimodel/composedOf> ;
                                                                            owl:someValuesFrom <https://ontology.architmitra.org/archimodel/BusinessService>
                                                                          ] ;
                                                      rdfs:subClassOf <https://ontology.architmitra.org/archimodel/Composite> ;
                                                      skos:definition "A product represents a coherent collection of services and/or passive structure elements, accompanied by a contract/set of agreements, which is offered as a whole to (internal or external) customers." .


###  https://ontology.architmitra.org/archimodel/Representation
<https://ontology.architmitra.org/archimodel/Representation> rdf:type owl:Class ;
                                                             owl:equivalentClass [ rdf:type owl:Restriction ;
                                                                                   owl:onProperty <https://ontology.architmitra.org/archimodel/realizes> ;
                                                                                   owl:someValuesFrom <https://ontology.architmitra.org/archimodel/BusinessObject>
                                                                                 ] ;
                                                             rdfs:subClassOf <https://ontology.architmitra.org/archimodel/BusinessPassiveStructure> ;
                                                             skos:definition "A representation represents a perceptible form of the information carried by a business object." .


###  https://ontology.architmitra.org/archimodel/Requirement
<https://ontology.architmitra.org/archimodel/Requirement> rdf:type owl:Class ;
                                                          owl:equivalentClass [ rdf:type owl:Restriction ;
                                                                                owl:onProperty <https://ontology.architmitra.org/archimodel/realizes> ;
                                                                                owl:someValuesFrom <https://ontology.architmitra.org/archimodel/Outcome>
                                                                              ] ,
                                                                              [ rdf:type owl:Restriction ;
                                                                                owl:onProperty <https://ontology.architmitra.org/archimodel/realizes> ;
                                                                                owl:someValuesFrom <https://ontology.architmitra.org/archimodel/Principle>
                                                                              ] ;
                                                          rdfs:subClassOf <https://ontology.architmitra.org/archimodel/Motivation> ;
                                                          skos:definition "A requirement represents a statement of need defining a property that applies to a specific system as described by the architecture." .


###  https://ontology.architmitra.org/archimodel/Resource
<https://ontology.architmitra.org/archimodel/Resource> rdf:type owl:Class ;
                                                       owl:equivalentClass [ rdf:type owl:Restriction ;
                                                                             owl:onProperty <https://ontology.architmitra.org/archimodel/assignedTo> ;
                                                                             owl:someValuesFrom <https://ontology.architmitra.org/archimodel/Strategy>
                                                                           ] ;
                                                       rdfs:subClassOf <https://ontology.architmitra.org/archimodel/Structure> ;
                                                       skos:definition "A resource represents an asset owned or controlled by an individual or organization." .


###  https://ontology.architmitra.org/archimodel/Stakeholder
<https://ontology.architmitra.org/archimodel/Stakeholder> rdf:type owl:Class ;
                                                          owl:equivalentClass [ rdf:type owl:Restriction ;
                                                                                owl:onProperty <https://ontology.architmitra.org/archimodel/hasConcern> ;
                                                                                owl:someValuesFrom <https://ontology.architmitra.org/archimodel/Concern>
                                                                              ] ,
                                                                              [ rdf:type owl:Restriction ;
                                                                                owl:onProperty <https://ontology.architmitra.org/archimodel/hasInterestIn> ;
                                                                                owl:someValuesFrom <https://ontology.architmitra.org/archimodel/SystemOfInterest>
                                                                              ] ;
                                                          rdfs:subClassOf <https://ontology.architmitra.org/archimodel/Motivation> ;
                                                          skos:definition "A stakeholder represents the role of an individual, team, or organization (or classes thereof) that represents their interests in the effects of the architecture." .


###  https://ontology.architmitra.org/archimodel/Strategy
<https://ontology.architmitra.org/archimodel/Strategy> rdf:type owl:Class ;
                                                       owl:equivalentClass [ rdf:type owl:Restriction ;
                                                                             owl:onProperty <https://ontology.architmitra.org/archimodel/flowsTo> ;
                                                                             owl:someValuesFrom <https://ontology.architmitra.org/archimodel/Strategy>
                                                                           ] ,
                                                                           [ rdf:type owl:Restriction ;
                                                                             owl:onProperty <https://ontology.architmitra.org/archimodel/realizes> ;
                                                                             owl:someValuesFrom <https://ontology.architmitra.org/archimodel/CourseOfAction>
                                                                           ] ,
                                                                           [ rdf:type owl:Restriction ;
                                                                             owl:onProperty <https://ontology.architmitra.org/archimodel/realizes> ;
                                                                             owl:someValuesFrom <https://ontology.architmitra.org/archimodel/Requirement>
                                                                           ] ,
                                                                           [ rdf:type owl:Restriction ;
                                                                             owl:onProperty <https://ontology.architmitra.org/archimodel/serves> ;
                                                                             owl:someValuesFrom <https://ontology.architmitra.org/archimodel/CourseOfAction>
                                                                           ] ,
                                                                           [ rdf:type owl:Restriction ;
                                                                             owl:onProperty <https://ontology.architmitra.org/archimodel/serves> ;
                                                                             owl:someValuesFrom <https://ontology.architmitra.org/archimodel/Strategy>
                                                                           ] ,
                                                                           [ rdf:type owl:Restriction ;
                                                                             owl:onProperty <https://ontology.architmitra.org/archimodel/triggers> ;
                                                                             owl:someValuesFrom <https://ontology.architmitra.org/archimodel/Strategy>
                                                                           ] ;
                                                       rdfs:subClassOf <https://ontology.architmitra.org/archimodel/Behavior> ;
                                                       skos:definition "The strategy elements are typically used to model the strategic direction and choices of an enterprise, as far as the impact on its architecture is concerned. They can be used to express how the enterprise wants to create value for its stakeholders, the capabilities it needs for that, the resources needed to support these capabilities, and how it plans to configure and use these capabilities and resources to achieve its aims (see Chapter 6). Strategy elements are used to model the strategic direction and choices of the enterprise, whereas Business Layer elements (Chapter 8) are used to model the operational organization of an enterprise." .


###  https://ontology.architmitra.org/archimodel/Structure
<https://ontology.architmitra.org/archimodel/Structure> rdf:type owl:Class ;
                                                        owl:equivalentClass [ rdf:type owl:Restriction ;
                                                                              owl:onProperty <https://ontology.architmitra.org/archimodel/influences> ;
                                                                              owl:someValuesFrom <https://ontology.architmitra.org/archimodel/Requirement>
                                                                            ] ,
                                                                            [ rdf:type owl:Restriction ;
                                                                              owl:onProperty <https://ontology.architmitra.org/archimodel/realizes> ;
                                                                              owl:someValuesFrom <https://ontology.architmitra.org/archimodel/Requirement>
                                                                            ] ;
                                                        rdfs:subClassOf <https://ontology.architmitra.org/archimodel/Element> ;
                                                        skos:definition "Represents Elements that can and cannot act" ;
                                                        skos:prefLabel "Structure" .


###  https://ontology.architmitra.org/archimodel/SystemOfInterest
<https://ontology.architmitra.org/archimodel/SystemOfInterest> rdf:type owl:Class ;
                                                               rdfs:subClassOf gist:System ;
                                                               skos:definition "StakeHolders have interests in a System Of Interest; those interests are called Concerns" ;
                                                               skos:prefLabel "System Of Interest" .


###  https://ontology.architmitra.org/archimodel/SystemSoftware
<https://ontology.architmitra.org/archimodel/SystemSoftware> rdf:type owl:Class ;
                                                             owl:equivalentClass [ rdf:type owl:Restriction ;
                                                                                   owl:onProperty <https://ontology.architmitra.org/archimodel/assignedTo> ;
                                                                                   owl:someValuesFrom <https://ontology.architmitra.org/archimodel/SystemSoftware>
                                                                                 ] ;
                                                             rdfs:subClassOf <https://ontology.architmitra.org/archimodel/Node> ;
                                                             skos:definition "System software represents software that provides or contributes to an environment for storing, executing, and using software or data deployed within it." ;
                                                             skos:prefLabel "System Software" .


###  https://ontology.architmitra.org/archimodel/TechnologyActiveStructure
<https://ontology.architmitra.org/archimodel/TechnologyActiveStructure> rdf:type owl:Class ;
                                                                        rdfs:subClassOf <https://ontology.architmitra.org/archimodel/ActiveStructure> ;
                                                                        skos:prefLabel "Technology Active Structure" .


###  https://ontology.architmitra.org/archimodel/TechnologyCollaboration
<https://ontology.architmitra.org/archimodel/TechnologyCollaboration> rdf:type owl:Class ;
                                                                      owl:equivalentClass [ rdf:type owl:Restriction ;
                                                                                            owl:onProperty <https://ontology.architmitra.org/archimodel/aggregates> ;
                                                                                            owl:someValuesFrom <https://ontology.architmitra.org/archimodel/TechnologyInternalActiveStructure>
                                                                                          ] ;
                                                                      rdfs:subClassOf <https://ontology.architmitra.org/archimodel/TechnologyInternalActiveStructure> ;
                                                                      skos:definition "A technology collaboration represents an aggregate of two or more technology internal active structure elements that work together to perform collective technology behavior." ;
                                                                      skos:prefLabel "Technology Collaboration" .


###  https://ontology.architmitra.org/archimodel/TechnologyEvent
<https://ontology.architmitra.org/archimodel/TechnologyEvent> rdf:type owl:Class ;
                                                              owl:equivalentClass [ rdf:type owl:Restriction ;
                                                                                    owl:onProperty <https://ontology.architmitra.org/archimodel/accesses> ;
                                                                                    owl:someValuesFrom <https://ontology.architmitra.org/archimodel/TechnologyObject>
                                                                                  ] ,
                                                                                  [ rdf:type owl:Restriction ;
                                                                                    owl:onProperty <https://ontology.architmitra.org/archimodel/realizes> ;
                                                                                    owl:someValuesFrom <https://ontology.architmitra.org/archimodel/ApplicationEvent>
                                                                                  ] ,
                                                                                  [ rdf:type owl:Restriction ;
                                                                                    owl:onProperty <https://ontology.architmitra.org/archimodel/realizes> ;
                                                                                    owl:someValuesFrom <https://ontology.architmitra.org/archimodel/BusinessEvent>
                                                                                  ] ,
                                                                                  [ rdf:type owl:Restriction ;
                                                                                    owl:onProperty <https://ontology.architmitra.org/archimodel/triggers> ;
                                                                                    owl:someValuesFrom <https://ontology.architmitra.org/archimodel/TechnologyEvent>
                                                                                  ] ,
                                                                                  [ rdf:type owl:Restriction ;
                                                                                    owl:onProperty <https://ontology.architmitra.org/archimodel/triggers> ;
                                                                                    owl:someValuesFrom <https://ontology.architmitra.org/archimodel/TechnologyInternalBehavior>
                                                                                  ] ,
                                                                                  [ rdf:type owl:Restriction ;
                                                                                    owl:onProperty <https://ontology.architmitra.org/archimodel/triggers> ;
                                                                                    owl:someValuesFrom <https://ontology.architmitra.org/archimodel/TechnologyService>
                                                                                  ] ;
                                                              rdfs:subClassOf <https://ontology.architmitra.org/archimodel/Event> ;
                                                              skos:prefLabel "Technology Event" .


###  https://ontology.architmitra.org/archimodel/TechnologyFunction
<https://ontology.architmitra.org/archimodel/TechnologyFunction> rdf:type owl:Class ;
                                                                 rdfs:subClassOf <https://ontology.architmitra.org/archimodel/TechnologyInternalBehavior> ;
                                                                 skos:definition "A technology function represents a collection of technology behavior that can be performed by a node." ;
                                                                 skos:prefLabel "Technology Function" .


###  https://ontology.architmitra.org/archimodel/TechnologyInteraction
<https://ontology.architmitra.org/archimodel/TechnologyInteraction> rdf:type owl:Class ;
                                                                    rdfs:subClassOf <https://ontology.architmitra.org/archimodel/TechnologyInternalBehavior> ;
                                                                    skos:definition "A technology interaction represents a unit of collective technology behavior performed by (a collaboration of) two or more nodes." ;
                                                                    skos:prefLabel "Technology Interaction" .


###  https://ontology.architmitra.org/archimodel/TechnologyInterface
<https://ontology.architmitra.org/archimodel/TechnologyInterface> rdf:type owl:Class ;
                                                                  owl:equivalentClass [ rdf:type owl:Restriction ;
                                                                                        owl:onProperty <https://ontology.architmitra.org/archimodel/assignedTo> ;
                                                                                        owl:someValuesFrom <https://ontology.architmitra.org/archimodel/TechnologyService>
                                                                                      ] ,
                                                                                      [ rdf:type owl:Restriction ;
                                                                                        owl:onProperty <https://ontology.architmitra.org/archimodel/realizes> ;
                                                                                        owl:someValuesFrom <https://ontology.architmitra.org/archimodel/ApplicationInterface>
                                                                                      ] ,
                                                                                      [ rdf:type owl:Restriction ;
                                                                                        owl:onProperty <https://ontology.architmitra.org/archimodel/realizes> ;
                                                                                        owl:someValuesFrom <https://ontology.architmitra.org/archimodel/BusinessInterface>
                                                                                      ] ,
                                                                                      [ rdf:type owl:Restriction ;
                                                                                        owl:onProperty <https://ontology.architmitra.org/archimodel/serves> ;
                                                                                        owl:someValuesFrom <https://ontology.architmitra.org/archimodel/ApplicationInternalActiveStructure>
                                                                                      ] ,
                                                                                      [ rdf:type owl:Restriction ;
                                                                                        owl:onProperty <https://ontology.architmitra.org/archimodel/serves> ;
                                                                                        owl:someValuesFrom <https://ontology.architmitra.org/archimodel/BusinessInternalActivStructure>
                                                                                      ] ,
                                                                                      [ rdf:type owl:Restriction ;
                                                                                        owl:onProperty <https://ontology.architmitra.org/archimodel/serves> ;
                                                                                        owl:someValuesFrom <https://ontology.architmitra.org/archimodel/TechnologyInternalActiveStructure>
                                                                                      ] ;
                                                                  rdfs:subClassOf <https://ontology.architmitra.org/archimodel/ExternalActiveStructure> ;
                                                                  skos:definition "A technology interface represents a point of access where technology services offered by a node can be accessed." ;
                                                                  skos:prefLabel "Technology Interface" .


###  https://ontology.architmitra.org/archimodel/TechnologyInternalActiveStructure
<https://ontology.architmitra.org/archimodel/TechnologyInternalActiveStructure> rdf:type owl:Class ;
                                                                                owl:equivalentClass [ rdf:type owl:Restriction ;
                                                                                                      owl:onProperty <https://ontology.architmitra.org/archimodel/assignedTo> ;
                                                                                                      owl:someValuesFrom <https://ontology.architmitra.org/archimodel/Artifact>
                                                                                                    ] ,
                                                                                                    [ rdf:type owl:Restriction ;
                                                                                                      owl:onProperty <https://ontology.architmitra.org/archimodel/assignedTo> ;
                                                                                                      owl:someValuesFrom <https://ontology.architmitra.org/archimodel/TechnologyEvent>
                                                                                                    ] ,
                                                                                                    [ rdf:type owl:Restriction ;
                                                                                                      owl:onProperty <https://ontology.architmitra.org/archimodel/composedOf> ;
                                                                                                      owl:someValuesFrom <https://ontology.architmitra.org/archimodel/TechnologyInterface>
                                                                                                    ] ;
                                                                                rdfs:subClassOf <https://ontology.architmitra.org/archimodel/TechnologyActiveStructure> ;
                                                                                skos:prefLabel "Technology Internal Active Structure" .


###  https://ontology.architmitra.org/archimodel/TechnologyInternalBehavior
<https://ontology.architmitra.org/archimodel/TechnologyInternalBehavior> rdf:type owl:Class ;
                                                                         owl:equivalentClass [ rdf:type owl:Restriction ;
                                                                                               owl:onProperty <https://ontology.architmitra.org/archimodel/accesses> ;
                                                                                               owl:someValuesFrom <https://ontology.architmitra.org/archimodel/Material>
                                                                                             ] ,
                                                                                             [ rdf:type owl:Restriction ;
                                                                                               owl:onProperty <https://ontology.architmitra.org/archimodel/aggregates> ;
                                                                                               owl:someValuesFrom <https://ontology.architmitra.org/archimodel/TechnologyInternalBehavior>
                                                                                             ] ,
                                                                                             [ rdf:type owl:Restriction ;
                                                                                               owl:onProperty <https://ontology.architmitra.org/archimodel/composedOf> ;
                                                                                               owl:someValuesFrom <https://ontology.architmitra.org/archimodel/TechnologyInternalBehavior>
                                                                                             ] ,
                                                                                             [ rdf:type owl:Restriction ;
                                                                                               owl:onProperty <https://ontology.architmitra.org/archimodel/realizes> ;
                                                                                               owl:someValuesFrom <https://ontology.architmitra.org/archimodel/ApplicationInternalBehavior>
                                                                                             ] ,
                                                                                             [ rdf:type owl:Restriction ;
                                                                                               owl:onProperty <https://ontology.architmitra.org/archimodel/realizes> ;
                                                                                               owl:someValuesFrom <https://ontology.architmitra.org/archimodel/BusinessinternalBehavior>
                                                                                             ] ,
                                                                                             [ rdf:type owl:Restriction ;
                                                                                               owl:onProperty <https://ontology.architmitra.org/archimodel/realizes> ;
                                                                                               owl:someValuesFrom <https://ontology.architmitra.org/archimodel/TechnologyService>
                                                                                             ] ,
                                                                                             [ rdf:type owl:Restriction ;
                                                                                               owl:onProperty <https://ontology.architmitra.org/archimodel/triggers> ;
                                                                                               owl:someValuesFrom <https://ontology.architmitra.org/archimodel/TechnologyEvent>
                                                                                             ] ,
                                                                                             [ rdf:type owl:Restriction ;
                                                                                               owl:onProperty <https://ontology.architmitra.org/archimodel/triggers> ;
                                                                                               owl:someValuesFrom <https://ontology.architmitra.org/archimodel/TechnologyInternalBehavior>
                                                                                             ] ;
                                                                         rdfs:subClassOf <https://ontology.architmitra.org/archimodel/InternalBehavior> ;
                                                                         skos:prefLabel "Technology Internal Behavior" .


###  https://ontology.architmitra.org/archimodel/TechnologyObject
<https://ontology.architmitra.org/archimodel/TechnologyObject> rdf:type owl:Class ;
                                                               owl:equivalentClass [ rdf:type owl:Restriction ;
                                                                                     owl:onProperty <https://ontology.architmitra.org/archimodel/realizes> ;
                                                                                     owl:someValuesFrom <https://ontology.architmitra.org/archimodel/BusinessObject>
                                                                                   ] ;
                                                               rdfs:subClassOf <https://ontology.architmitra.org/archimodel/PassiveStructure> ;
                                                               skos:prefLabel "Technology Object" .


###  https://ontology.architmitra.org/archimodel/TechnologyProcess
<https://ontology.architmitra.org/archimodel/TechnologyProcess> rdf:type owl:Class ;
                                                                rdfs:subClassOf <https://ontology.architmitra.org/archimodel/TechnologyInternalBehavior> ;
                                                                skos:definition "A technology process represents a sequence of technology behaviors that achieves a specific result." ;
                                                                skos:prefLabel "Technology Process" .


###  https://ontology.architmitra.org/archimodel/TechnologyService
<https://ontology.architmitra.org/archimodel/TechnologyService> rdf:type owl:Class ;
                                                                owl:equivalentClass [ rdf:type owl:Restriction ;
                                                                                      owl:onProperty <https://ontology.architmitra.org/archimodel/accesses> ;
                                                                                      owl:someValuesFrom <https://ontology.architmitra.org/archimodel/TechnologyObject>
                                                                                    ] ,
                                                                                    [ rdf:type owl:Restriction ;
                                                                                      owl:onProperty <https://ontology.architmitra.org/archimodel/realizes> ;
                                                                                      owl:someValuesFrom <https://ontology.architmitra.org/archimodel/ApplicationService>
                                                                                    ] ,
                                                                                    [ rdf:type owl:Restriction ;
                                                                                      owl:onProperty <https://ontology.architmitra.org/archimodel/realizes> ;
                                                                                      owl:someValuesFrom <https://ontology.architmitra.org/archimodel/BusinessService>
                                                                                    ] ,
                                                                                    [ rdf:type owl:Restriction ;
                                                                                      owl:onProperty <https://ontology.architmitra.org/archimodel/serves> ;
                                                                                      owl:someValuesFrom <https://ontology.architmitra.org/archimodel/ApplicationInternalActiveStructure>
                                                                                    ] ,
                                                                                    [ rdf:type owl:Restriction ;
                                                                                      owl:onProperty <https://ontology.architmitra.org/archimodel/serves> ;
                                                                                      owl:someValuesFrom <https://ontology.architmitra.org/archimodel/ApplicationInternalBehavior>
                                                                                    ] ,
                                                                                    [ rdf:type owl:Restriction ;
                                                                                      owl:onProperty <https://ontology.architmitra.org/archimodel/serves> ;
                                                                                      owl:someValuesFrom <https://ontology.architmitra.org/archimodel/BusinessInternalActivStructure>
                                                                                    ] ,
                                                                                    [ rdf:type owl:Restriction ;
                                                                                      owl:onProperty <https://ontology.architmitra.org/archimodel/serves> ;
                                                                                      owl:someValuesFrom <https://ontology.architmitra.org/archimodel/BusinessinternalBehavior>
                                                                                    ] ,
                                                                                    [ rdf:type owl:Restriction ;
                                                                                      owl:onProperty <https://ontology.architmitra.org/archimodel/serves> ;
                                                                                      owl:someValuesFrom <https://ontology.architmitra.org/archimodel/TechnologyInternalActiveStructure>
                                                                                    ] ,
                                                                                    [ rdf:type owl:Restriction ;
                                                                                      owl:onProperty <https://ontology.architmitra.org/archimodel/serves> ;
                                                                                      owl:someValuesFrom <https://ontology.architmitra.org/archimodel/TechnologyInternalBehavior>
                                                                                    ] ,
                                                                                    [ rdf:type owl:Restriction ;
                                                                                      owl:onProperty <https://ontology.architmitra.org/archimodel/triggers> ;
                                                                                      owl:someValuesFrom <https://ontology.architmitra.org/archimodel/TechnologyEvent>
                                                                                    ] ,
                                                                                    [ rdf:type owl:Restriction ;
                                                                                      owl:onProperty <https://ontology.architmitra.org/archimodel/triggers> ;
                                                                                      owl:someValuesFrom <https://ontology.architmitra.org/archimodel/TechnologyService>
                                                                                    ] ;
                                                                rdfs:subClassOf <https://ontology.architmitra.org/archimodel/ExternalBehavior> ;
                                                                skos:prefLabel "Technology Service" .


###  https://ontology.architmitra.org/archimodel/Value
<https://ontology.architmitra.org/archimodel/Value> rdf:type owl:Class ;
                                                    owl:equivalentClass [ rdf:type owl:Restriction ;
                                                                          owl:onProperty <https://ontology.architmitra.org/archimodel/associatedWith> ;
                                                                          owl:someValuesFrom <https://ontology.architmitra.org/archimodel/Behavior>
                                                                        ] ,
                                                                        [ rdf:type owl:Restriction ;
                                                                          owl:onProperty <https://ontology.architmitra.org/archimodel/associatedWith> ;
                                                                          owl:someValuesFrom <https://ontology.architmitra.org/archimodel/Composite>
                                                                        ] ,
                                                                        [ rdf:type owl:Restriction ;
                                                                          owl:onProperty <https://ontology.architmitra.org/archimodel/associatedWith> ;
                                                                          owl:someValuesFrom <https://ontology.architmitra.org/archimodel/Structure>
                                                                        ] ;
                                                    rdfs:subClassOf <https://ontology.architmitra.org/archimodel/Motivation> ;
                                                    skos:definition "Value represents the relative worth, utility, or importance of a concept." .


###  https://ontology.architmitra.org/archimodel/ValueStream
<https://ontology.architmitra.org/archimodel/ValueStream> rdf:type owl:Class ;
                                                          rdfs:subClassOf <https://ontology.architmitra.org/archimodel/Strategy> ;
                                                          skos:definition "A value stream represents a sequence of activities that create an overall result for a customer, stakeholder, or end user." ;
                                                          skos:prefLabel "Value Stream" .


###  https://ontology.architmitra.org/archimodel/WorkPackage
<https://ontology.architmitra.org/archimodel/WorkPackage> rdf:type owl:Class ;
                                                          owl:equivalentClass [ rdf:type owl:Restriction ;
                                                                                owl:onProperty <https://ontology.architmitra.org/archimodel/accesses> ;
                                                                                owl:someValuesFrom <https://ontology.architmitra.org/archimodel/Deliverable>
                                                                              ] ,
                                                                              [ rdf:type owl:Restriction ;
                                                                                owl:onProperty <https://ontology.architmitra.org/archimodel/realizes> ;
                                                                                owl:someValuesFrom <https://ontology.architmitra.org/archimodel/Deliverable>
                                                                              ] ,
                                                                              [ rdf:type owl:Restriction ;
                                                                                owl:onProperty <https://ontology.architmitra.org/archimodel/realizes> ;
                                                                                owl:someValuesFrom <https://ontology.architmitra.org/archimodel/ExternalBehavior>
                                                                              ] ,
                                                                              [ rdf:type owl:Restriction ;
                                                                                owl:onProperty <https://ontology.architmitra.org/archimodel/realizes> ;
                                                                                owl:someValuesFrom <https://ontology.architmitra.org/archimodel/InternalBehavior>
                                                                              ] ,
                                                                              [ rdf:type owl:Restriction ;
                                                                                owl:onProperty <https://ontology.architmitra.org/archimodel/realizes> ;
                                                                                owl:someValuesFrom <https://ontology.architmitra.org/archimodel/Location>
                                                                              ] ,
                                                                              [ rdf:type owl:Restriction ;
                                                                                owl:onProperty <https://ontology.architmitra.org/archimodel/realizes> ;
                                                                                owl:someValuesFrom <https://ontology.architmitra.org/archimodel/Product>
                                                                              ] ,
                                                                              [ rdf:type owl:Restriction ;
                                                                                owl:onProperty <https://ontology.architmitra.org/archimodel/realizes> ;
                                                                                owl:someValuesFrom <https://ontology.architmitra.org/archimodel/Strategy>
                                                                              ] ,
                                                                              [ rdf:type owl:Restriction ;
                                                                                owl:onProperty <https://ontology.architmitra.org/archimodel/realizes> ;
                                                                                owl:someValuesFrom <https://ontology.architmitra.org/archimodel/Structure>
                                                                              ] ,
                                                                              [ rdf:type owl:Restriction ;
                                                                                owl:onProperty <https://ontology.architmitra.org/archimodel/triggers> ;
                                                                                owl:someValuesFrom <https://ontology.architmitra.org/archimodel/ImplementationEvent>
                                                                              ] ,
                                                                              [ rdf:type owl:Restriction ;
                                                                                owl:onProperty <https://ontology.architmitra.org/archimodel/triggers> ;
                                                                                owl:someValuesFrom <https://ontology.architmitra.org/archimodel/WorkPackage>
                                                                              ] ;
                                                          rdfs:subClassOf <https://ontology.architmitra.org/archimodel/InternalBehavior> ;
                                                          skos:prefLabel "Work Package" .


#################################################################
#    Individuals
#################################################################

###  https://ontologies.semanticarts.com/gist/_PrefixDeclaration_gist
gist:_PrefixDeclaration_gist rdf:type owl:NamedIndividual ,
                                      sh:PrefixDeclaration ;
                             sh:namespace "https://ontologies.semanticarts.com/gist/"^^xsd:anyURI ;
                             sh:prefix "gist" .


###  https://ontologies.semanticarts.com/gist/_USDollar
gist:_USDollar rdf:type owl:NamedIndividual ,
                        owl:Thing ,
                        gist:BaseUnit ;
               gist:hasBaseUnit gist:_USDollar ;
               gist:conversionFactor "1.0"^^xsd:double ;
               gist:unitSymbol "USD" ;
               rdfs:isDefinedBy <https://ontologies.semanticarts.com/o/gistCore> ;
               skos:definition "The base unit for currency." ;
               skos:prefLabel "US Dollar" .


###  https://ontologies.semanticarts.com/gist/_ampere
gist:_ampere rdf:type owl:NamedIndividual ,
                      owl:Thing ,
                      gist:BaseUnit ;
             gist:hasBaseUnit gist:_ampere ;
             gist:conversionFactor "1.0"^^xsd:double ;
             gist:unitSymbol "A" ;
             rdfs:isDefinedBy <https://ontologies.semanticarts.com/o/gistCore> ;
             skos:definition "The base unit for electrical current." ;
             skos:prefLabel "ampere" .


###  https://ontologies.semanticarts.com/gist/_bit
gist:_bit rdf:type owl:NamedIndividual ,
                   owl:Thing ,
                   gist:BaseUnit ;
          gist:hasBaseUnit gist:_bit ;
          gist:conversionFactor "1.0"^^xsd:double ;
          rdfs:isDefinedBy <https://ontologies.semanticarts.com/o/gistCore> ;
          skos:definition "The base unit for measuring digital information." ;
          skos:prefLabel "bit" ;
          skos:scopeNote "A bit (short for binary digit) is the smallest unit of data in a computer. A bit has a single binary value, either 0 or 1." .


###  https://ontologies.semanticarts.com/gist/_candela
gist:_candela rdf:type owl:NamedIndividual ,
                       owl:Thing ,
                       gist:BaseUnit ;
              gist:hasBaseUnit gist:_candela ;
              gist:conversionFactor "1.0"^^xsd:double ;
              gist:unitSymbol "cd" ;
              rdfs:isDefinedBy <https://ontologies.semanticarts.com/o/gistCore> ;
              skos:definition "The base unit for luminous intensity." ;
              skos:prefLabel "candela" .


###  https://ontologies.semanticarts.com/gist/_day
gist:_day rdf:type owl:NamedIndividual ,
                   gist:DurationUnit ;
          gist:hasBaseUnit gist:_second ;
          gist:conversionFactor "86400.0"^^xsd:double ;
          skos:definition "A duration unit that is 24 hours long." ;
          skos:prefLabel "day" .


###  https://ontologies.semanticarts.com/gist/_each
gist:_each rdf:type owl:NamedIndividual ,
                    owl:Thing ,
                    gist:BaseUnit ;
           gist:hasBaseUnit gist:_each ;
           gist:conversionFactor "1.0"^^xsd:double ;
           rdfs:isDefinedBy <https://ontologies.semanticarts.com/o/gistCore> ;
           skos:definition "The base unit for count magnitudes." ;
           skos:prefLabel "each" .


###  https://ontologies.semanticarts.com/gist/_kelvin
gist:_kelvin rdf:type owl:NamedIndividual ,
                      owl:Thing ,
                      gist:BaseUnit ;
             gist:hasBaseUnit gist:_kelvin ;
             gist:conversionFactor "1.0"^^xsd:double ;
             gist:conversionOffset "0.0"^^xsd:double ;
             gist:unitSymbol "K" ;
             rdfs:isDefinedBy <https://ontologies.semanticarts.com/o/gistCore> ;
             skos:definition "The base unit for measuring temperature." ;
             skos:prefLabel "Kelvin" .


###  https://ontologies.semanticarts.com/gist/_kilogram
gist:_kilogram rdf:type owl:NamedIndividual ,
                        owl:Thing ,
                        gist:BaseUnit ;
               gist:hasBaseUnit gist:_kilogram ;
               gist:conversionFactor "1.0"^^xsd:double ;
               gist:unitSymbol "kg" ;
               rdfs:isDefinedBy <https://ontologies.semanticarts.com/o/gistCore> ;
               skos:definition "The base unit for measuring mass." ;
               skos:prefLabel "mass" .


###  https://ontologies.semanticarts.com/gist/_meter
gist:_meter rdf:type owl:NamedIndividual ,
                     owl:Thing ,
                     gist:BaseUnit ;
            gist:hasBaseUnit gist:_meter ;
            gist:conversionFactor "1.0"^^xsd:double ;
            gist:unitSymbol "m" ;
            rdfs:isDefinedBy <https://ontologies.semanticarts.com/o/gistCore> ;
            skos:definition "The base unit for measuring distance." ;
            skos:prefLabel "distance" .


###  https://ontologies.semanticarts.com/gist/_millisecond
gist:_millisecond rdf:type owl:NamedIndividual ,
                           gist:DurationUnit ;
                  gist:hasBaseUnit gist:_second ;
                  gist:conversionFactor "0.001"^^xsd:double ;
                  gist:unitSymbol "ms" ;
                  skos:definition "A unit equal to a thousandth of a second." ;
                  skos:prefLabel "millisecond" .


###  https://ontologies.semanticarts.com/gist/_minute
gist:_minute rdf:type owl:NamedIndividual ,
                      gist:DurationUnit ;
             gist:hasBaseUnit gist:_second ;
             gist:conversionFactor "60.0"^^xsd:double ;
             gist:unitSymbol "min" ;
             skos:definition "A unit equal to 60 seconds." ;
             skos:prefLabel "minute" .


###  https://ontologies.semanticarts.com/gist/_mole
gist:_mole rdf:type owl:NamedIndividual ,
                    owl:Thing ,
                    gist:BaseUnit ;
           gist:hasBaseUnit gist:_mole ;
           gist:conversionFactor "1.0"^^xsd:double ;
           gist:unitSymbol "mol" ;
           rdfs:isDefinedBy <https://ontologies.semanticarts.com/o/gistCore> ;
           skos:definition "The base unit for measuring molar quantities." ;
           skos:prefLabel "mole" .


###  https://ontologies.semanticarts.com/gist/_second
gist:_second rdf:type owl:NamedIndividual ,
                      owl:Thing ,
                      gist:BaseUnit ;
             gist:hasBaseUnit gist:_second ;
             gist:conversionFactor "1.0"^^xsd:double ;
             gist:unitSymbol "s" ;
             rdfs:isDefinedBy <https://ontologies.semanticarts.com/o/gistCore> ;
             skos:definition "The base unit for measuring durations." ;
             skos:prefLabel "second" .


#################################################################
#    General axioms
#################################################################

[ rdf:type owl:AllDifferent ;
  owl:distinctMembers ( gist:_USDollar
                        gist:_ampere
                        gist:_bit
                        gist:_candela
                        gist:_each
                        gist:_kelvin
                        gist:_kilogram
                        gist:_meter
                        gist:_mole
                        gist:_second
                      )
] .


###  Generated by the OWL API (version 4.5.25.2023-02-15T19:15:49Z) https://github.com/owlcs/owlapi
